refine: arch-split Retype_R
Finding an interface that encompassed all architectures was tricky this
time. It required adding assumptions related to canonical_address and
sz <= maxUntypedSize when creating new objects on architectures that did
not need these previously (mainly ARM and ARM_HYP).

CreateNewCaps required a fair few wp lemmas to become part of the
Retype_R interface.

Some preconditions originating from CopyGlobalMappings had to be wrapped
up, placed in ArchCSpace_R and requalified manually due having a free
type variable that could not be placed in a locale.

APIType_capBits_generic and APIType_map2_generic lemmas were added to
the interface and declared [simp], in order to allow non-arch cap
instances to unfold the respective definitions.

Signed-off-by: Rafal Kolanski <rafal.kolanski@proofcraft.systems>

proof/refine/ARM/ArchCSpace_R.thy
@@ -1413,4 +1413,33 @@ sublocale mdb_move_gen
 
 end
 
+context Arch begin arch_global_naming
+
+(* createNewCaps can't deal with top-level page table entries on this architecture;
+   required for Retype_R setup *)
+
+definition createNewCaps_arch_ko_pre :: "(kernel_object \<Rightarrow> bool) \<Rightarrow> bool" where
+  "createNewCaps_arch_ko_pre P \<equiv>
+     \<forall>pde pde'. P (KOArch (KOPDE pde)) = P (KOArch (KOPDE pde'))"
+
+definition createNewCaps_arch_ko_type_pre :: "kernel_object_type \<Rightarrow> bool" where
+  "createNewCaps_arch_ko_type_pre ty \<equiv> ty \<noteq> koType(TYPE(pde))"
+
+(* interface lemma, but can't be locale assumption due to free type variable  *)
+lemma createNewCaps_arch_ko_type_preD:
+  "\<lbrakk> createNewCaps_arch_ko_type_pre (koType(TYPE('a::pspace_storable))) \<rbrakk>
+   \<Longrightarrow> createNewCaps_arch_ko_pre (\<lambda>ko. \<exists>obj. projectKO_opt ko = Some (obj::'a) \<and> P obj)"
+  unfolding createNewCaps_arch_ko_type_pre_def createNewCaps_arch_ko_pre_def
+  by (auto dest!: project_koType[THEN iffD1, OF exI])
+
+end (* Arch *)
+
+arch_requalify_consts
+  createNewCaps_arch_ko_pre
+  createNewCaps_arch_ko_type_pre
+
+(* requalify interface lemmas which can't be locale assumptions due to free type variable *)
+arch_requalify_facts
+  createNewCaps_arch_ko_type_preD
+
 end
