proof/refine/Retype_R.thy
@@ -12,4 +12,3898 @@ theory Retype_R
 imports ArchVSpace_R
 begin
 
+arch_requalify_consts
+  no_gs_types
+
+lemma placeNewObject_def2:
+  "placeNewObject ptr val gb = createObjects' ptr 1 (injectKO val) gb"
+  by (clarsimp simp: placeNewObject_def placeNewObject'_def createObjects'_def shiftL_nat)
+
+lemma createObjects_ret:
+  "\<lbrakk>n < 2^word_bits; n\<noteq> 0\<rbrakk> \<Longrightarrow>
+   \<lbrace>\<top>\<rbrace> createObjects y n ko gbits
+   \<lbrace>\<lambda>r s. r = map (\<lambda>p. ptr_add y (p * 2 ^ objBitsKO ko * 2 ^ gbits)) [0..< n]\<rbrace>"
+  unfolding createObjects_def createObjects'_def
+  supply toEnum_of_nat[simp del] (* not safe for generic proof *)
+  apply (simp add: split_def)
+  apply (wpsimp cong: if_cong)
+  apply (clarsimp simp: ptr_add_def upto_enum_def o_def
+                        unat_sub word_le_nat_alt
+                        power_sub[symmetric]
+                        objBits_def[symmetric]
+              simp del: upt_Suc)
+  (* avoid unfolding word_bits_def *)
+  apply (subst unat_of_nat_minus_1[where 'a=machine_word_len, folded word_bits_def];
+         clarsimp)
+  apply (clarsimp simp: shiftl_t2n)
+  (* avoid unfolding word_bits_def *)
+  apply (subst toEnum_of_nat[where 'a=machine_word_len, folded word_bits_def], simp)
+  apply (clarsimp simp: power_add)
+  done
+
+text \<open>makeObject etc. lemmas\<close>
+
+lemma NullCap_valid' [iff]: "s \<turnstile>' capability.NullCap"
+  unfolding valid_cap'_def by simp
+
+lemma valid_obj_makeObject_cte [simp]:
+  "valid_obj' (KOCTE makeObject) s"
+  unfolding valid_obj'_def valid_cte'_def
+  by (clarsimp simp: makeObject_cte)
+
+lemma valid_obj_makeObject_endpoint [simp]:
+  "valid_obj' (KOEndpoint makeObject) s"
+  unfolding valid_obj'_def valid_ep'_def
+  by (clarsimp simp: makeObject_endpoint)
+
+lemma valid_obj_makeObject_notification [simp]:
+  "valid_obj' (KONotification makeObject) s"
+  unfolding valid_obj'_def valid_ntfn'_def
+  by (clarsimp simp: makeObject_notification)
+
+lemma valid_obj_makeObject_user_data [simp]:
+  "valid_obj' (KOUserData) s"
+  unfolding valid_obj'_def by simp
+
+lemma valid_obj_makeObject_user_data_device [simp]:
+  "valid_obj' (KOUserDataDevice) s"
+  unfolding valid_obj'_def by simp
+
+text \<open>On the abstract side\<close>
+
+text \<open>Lemmas for createNewObjects etc.\<close>
+
+lemma pspace_dom_upd:
+  assumes      orth: "set as \<inter> dom ps = {}"
+  shows "pspace_dom (foldr (\<lambda>p ps. ps(p \<mapsto> ko)) as ps) =
+       pspace_dom ps \<union> (\<Union>x \<in> set as. fst ` obj_relation_cuts ko x)"
+  using orth
+  apply (subst foldr_upd_app_if)
+  apply (rule set_eqI, simp add: pspace_dom_def)
+  apply (rule iffI)
+   apply (clarsimp split: if_split_asm)
+   apply (rule rev_bexI, erule domI)
+   apply (fastforce simp: image_def)
+  apply (erule disjE)
+   apply clarsimp
+   apply (rule rev_bexI)
+    apply (clarsimp simp: domIff)
+    apply (erule exI)
+   apply clarsimp
+   apply (intro conjI impI)
+    apply (drule equals0D, erule notE, erule IntI, erule domI)
+   apply (fastforce simp: image_def)
+  apply clarsimp
+  apply (rule rev_bexI)
+   apply (clarsimp simp: domIff)
+   apply (erule(1) notE)
+  apply clarsimp
+  apply (fastforce simp: image_def)
+  done
+
+definition
+  "new_cap_addrs \<equiv> \<lambda>n ptr ko. map (\<lambda>p. ptr + ((of_nat p :: machine_word) << (objBitsKO ko)))
+                [0 ..< n]"
+
+definition
+  null_filter' :: "('a \<rightharpoonup> cte) \<Rightarrow> ('a \<rightharpoonup> cte)"
+where
+ "null_filter' f \<equiv> \<lambda>x. if f x = Some (CTE NullCap nullMDBNode) then None else f x"
+
+lemma across_null_filter_eq':
+  assumes eq: "null_filter' xs = null_filter' ys"
+  shows "\<lbrakk> xs x = Some v; ys x = Some v \<Longrightarrow> R;
+           \<lbrakk> v = CTE NullCap nullMDBNode; ys x = None \<rbrakk> \<Longrightarrow> R \<rbrakk>
+            \<Longrightarrow> R"
+  apply (cases "null_filter' xs x")
+   apply (subgoal_tac "null_filter' ys x = None")
+    apply (simp add: null_filter'_def split: if_split_asm)
+   apply (simp add: eq)
+  apply (subgoal_tac "null_filter' ys x = Some a")
+   apply (simp add: null_filter'_def split: if_split_asm)
+  apply (simp add: eq)
+  done
+
+lemma null_filter_parent_of'':
+  "\<lbrakk> null_filter' xs = null_filter' ys; xs \<turnstile> x \<leadsto> c; c \<noteq> 0 \<rbrakk>
+     \<Longrightarrow> ys \<turnstile> x \<leadsto> c"
+  apply (clarsimp simp add: mdb_next_unfold)
+  apply (drule arg_cong[where f="\<lambda>xs. xs x"])
+  apply (simp add: null_filter'_def nullPointer_def split: if_split_asm)
+  done
+
+lemma null_filter_parentOf:
+  "\<lbrakk> null_filter' xs = null_filter' ys; xs \<turnstile> x parentOf y \<rbrakk>
+      \<Longrightarrow> ys \<turnstile> x parentOf y"
+  apply (clarsimp simp add: parentOf_def)
+  apply (rule across_null_filter_eq'[where x=x], assumption+)
+   apply (erule(1) across_null_filter_eq')
+    apply clarsimp
+   apply simp
+  apply simp
+  done
+
+lemma null_filter_descendant:
+  "\<lbrakk> null_filter' xs = null_filter' ys; xs \<turnstile> x \<rightarrow> y \<rbrakk>
+      \<Longrightarrow> ys \<turnstile> x \<rightarrow> y"
+  apply (erule subtree.induct)
+   apply (rule subtree.direct_parent)
+     apply (erule(2) null_filter_parent_of'')
+    apply assumption
+   apply (erule(1) null_filter_parentOf)
+  apply (erule subtree.trans_parent)
+    apply (erule(2) null_filter_parent_of'')
+   apply assumption
+  apply (erule(1) null_filter_parentOf)
+  done
+
+lemma null_filter_descendants_of':
+  "null_filter' xs = null_filter' ys
+    \<Longrightarrow> descendants_of' x xs = descendants_of' x ys"
+  apply (simp add: descendants_of'_def)
+  apply (rule set_eqI, rule iffI)
+   apply simp
+   apply (erule(1) null_filter_descendant)
+  apply simp
+  apply (erule(1) null_filter_descendant[OF sym])
+  done
+
+lemma descendants_of_cte_at':
+  "\<lbrakk> p \<in> descendants_of x (cdt s); valid_mdb s \<rbrakk>
+  \<Longrightarrow> cte_wp_at (\<lambda>c. c \<noteq> cap.NullCap) p s"
+  apply (simp add: descendants_of_def)
+  apply (drule tranclD2)
+  apply (clarsimp simp: cdt_parent_defs valid_mdb_def mdb_cte_at_def
+                  simp del: split_paired_All)
+  apply (fastforce elim: cte_wp_at_weakenE)
+  done
+
+
+lemma descendants_of_cte_at2':
+  "\<lbrakk> p \<in> descendants_of x (cdt s); valid_mdb s \<rbrakk>
+  \<Longrightarrow> cte_wp_at (\<lambda>c. c \<noteq> cap.NullCap) x s"
+  apply (simp add: descendants_of_def)
+  apply (drule tranclD)
+  apply (clarsimp simp: cdt_parent_defs valid_mdb_def mdb_cte_at_def
+                  simp del: split_paired_All)
+  apply (fastforce elim: cte_wp_at_weakenE)
+  done
+
+lemma cte_at_next_slot'':
+  notes split_paired_All[simp del] split_paired_Ex[simp del]
+  shows "\<lbrakk>valid_list s; valid_mdb s; finite_depth (cdt s)\<rbrakk>
+    \<Longrightarrow> next_slot p (cdt_list s) (cdt s) = Some n \<Longrightarrow> cte_wp_at (\<lambda>c. c \<noteq> cap.NullCap) p s"
+  apply(simp add: next_slot_def)
+  apply(simp split: if_split_asm)
+   apply(drule next_childD, simp)
+   apply(rule_tac p=n in descendants_of_cte_at2')
+    apply(simp add: child_descendant)
+   apply(simp)
+  apply(subgoal_tac "next_not_child_dom (p, cdt_list s, cdt s)")
+   prefer 2
+   apply(simp add: next_not_child_termination valid_mdb_def valid_list_def)
+  apply(simp split: if_split_asm)
+   apply(case_tac "cdt s p")
+    apply(simp)
+   apply(rule descendants_of_cte_at')
+    apply(simp add: descendants_of_def cdt_parent_defs)
+    apply(rule r_into_trancl, simp)
+   apply(simp)
+  apply(drule next_sibD)
+  apply(elim exE conjE)
+  apply(drule after_in_list_in_list)
+  apply(rule descendants_of_cte_at')
+   apply(simp add: descendants_of_def cdt_parent_defs)
+   apply(rule r_into_trancl, simp)
+  apply(simp)
+  done
+
+lemma lookupAround2_pspace_no:
+  "is_aligned ptr sz \<Longrightarrow>
+   (case fst (lookupAround2 (ptr + 2 ^ sz - 1) ps) of None \<Rightarrow> return ()
+             | Some (x, y) \<Rightarrow> haskell_assert (x < fromPPtr ptr) [])
+      = assert ({ptr..ptr + 2 ^ sz - 1} \<inter> dom ps = {})"
+  apply (simp add: assert_def split: option.split)
+  apply safe
+    apply (clarsimp simp: lookupAround2_None1)
+   apply (clarsimp simp: lookupAround2_char1)
+  apply (clarsimp simp: lookupAround2_char1)
+  apply (drule_tac a=a in equals0D)
+  apply (simp add: linorder_not_less)
+  apply fastforce
+  done
+
+lemma pspace_no_overlap_disjoint':
+  "\<lbrakk>pspace_aligned' s;pspace_no_overlap' x n s\<rbrakk>
+   \<Longrightarrow> {x .. (x && ~~ mask n) + 2 ^ n  - 1} \<inter> dom (ksPSpace s) = {}"
+  unfolding pspace_no_overlap'_def
+  apply (rule disjointI)
+  apply (rule ccontr)
+  apply (clarsimp simp: mask_def add_diff_eq)
+  apply (elim allE impE notE)
+    apply (simp add:field_simps)+
+    apply (erule(2) order_trans[OF _ is_aligned_no_overflow,OF _ pspace_alignedD'])
+    apply (erule(1) is_aligned_no_overflow[OF pspace_alignedD'])
+  apply (erule order_trans)
+  apply (simp add:p_assoc_help)
+done
+
+lemma foldr_update_ko_wp_at':
+  assumes pv: "pspace_aligned' s" "pspace_distinct' s"
+     and pv': "pspace_aligned' (ksPSpace_update (\<lambda>x xa. if xa \<in> set addrs then Some obj else ksPSpace s xa) s)"
+              "pspace_distinct' (ksPSpace_update (\<lambda>x xa. if xa \<in> set addrs then Some obj else ksPSpace s xa) s)"
+      and al: "\<forall>x \<in> set addrs. is_aligned x (objBitsKO obj)"
+   shows
+  "ko_wp_at' P p (ksPSpace_update (\<lambda>x xa. if xa \<in> set addrs then Some obj else ksPSpace s xa) s)
+         = (if p \<in> set addrs then P obj
+                         else ko_wp_at' P p s)"
+  (is "ko_wp_at' P p ?s' = ?Q")
+  apply (clarsimp simp: ko_wp_at'_def al)
+  apply (intro conjI impI)
+   apply safe[1]
+   apply (rule pspace_distinctD' [OF _ pv'(2)])
+   apply simp
+  apply safe[1]
+   apply (simp add: ps_clear_def dom_if_Some)
+   apply blast
+  apply simp
+  apply (rule pspace_distinctD' [OF _ pv'(2)])
+  apply simp
+  done
+
+lemma foldr_update_obj_at':
+  assumes pv: "pspace_aligned' s" "pspace_distinct' s"
+     and pv': "pspace_aligned' (ksPSpace_update (\<lambda>x xa. if xa \<in> set addrs then Some obj else ksPSpace s xa) s)"
+              "pspace_distinct' (ksPSpace_update (\<lambda>x xa. if xa \<in> set addrs then Some obj else ksPSpace s xa) s)"
+      and al: "\<forall>x \<in> set addrs. is_aligned x (objBitsKO obj)"
+   shows
+  "obj_at' P p (ksPSpace_update (\<lambda>x xa. if xa \<in> set addrs then Some obj else ksPSpace s xa) s)
+         = (if p \<in> set addrs then (\<exists>obj'. projectKO_opt obj = Some obj' \<and> P obj')
+                         else obj_at' P p s)"
+  apply (simp only: obj_at'_real_def)
+  apply (rule foldr_update_ko_wp_at' [OF pv pv' al])
+  done
+
+lemma pspace_no_overlap_base':
+  "\<lbrakk>pspace_aligned' s;pspace_no_overlap' x n s; is_aligned x n \<rbrakk> \<Longrightarrow> ksPSpace s x = None"
+  apply (drule(1) pspace_no_overlap_disjoint')
+  apply (drule equals0D[where a=x])
+  apply (rule ccontr, clarsimp)
+  apply (erule is_aligned_get_word_bits)
+   apply (erule impE)
+   apply (frule mask_out_add_aligned[where q = 0,simplified,symmetric])
+   apply (fastforce simp add: is_aligned_no_overflow)
+  apply clarsimp+
+  done
+
+lemma the_ctes_makeObject:
+  "fst (the (tcb_cte_cases n)) makeObject
+     = (if tcb_cte_cases n = None
+           then fst (the None :: (Structures_H.tcb \<Rightarrow> cte) \<times> ((cte \<Rightarrow> cte) \<Rightarrow> Structures_H.tcb \<Rightarrow> Structures_H.tcb))
+                     (makeObject :: tcb)
+           else makeObject)"
+  apply (simp add: makeObject_tcb)
+  apply (clarsimp simp: tcb_cte_cases_def)
+  done
+
+lemma cte_wp_at_obj_cases_mask:
+  "cte_wp_at' P p s =
+       (obj_at' P p s \<or>
+          (p && mask tcbBlockSizeBits \<in> dom tcb_cte_cases
+             \<and> obj_at' (P \<circ> fst (the (tcb_cte_cases (p && mask tcbBlockSizeBits))))
+                     (p && ~~ mask tcbBlockSizeBits) s))"
+  apply (simp add: cte_wp_at_obj_cases')
+  apply (rule arg_cong [where f="\<lambda>x. F \<or> x" for F])
+  apply (rule iffI)
+   apply (clarsimp simp: obj_at'_def gen_objBits_simps)
+   apply (frule(1) tcb_cte_cases_aligned_helpers)
+   apply fastforce
+  apply (clarsimp simp: obj_at'_def gen_objBits_simps)
+  apply (rule bexI[where x="p && mask tcbBlockSizeBits"])
+   apply (clarsimp simp: subtract_mask)
+  apply fastforce
+  done
+
+lemma ps_clearD:
+  "\<lbrakk> ps_clear x n s; ksPSpace s y = Some v; x < y; y \<le> x + 2 ^ n - 1 \<rbrakk> \<Longrightarrow> False"
+  apply (clarsimp simp: ps_clear_def)
+  apply (drule_tac a=y in equals0D)
+  apply (simp add: dom_def mask_def add_diff_eq)
+  apply fastforce
+  done
+
+(* generic part of APIType_map2 *)
+definition APIType_map2_gen :: "apiobject_type \<Rightarrow> Structures_A.apiobject_type" where
+  "APIType_map2_gen ty \<equiv> case ty of
+       ArchTypes_H.Untyped \<Rightarrow> Structures_A.Untyped
+     | ArchTypes_H.TCBObject \<Rightarrow> Structures_A.TCBObject
+     | ArchTypes_H.EndpointObject \<Rightarrow> Structures_A.EndpointObject
+     | ArchTypes_H.NotificationObject \<Rightarrow> Structures_A.NotificationObject
+     | ArchTypes_H.CapTableObject \<Rightarrow> Structures_A.CapTableObject"
+
+(* generic part of makeObjectKO *)
+definition
+  makeObjectKO_gen :: "domain \<Rightarrow> apiobject_type \<rightharpoonup> kernel_object" where
+  "makeObjectKO_gen d ty \<equiv> case ty of
+       ArchTypes_H.TCBObject \<Rightarrow> Some (KOTCB (tcbDomain_update (\<lambda>_. d) makeObject))
+     | ArchTypes_H.EndpointObject \<Rightarrow> Some (KOEndpoint makeObject)
+     | ArchTypes_H.NotificationObject \<Rightarrow> Some (KONotification makeObject)
+     | ArchTypes_H.CapTableObject \<Rightarrow> Some (KOCTE makeObject)
+     | ArchTypes_H.Untyped \<Rightarrow> None"
+
+(* generic part of APIType_capBits *)
+definition APIType_capBits_gen :: "apiobject_type \<Rightarrow> nat \<Rightarrow> nat" where
+  "APIType_capBits_gen ty us \<equiv> case ty of
+      ArchTypes_H.Untyped \<Rightarrow> us
+    | ArchTypes_H.TCBObject \<Rightarrow> objBits (makeObject :: tcb)
+    | ArchTypes_H.EndpointObject \<Rightarrow> objBits (makeObject :: endpoint)
+    | ArchTypes_H.NotificationObject \<Rightarrow> objBits (makeObject :: Structures_H.notification)
+    | ArchTypes_H.CapTableObject \<Rightarrow> objBits (makeObject :: cte) + us"
+
+definition obj_relation_retype :: "Structures_A.kernel_object \<Rightarrow> Structures_H.kernel_object \<Rightarrow> bool"
+  where
+  "obj_relation_retype ko ko' \<equiv>
+    obj_bits ko \<ge> objBitsKO ko'
+    \<and> (\<forall>p. fst ` obj_relation_cuts ko p
+           = {p + x * 2 ^ (objBitsKO ko') | x. x < 2 ^ (obj_bits ko - objBitsKO ko')}
+           \<and> (\<forall>x \<in> obj_relation_cuts ko p. snd x ko ko'))"
+
+abbreviation
+  "injectKOS \<equiv> (injectKO :: ('a :: pspace_storable) \<Rightarrow> kernel_object)"
+
+crunch createObjects, doMachineOp
+  for ct[wp]: "\<lambda>s. P (ksCurThread s)"
+  and ksCurDomain[wp]: "\<lambda>s. P (ksCurDomain s)"
+  and qs[wp]: "\<lambda>s. P (ksReadyQueues s)"
+  and qsL1[wp]: "\<lambda>s. P (ksReadyQueuesL1Bitmap s)"
+  and qsL2[wp]: "\<lambda>s. P (ksReadyQueuesL2Bitmap s)"
+  and nosch[wp]: "\<lambda>s. P (ksSchedulerAction s)"
+  and ksDomSchedule[wp]: "\<lambda>s. P (ksDomSchedule s)"
+  and ksDomScheduleIdx[wp]: "\<lambda>s. P (ksDomScheduleIdx s)"
+  and ksInterrupt[wp]: "\<lambda>s. P (ksInterruptState s)"
+  and it[wp]: "\<lambda>s. P (ksIdleThread s)"
+  (simp: crunch_simps wp: crunch_wps setObject_ksPSpace_only updateObject_default_inv mapM_x_wp')
+
+lemma createObjects_createObjects'_inv:
+  "createObjects ptr numObjects val gSize \<lbrace>P\<rbrace>
+   = createObjects' ptr numObjects val gSize \<lbrace>P\<rbrace>"
+  unfolding createObjects_def
+  by (fastforce simp: createObjects_def valid_def bind_def return_def)
+
+locale Retype_R =
+  assumes valid_arch_tcb'_newArchTCB[simp]:
+    "\<And>s. valid_arch_tcb' newArchTCB s"
+  fixes makeObjectKO :: "bool \<Rightarrow> domain \<Rightarrow> (kernel_object + object_type) \<rightharpoonup> kernel_object"
+  fixes APIType_map2 :: "kernel_object + object_type \<Rightarrow> Structures_A.apiobject_type"
+  fixes APIType_capBits :: "object_type \<Rightarrow> nat \<Rightarrow> nat"
+  fixes update_gs :: "Structures_A.apiobject_type \<Rightarrow> nat \<Rightarrow> machine_word set
+                      \<Rightarrow> kernel_state \<Rightarrow> kernel_state"
+  assumes makeObjectKO_generic[simp]:
+    "\<And>dev d api. makeObjectKO dev d (Inr (APIObjectType api)) = makeObjectKO_gen d api"
+  assumes APIType_map2_generic[simp]:
+    "\<And>api. APIType_map2 (Inr (APIObjectType api)) = APIType_map2_gen api"
+  assumes makeObjectKO_eq:
+    "\<And>v cte tp dev d.
+      makeObjectKO dev d tp = Some v \<Longrightarrow>
+       (v = KOCTE cte)
+       = (tp = Inr (APIObjectType ArchTypes_H.apiobject_type.CapTableObject) \<and> cte = makeObject)"
+    "\<And>v tcb tp dev d.
+     makeObjectKO dev d tp = Some v \<Longrightarrow>
+       (v = KOTCB tcb)
+       = (tp = Inr (APIObjectType ArchTypes_H.apiobject_type.TCBObject)
+         \<and> tcb = tcbDomain_update (\<lambda>_. d) makeObject)"
+  assumes APIType_map2_Untyped[simp]:
+    "\<And>tp. (APIType_map2 tp = Structures_A.Untyped) = (tp = Inr (APIObjectType ArchTypes_H.Untyped))"
+  assumes APIType_map2_TCBObject[simp]:
+    "\<And>tp. (APIType_map2 tp = Structures_A.TCBObject) = (tp = Inr (APIObjectType ArchTypes_H.TCBObject))"
+  assumes APIType_capBits_generic[simp]:
+    "\<And>api us. APIType_capBits (APIObjectType api) us = APIType_capBits_gen api us"
+  assumes toAPIType_Some[simp]:
+    "\<And>ty x. (toAPIType ty = Some x) = (ty = APIObjectType x)"
+  assumes objBits_le_obj_bits_api:
+    "\<And>dev d ty ko us.
+     makeObjectKO dev d ty = Some ko \<Longrightarrow> objBitsKO ko \<le> obj_bits_api (APIType_map2 ty) us"
+  assumes ksPSpace_update_gs_eq[simp]:
+    "\<And>ty us ptrs s. ksPSpace (update_gs ty us ptrs s) = ksPSpace s"
+  assumes no_gs_types_CapTableObject:
+    "Structures_A.apiobject_type.CapTableObject \<notin> no_gs_types"
+  assumes objBitsKO_gt_0:
+    "\<And>ko. 0 < objBitsKO ko"
+  assumes arch_tcb_relation_default:
+    "arch_tcb_relation default_arch_tcb newArchTCB"
+  assumes obj_relation_retype_other_obj:
+    "\<And>ko ko'.
+     \<lbrakk> is_other_obj_relation_type (a_type ko); other_obj_relation ko ko' \<rbrakk>
+     \<Longrightarrow> obj_relation_retype ko ko'"
+  assumes update_gs_id:
+    "\<And>tp us addrs. tp \<in> no_gs_types \<Longrightarrow> update_gs tp us addrs = id"
+  assumes valid_untyped'_helper_arch_cap:
+    "\<And>s ptr sz val n acap.
+     \<lbrakk>pspace_aligned' s; pspace_distinct' s; pspace_no_overlap' ptr sz s;
+      range_cover ptr sz (objBitsKO val) n; valid_arch_cap' acap s \<rbrakk>
+     \<Longrightarrow> valid_arch_cap' acap
+          (s\<lparr>ksPSpace := foldr (\<lambda>addr. data_map_insert addr val) (new_cap_addrs n ptr val) (ksPSpace s)\<rparr>)"
+  assumes retype_in_kernel_mappings':
+    "\<And>s' ptr sz ko n.
+     \<lbrakk>pspace_in_kernel_mappings' s'; range_cover ptr sz (objBitsKO ko) n; sz \<le> maxUntypedSizeBits;
+      ptr && ~~ mask sz \<in> kernel_mappings\<rbrakk>
+     \<Longrightarrow> pspace_in_kernel_mappings'
+          (s'\<lparr>ksPSpace := foldr (\<lambda>addr. data_map_insert addr ko) (new_cap_addrs n ptr ko)
+                                (ksPSpace s')\<rparr>)"
+  assumes createNewCaps_cte_wp_at':
+    "\<And>P p ptr sz ty us n dev.
+     \<lbrace>\<lambda>s. cte_wp_at' P p s \<and>
+          range_cover ptr sz (APIType_capBits ty us) n \<and>
+          n \<noteq> 0 \<and> pspace_aligned' s \<and> pspace_distinct' s \<and> pspace_no_overlap' ptr sz s\<rbrace>
+     createNewCaps ty ptr n us dev
+     \<lbrace>\<lambda>rv. cte_wp_at' P p\<rbrace>"
+  assumes createNewCaps_arch_ko_type_pre_non_arch:
+    "\<And>ty. (case ty of ArchT _ \<Rightarrow> False | _ \<Rightarrow> True) \<Longrightarrow> createNewCaps_arch_ko_type_pre ty"
+  assumes createNewCaps_ko_wp_atQ':
+    "\<And>P P' p ptr sz ty us n dev.
+     \<lbrace>(\<lambda>s. P (ko_wp_at' P' p s)
+       \<and> range_cover ptr sz (APIType_capBits ty us) n \<and> n \<noteq> 0
+       \<and> pspace_aligned' s \<and> pspace_distinct' s
+       \<and> pspace_no_overlap' ptr sz s)
+       and K (createNewCaps_arch_ko_pre P')
+       and K (\<forall>d tcb_x. \<not>tcbQueued tcb_x \<and> tcbState tcb_x = Inactive
+                        \<longrightarrow> P' (injectKO (tcb_x \<lparr> tcbDomain := d \<rparr>)) = P' (injectKO tcb_x))
+       and (\<lambda>s. \<forall>v. makeObjectKO dev (ksCurDomain s) (Inr ty) = Some v \<longrightarrow> P' v \<longrightarrow> P True)\<rbrace>
+     createNewCaps ty ptr n us dev
+     \<lbrace>\<lambda>_ s. P (ko_wp_at' P' p s)\<rbrace>"
+  assumes createNewCaps_cte_wp_at2:
+    "\<And>P P' p n ptr sz ty objsz dev.
+     \<lbrace>\<lambda>s. P (cte_wp_at' P' p s) \<and>
+          \<not> P' makeObject \<and>
+          n \<noteq> 0 \<and>
+          range_cover ptr sz (APIType_capBits ty objsz) n \<and>
+          pspace_aligned' s \<and> pspace_distinct' s \<and> pspace_no_overlap' ptr sz s\<rbrace>
+     createNewCaps ty ptr n objsz dev
+     \<lbrace>\<lambda>rv s. P (cte_wp_at' P' p s)\<rbrace>"
+  assumes createNewCaps_ct[wp]:
+    "\<And>t regionBase numObjects userSize dev P.
+     createNewCaps t regionBase numObjects userSize dev \<lbrace>\<lambda>s. P (ksCurThread s)\<rbrace>"
+  assumes createNewCaps_ksInterrupt[wp]:
+    "\<And>t regionBase numObjects userSize dev P.
+     createNewCaps t regionBase numObjects userSize dev \<lbrace>\<lambda>s. P (ksInterruptState s)\<rbrace>"
+  assumes createNewCaps_ksCurDomain[wp]:
+    "\<And>t regionBase numObjects userSize dev P.
+     createNewCaps t regionBase numObjects userSize dev \<lbrace>\<lambda>s. P (ksCurDomain s)\<rbrace>"
+  assumes createNewCaps_it[wp]:
+    "\<And>t regionBase numObjects userSize dev P.
+     createNewCaps t regionBase numObjects userSize dev \<lbrace>\<lambda>s. P (ksIdleThread s)\<rbrace>"
+  assumes createNewCaps_nosch[wp]:
+    "\<And>t regionBase numObjects userSize dev P.
+     createNewCaps t regionBase numObjects userSize dev \<lbrace>\<lambda>s. P (ksSchedulerAction s)\<rbrace>"
+  assumes createNewCaps_ksDomSchedule[wp]:
+    "\<And>t regionBase numObjects userSize dev P.
+     createNewCaps t regionBase numObjects userSize dev \<lbrace>\<lambda>s. P (ksDomSchedule s)\<rbrace>"
+  assumes createNewCaps_ksDomScheduleIdx[wp]:
+    "\<And>t regionBase numObjects userSize dev P.
+     createNewCaps t regionBase numObjects userSize dev \<lbrace>\<lambda>s. P (ksDomScheduleIdx s)\<rbrace>"
+  assumes createNewCaps_gsUntypedZeroRanges[wp]:
+    "\<And>t regionBase numObjects userSize dev P.
+     createNewCaps t regionBase numObjects userSize dev \<lbrace>\<lambda>s. P (gsUntypedZeroRanges s)\<rbrace>"
+  assumes createNewCaps_irq_states'[wp]:
+    "\<And>t regionBase numObjects userSize dev.
+     createNewCaps t regionBase numObjects userSize dev \<lbrace>valid_irq_states'\<rbrace>"
+   assumes createNewCaps_pspace_domain_valid[wp]:
+    "\<And>ptr sz ty us n dev.
+     \<lbrace>pspace_domain_valid and K ({ptr .. (ptr && ~~ mask sz) + 2 ^ sz - 1} \<inter> kernel_data_refs = {}
+                                 \<and> range_cover ptr sz (APIType_capBits ty us) n \<and> 0 < n)\<rbrace>
+     createNewCaps ty ptr n us dev
+     \<lbrace>\<lambda>rv. pspace_domain_valid\<rbrace>"
+  assumes createNewCaps_state_refs_of':
+    "\<And>ty ptr n us dev sz.
+     \<lbrakk>range_cover ptr sz (APIType_capBits ty us) n; n \<noteq> 0\<rbrakk> \<Longrightarrow>
+     \<lbrace>\<lambda>s. valid_pspace' s \<and> pspace_no_overlap' ptr sz s \<and> P (state_refs_of' s)\<rbrace>
+     createNewCaps ty ptr n us dev
+     \<lbrace>\<lambda>rv s. P (state_refs_of' s)\<rbrace>"
+  assumes createNewCaps_state_hyp_refs_of':
+  "\<And>ty ptr n us dev sz.
+     \<lbrakk>range_cover ptr sz (APIType_capBits ty us) n; n \<noteq> 0\<rbrakk> \<Longrightarrow>
+     \<lbrace>\<lambda>s. valid_pspace' s \<and> pspace_no_overlap' ptr sz s \<and> P (state_hyp_refs_of' s)\<rbrace>
+     createNewCaps ty ptr n us dev
+     \<lbrace>\<lambda>rv s. P (state_hyp_refs_of' s)\<rbrace>"
+  assumes createNewCaps_iflive':
+    "\<And>ty ptr n us dev sz.
+     \<lbrakk>range_cover ptr sz (APIType_capBits ty us) n; n \<noteq> 0\<rbrakk> \<Longrightarrow>
+     \<lbrace>\<lambda>s. valid_pspace' s \<and> pspace_no_overlap' ptr sz s \<and> if_live_then_nonz_cap' s\<rbrace>
+     createNewCaps ty ptr n us dev
+     \<lbrace>\<lambda>rv. if_live_then_nonz_cap'\<rbrace>"
+  assumes createNewCaps_global_refs':
+    "\<And>ty ptr n us d sz.
+     \<lbrace>\<lambda>s. range_cover ptr sz (APIType_capBits ty us) n \<and> n \<noteq> 0 \<and> pspace_aligned' s \<and>
+          pspace_distinct' s \<and> pspace_no_overlap' ptr sz s \<and> valid_global_refs' s \<and>
+          0 < gsMaxObjectSize s\<rbrace>
+     createNewCaps ty ptr n us d
+     \<lbrace>\<lambda>rv. valid_global_refs'\<rbrace>"
+  assumes createNewCaps_valid_sched_pointers:
+    "\<And>ty ptr n us dev sz.
+     \<lbrace>\<lambda>s. valid_pspace' s \<and> pspace_no_overlap' ptr sz s \<and> valid_sched_pointers s\<rbrace>
+     createNewCaps ty ptr n us dev
+     \<lbrace>\<lambda>_. valid_sched_pointers\<rbrace>"
+  assumes createNewCaps_valid_bitmaps:
+    "\<And>ty ptr n us dev sz.
+     \<lbrace>\<lambda>s. valid_pspace' s \<and> pspace_no_overlap' ptr sz s \<and> valid_bitmaps s\<rbrace>
+     createNewCaps ty ptr n us dev
+     \<lbrace>\<lambda>_. valid_bitmaps\<rbrace>"
+  assumes createNewCaps_vms:
+    "\<And>ty ptr n us dev sz.
+     \<lbrace>pspace_aligned' and pspace_distinct' and pspace_no_overlap' ptr sz and
+      K (range_cover ptr sz (APIType_capBits ty us) n \<and> 0 < n) and valid_machine_state'\<rbrace>
+     createNewCaps ty ptr n us dev
+     \<lbrace>\<lambda>_. valid_machine_state'\<rbrace>"
+begin
+
+lemma valid_obj_makeObject_tcb[simp]:
+  "valid_obj' (KOTCB makeObject) s"
+  by (simp add: valid_obj'_def valid_tcb'_def makeObject_tcb tcb_cte_cases_def tcb_cte_cases_neqs
+                VPtr_def valid_tcb_state'_def minBound_word makeObject_cte)
+
+lemma valid_obj_makeObject_tcb_tcbDomain_update[simp]:
+  "d \<le> maxDomain \<Longrightarrow> valid_obj' (KOTCB (tcbDomain_update (\<lambda>_. d) makeObject)) s"
+  unfolding valid_obj'_def valid_tcb'_def valid_tcb_state'_def
+  by (clarsimp simp: makeObject_tcb makeObject_cte gen_objBits_simps minBound_word VPtr_def
+                     tcb_cte_cases_def tcb_cte_cases_neqs)
+
+lemmas gen_valid_obj_makeObject_rules =
+  valid_obj_makeObject_user_data valid_obj_makeObject_tcb
+  valid_obj_makeObject_endpoint valid_obj_makeObject_notification
+  valid_obj_makeObject_cte valid_obj_makeObject_user_data_device
+
+sublocale update_gs: pspace_update_eq' "update_gs ty us ptrs"
+  by (simp add: pspace_update_eq'_def)
+
+end
+
+lemma state_relation_null_filterE:
+  "\<lbrakk> (s, s') \<in> state_relation; t = kheap_update f s;
+     \<exists>f' g' h' as'.
+     t' = s'\<lparr>ksPSpace := f' (ksPSpace s'), gsUserPages := g' (gsUserPages s'),
+             gsCNodes := h' (gsCNodes s'),
+             ksArchState := as' (ksArchState s') \<rparr>;
+     null_filter (caps_of_state t) = null_filter (caps_of_state s);
+     null_filter' (ctes_of t') = null_filter' (ctes_of s');
+     pspace_relation (kheap t) (ksPSpace t'); ready_queues_relation t t';
+     (arch_state t, ksArchState t') \<in> arch_state_relation;
+     ghost_relation_wrapper t t';
+     valid_list s;
+     pspace_aligned' s'; pspace_distinct' s'; valid_objs s; valid_mdb s;
+     pspace_aligned' t'; pspace_distinct' t';
+     mdb_cte_at (swp (cte_wp_at ((\<noteq>) cap.NullCap)) s) (cdt s) \<rbrakk>
+      \<Longrightarrow> (t, t') \<in> state_relation"
+  apply (clarsimp simp: state_relation_def)
+  apply (intro conjI)
+     apply (simp add: cdt_relation_def cte_wp_at_caps_of_state)
+     apply (elim allEI)
+     apply clarsimp
+     apply (erule(1) across_null_filter_eq)
+      apply simp
+      apply (rule null_filter_descendants_of', simp)
+     apply simp
+     apply (case_tac "cdt s (a, b)")
+      apply (subst mdb_cte_at_no_descendants, assumption)
+       apply (simp add: cte_wp_at_caps_of_state swp_def)
+      apply (cut_tac s="kheap_update f s"  and
+                     s'="s'\<lparr>ksPSpace := f' (ksPSpace s'),
+                            gsUserPages := g' (gsUserPages s'),
+                            gsCNodes := h' (gsCNodes s'),
+                            ksArchState := as' (ksArchState s')\<rparr>"
+             in pspace_relation_ctes_ofI, simp_all)[1]
+       apply (erule caps_of_state_cteD)
+      apply (clarsimp simp: descendants_of'_def)
+      apply (case_tac cte)
+      apply (erule Null_not_subtree[rotated])
+      apply simp
+     apply (drule(1) mdb_cte_atD)
+     apply (clarsimp simp: cte_wp_at_caps_of_state)
+    apply(simp add: cdt_list_relation_def cte_wp_at_caps_of_state)
+    apply(elim allEI)
+    apply(clarsimp)
+    apply(case_tac "next_slot (a, b) (cdt_list (s)) (cdt s)")
+     apply(simp)
+    apply(subgoal_tac "cte_wp_at (\<lambda>c. c \<noteq> cap.NullCap) (a, b) s")
+     apply(drule_tac f="\<lambda>cs. cs (a, b)" in arg_cong)
+     apply(clarsimp simp: cte_wp_at_caps_of_state)
+     apply(clarsimp simp: null_filter_def split: if_split_asm)
+     apply(drule_tac f="\<lambda>ctes. ctes (cte_map (a, b))" in arg_cong)
+     apply(simp add: null_filter'_def cte_wp_at_ctes_of split: if_split_asm)
+     apply(frule pspace_relation_cte_wp_at)
+        apply(simp add: cte_wp_at_caps_of_state)
+       apply(simp)
+      apply(simp)
+     apply(simp add: cte_wp_at_ctes_of)
+    apply (simp add: mdb_cte_at_def)
+    apply(frule finite_depth)
+    apply(frule(3) cte_at_next_slot'')
+    apply simp
+   apply (simp add: revokable_relation_def)
+   apply (elim allEI, rule impI, drule(1) mp, elim allEI)
+   apply (clarsimp elim!: null_filterE)
+   apply (drule(3) pspace_relation_cte_wp_at [OF _ caps_of_state_cteD])
+   apply (drule_tac f="\<lambda>ctes. ctes (cte_map (a, b))" in arg_cong)
+   apply (clarsimp simp: null_filter'_def cte_wp_at_ctes_of
+                  split: if_split_asm)
+  done
+
+lemma None_ctes_of_cte_at:
+  "(None = ctes_of s x) = (\<not> cte_at' x s)"
+  by (fastforce simp add: cte_wp_at_ctes_of)
+
+context Retype_R begin
+
+lemma cte_wp_at_retype':
+  assumes ko: "makeObjectKO dev d tp = Some obj"
+      and pv: "pspace_aligned' s" "pspace_distinct' s"
+     and pv': "pspace_aligned' (ksPSpace_update (\<lambda>x xa. if xa \<in> set addrs then Some obj else ksPSpace s xa) s)"
+              "pspace_distinct' (ksPSpace_update (\<lambda>x xa. if xa \<in> set addrs then Some obj else ksPSpace s xa) s)"
+      and al: "\<forall>x \<in> set addrs. is_aligned x (objBitsKO obj)"
+      and pn: "\<forall>x \<in> set addrs. ksPSpace s x = None"
+  shows
+  "cte_wp_at' P p (ksPSpace_update (\<lambda>x xa. if xa \<in> set addrs then Some obj else ksPSpace s xa) s)
+      = (if tp = Inr (APIObjectType ArchTypes_H.CapTableObject) \<and> p \<in> set addrs
+           \<or> tp = Inr (APIObjectType ArchTypes_H.TCBObject)
+                         \<and> (p && ~~ mask tcbBlockSizeBits \<in> set addrs) \<and> (p && mask tcbBlockSizeBits \<in> dom tcb_cte_cases)
+              then P (CTE NullCap nullMDBNode)
+              else cte_wp_at' P p s)"
+  (is "cte_wp_at' P p ?s' = ?Q")
+  apply (subgoal_tac "\<forall>p \<in> set addrs. \<forall>(P :: cte \<Rightarrow> bool). \<not> obj_at' P p s")
+   apply (subgoal_tac "\<forall>p \<in> set addrs. \<forall>(P :: tcb \<Rightarrow> bool). \<not> obj_at' P p s")
+    apply (subgoal_tac "(\<exists>P :: cte \<Rightarrow> bool. obj_at' P p ?s')
+                          \<longrightarrow> (\<not> (\<exists>P :: tcb \<Rightarrow> bool. obj_at' P (p && ~~ mask tcbBlockSizeBits) ?s'))")
+     apply (simp only: cte_wp_at_obj_cases_mask foldr_update_obj_at'[OF pv pv' al])
+     apply (simp    add: the_ctes_makeObject makeObjectKO_eq[OF ko] makeObject_cte
+              split del: if_split
+                   cong: if_cong)
+     apply (insert al ko)
+     apply simp
+     apply (safe; simp)
+                apply ((fastforce simp: makeObject_cte makeObject_tcb tcb_cte_cases_def
+                                 split: if_split_asm)+)[12]
+    apply (clarsimp elim!: obj_atE' simp: gen_objBits_simps)
+    apply (drule ps_clearD[where y=p and n=tcbBlockSizeBits])
+       apply simp
+      apply (rule order_trans_rules(17))
+       apply (clarsimp cong: if_cong)
+      apply (rule word_and_le2)
+     apply (simp add: word_neg_and_le[simplified field_simps])
+    apply simp
+   apply (clarsimp elim!: obj_atE' simp: pn)
+  apply (clarsimp elim!: obj_atE' simp: pn)
+  done
+
+lemma ctes_of_retype:
+  assumes ko: "makeObjectKO dev d tp = Some obj"
+      and pv: "pspace_aligned' s" "pspace_distinct' s"
+     and pv': "pspace_aligned' (ksPSpace_update (\<lambda>x xa. if xa \<in> set addrs then Some obj else ksPSpace s xa) s)"
+              "pspace_distinct' (ksPSpace_update (\<lambda>x xa. if xa \<in> set addrs then Some obj else ksPSpace s xa) s)"
+      and al: "\<forall>x \<in> set addrs. is_aligned x (objBitsKO obj)"
+      and pn: "\<forall>x \<in> set addrs. ksPSpace s x = None"
+   shows
+  "map_to_ctes (\<lambda> xa. if xa \<in> set addrs then Some obj else ksPSpace s xa)
+      = (\<lambda>x. if tp = Inr (APIObjectType ArchTypes_H.CapTableObject) \<and> x \<in> set addrs
+              \<or> tp = Inr (APIObjectType ArchTypes_H.TCBObject)
+                         \<and> (x && ~~ mask tcbBlockSizeBits \<in> set addrs) \<and> (x && mask tcbBlockSizeBits \<in> dom tcb_cte_cases)
+             then Some (CTE NullCap nullMDBNode)
+             else map_to_ctes (ksPSpace s) x)"
+  (is "map_to_ctes ?ps' = ?map'")
+  using cte_wp_at_retype' [where P="(=) cte" for cte, OF ko pv pv' al pn]
+        arg_cong [where f=Not, OF cte_wp_at_retype' [OF ko pv pv' al pn, where P="\<top>"]]
+  apply (simp(no_asm_use) add: cte_wp_at_ctes_of cong: if_cong)
+  apply (rule ext)
+  apply (case_tac "map_to_ctes ?ps' x")
+   apply (simp(no_asm_simp))
+   apply (simp split: if_split_asm)
+  apply simp
+  done
+
+lemma null_filter_ctes_retype:
+  assumes ko: "makeObjectKO dev d tp = Some obj"
+      and pv: "pspace_aligned' s" "pspace_distinct' s"
+     and pv': "pspace_aligned' (ksPSpace_update (\<lambda>x xa. if xa \<in> set addrs then Some obj else ksPSpace s xa) s)"
+              "pspace_distinct' (ksPSpace_update (\<lambda>x xa. if xa \<in> set addrs then Some obj else ksPSpace s xa) s)"
+      and al: "\<forall>x \<in> set addrs. is_aligned x (objBitsKO obj)"
+      and pn: "\<forall>x \<in> set addrs. ksPSpace s x = None"
+  shows
+  "null_filter' (map_to_ctes (foldr (\<lambda>addr. data_map_insert addr obj) addrs (ksPSpace s)))
+    = null_filter' (map_to_ctes (ksPSpace s))"
+  apply (subst foldr_upd_app_if[folded data_map_insert_def])
+  apply (subst ctes_of_retype[OF ko pv pv' al pn])
+  apply (rule ext)
+  apply (clarsimp simp: null_filter'_def None_ctes_of_cte_at)
+  apply (intro conjI impI notI)
+   apply (elim cte_wp_atE' disjE conjE)
+    apply (simp_all add: pn)
+   apply (cut_tac x="ptr'" and v="if ptr' \<in> set addrs then obj else KOTCB tcb"
+                in pspace_distinctD'[OF _ pv'(2)])[1]
+    apply simp
+   apply (insert ko[symmetric],
+          simp add: makeObjectKO_gen_def gen_objBits_simps pn
+             split: if_split_asm)[1]
+   apply (drule(2) tcb_ctes_clear[where s="ksPSpace_update f s" for f s])
+    apply simp
+   apply fastforce
+  apply (cut_tac x="x && ~~ mask tcbBlockSizeBits" in pspace_distinctD'[OF _ pv'(2)])[1]
+   apply simp
+  apply (elim cte_wp_atE' disjE conjE)
+   apply (insert ko[symmetric], simp add: makeObjectKO_gen_def gen_objBits_simps)
+   apply clarsimp
+   apply (subst(asm) subtract_mask[symmetric],
+          erule_tac v="if x \<in> set addrs then KOTCB (tcbDomain_update (\<lambda>_. d) makeObject)
+                                        else KOCTE cte"
+                in tcb_space_clear)
+       apply (simp add: is_aligned_mask word_bw_assocs)
+      apply assumption
+     apply simp
+    apply simp
+   apply (simp add: pn)
+  apply (clarsimp simp: makeObjectKO_gen_def)
+  apply (drule(1) tcb_cte_cases_aligned_helpers)
+  apply (clarsimp simp: pn)
+  done
+
+end (* Retype_R *)
+
+lemma new_cap_addrs_aligned:
+  "\<lbrakk> is_aligned ptr (objBitsKO ko) \<rbrakk>
+    \<Longrightarrow> \<forall>x \<in> set (new_cap_addrs n ptr ko). is_aligned x (objBitsKO ko)"
+  apply (clarsimp simp: new_cap_addrs_def)
+  apply (erule aligned_add_aligned[OF _ is_aligned_shift])
+  apply simp
+  done
+
+lemma new_cap_addrs_distinct:
+  assumes cover: "range_cover ptr sz (objBitsKO ko) n"
+  shows "distinct (new_cap_addrs n ptr ko)"
+  unfolding new_cap_addrs_def
+  apply (simp add: distinct_map)
+  apply (rule comp_inj_on[where f=of_nat, unfolded o_def])
+   apply (rule subset_inj_on)
+    apply (rule word_unat.Abs_inj_on)
+   apply (clarsimp simp only: unats_def atLeastLessThan_iff
+                  dest!: less_two_pow_divD)
+   apply (insert cover)
+   apply (erule less_le_trans)
+   apply (insert range_cover.range_cover_n_le[OF cover])
+   apply (erule le_trans)
+   apply (cases "objBitsKO ko = 0")
+    apply (simp add:word_bits_def)
+   apply (rule less_imp_le)
+    apply (rule power_strict_increasing)
+    apply (simp add:word_bits_def)
+   apply simp
+  apply (rule inj_onI)
+  apply clarsimp
+  apply (drule arg_cong[where f="\<lambda>x. x >> objBitsKO ko"])
+  apply (cases "objBitsKO ko = 0")
+   apply simp
+  apply (subst(asm) shiftl_shiftr_id, simp add: range_cover_def)
+   apply (subst word_unat_power, rule of_nat_mono_maybe)
+    apply (rule power_strict_increasing)
+     apply (simp add: word_bits_def)
+    apply simp
+   apply (erule order_less_le_trans)
+   apply simp
+  apply (subst(asm) shiftl_shiftr_id, simp add: range_cover_def)
+   apply (subst word_unat_power, rule of_nat_mono_maybe)
+    apply (rule power_strict_increasing)
+     apply (simp add: word_bits_def)
+    apply simp
+   apply (erule order_less_le_trans)
+   apply simp
+  apply assumption
+  done
+
+lemma new_cap_addrs_subset:
+  assumes range_cover:"range_cover ptr sz (objBitsKO ko) n"
+  shows "set (new_cap_addrs n ptr ko) \<subseteq> {ptr .. ptr_add (ptr && ~~ mask sz) (2 ^ sz - 1)}"
+  apply (clarsimp simp add: new_cap_addrs_def shiftl_t2n
+                            field_simps
+                     dest!: less_two_pow_divD)
+  apply (intro conjI)
+  apply (insert range_cover)
+  apply (rule machine_word_plus_mono_right_split[OF range_cover.range_cover_compare])
+    apply assumption
+    apply simp
+    apply (simp add:range_cover_def word_bits_def)
+  apply (clarsimp simp:ptr_add_def)
+  apply (subst word_plus_and_or_coroll2[symmetric,where w = "mask sz"])
+  apply (subst add.commute)
+  apply (subst add.assoc)
+  apply (rule word_plus_mono_right)
+  apply (drule(1) range_cover.range_cover_compare)
+  apply (rule iffD1[OF le_m1_iff_lt,THEN iffD2])
+    using range_cover
+    apply (simp add: p2_gt_0 range_cover_def word_bits_def)
+   apply (rule iffD2[OF word_less_nat_alt])
+   apply (rule le_less_trans[OF unat_plus_gt])
+   using range_cover
+   apply (clarsimp simp: range_cover_def)
+  apply (insert range_cover)
+  apply (rule is_aligned_no_wrap'[OF is_aligned_neg_mask,OF le_refl ])
+   apply (simp add:range_cover_def)+
+  done
+
+lemma obj_relation_retype_cutsD:
+  "\<lbrakk> (x, P) \<in> obj_relation_cuts ko p; obj_relation_retype ko ko' \<rbrakk>
+   \<Longrightarrow> \<exists>y. x = p + y * 2 ^ (objBitsKO ko') \<and> y < 2 ^ (obj_bits ko - objBitsKO ko')
+          \<and> P ko ko'"
+  apply (clarsimp simp: obj_relation_retype_def)
+  apply (drule spec[where x=p])
+  apply clarsimp
+  apply (drule(1) bspec)
+  apply (drule arg_cong[where f="\<lambda>S. x \<in> S"])
+  apply clarsimp
+  apply (fastforce simp: image_def)
+  done
+
+lemma obj_relation_retype_leD:
+  "\<lbrakk> obj_relation_retype ko ko' \<rbrakk>
+      \<Longrightarrow> objBitsKO ko' \<le> obj_bits ko"
+  by (simp add: obj_relation_retype_def)
+
+context Retype_R begin
+
+lemma obj_relation_retype_default_leD:
+  "\<lbrakk> obj_relation_retype (default_object (APIType_map2 ty) dev us d) ko;
+       ty \<noteq> Inr (APIObjectType ArchTypes_H.Untyped) \<rbrakk>
+      \<Longrightarrow> objBitsKO ko \<le> obj_bits_api (APIType_map2 ty) us"
+  by (simp add: obj_relation_retype_def objBits_def obj_bits_dev_irr)
+
+lemma makeObjectKO_Untyped:
+  "makeObjectKO dev d ty = Some v \<Longrightarrow> ty \<noteq> Inr (APIObjectType ArchTypes_H.Untyped)"
+  by (clarsimp simp: makeObjectKO_gen_def)
+
+lemma obj_relation_retype_addrs_eq:
+  assumes not_unt:"ty \<noteq> Inr (APIObjectType ArchTypes_H.Untyped)"
+  assumes  amp: "m = 2^ ((obj_bits_api (APIType_map2 ty) us) - (objBitsKO ko)) * n"
+  assumes  orr: "obj_relation_retype (default_object (APIType_map2 ty) dev us d) ko"
+  shows  "\<lbrakk> range_cover ptr sz (obj_bits_api (APIType_map2 ty) us) n \<rbrakk> \<Longrightarrow>
+   (\<Union>x \<in> set (retype_addrs ptr (APIType_map2 ty) n us).
+            fst ` obj_relation_cuts (default_object (APIType_map2 ty) dev us d) x)
+      = set (new_cap_addrs m ptr ko)"
+  apply (rule set_eqI, rule iffI)
+   apply (clarsimp simp: retype_addrs_def)
+   apply (rename_tac p a b)
+   apply (drule obj_relation_retype_cutsD[OF _ orr])
+   apply (cut_tac obj_relation_retype_default_leD[OF orr not_unt])
+   apply (clarsimp simp: new_cap_addrs_def image_def
+                  dest!: less_two_pow_divD)
+   apply (rule_tac x="p * 2 ^ (obj_bits_api (APIType_map2 ty) us - objBitsKO ko) + unat y"
+                 in rev_bexI)
+    apply (simp add: amp obj_bits_api_default_object not_unt obj_bits_dev_irr)
+    apply (rule less_le_trans[OF nat_add_left_cancel_less[THEN iffD2]])
+    apply (erule unat_mono)
+      apply (subst unat_power_lower)
+      apply (rule le_less_trans[OF diff_le_self])
+      apply (clarsimp simp: range_cover_def
+        split: Structures_A.apiobject_type.splits)
+    apply (simp add:field_simps,subst mult_Suc[symmetric])
+    apply (rule mult_le_mono1)
+      apply simp
+   apply (simp add: ptr_add_def shiftl_t2n field_simps
+                    objBits_def[symmetric] word_unat_power[symmetric])
+   apply (simp add: power_add[symmetric])
+  apply (clarsimp simp: new_cap_addrs_def retype_addrs_def
+                 dest!: less_two_pow_divD)
+  apply (rename_tac p)
+  apply (cut_tac obj_relation_retype_default_leD[OF orr not_unt])
+  apply (cut_tac obj_relation_retype_leD[OF orr])
+  apply (case_tac "n = 0")
+    apply (simp add:amp)
+  apply (case_tac "p = 0")
+    apply simp
+    apply (rule_tac x = 0 in rev_bexI)
+    apply simp+
+    apply (rule obj_relation_cuts_trivial)
+  apply (rule_tac x="p div (2 ^ (obj_bits_api (APIType_map2 ty) us - objBitsKO ko))"
+           in rev_bexI)
+   apply (simp add:amp)
+   apply (rule td_gal_lt[THEN iffD1])
+     apply (simp add:field_simps)+
+  using orr
+  apply (clarsimp simp: obj_relation_retype_def ptr_add_def)
+  apply (thin_tac "\<forall>x. P x" for P)
+  apply (rule_tac x="of_nat (p mod (2 ^ (obj_bits_api (APIType_map2 ty) us - objBitsKO ko)))" in exI)
+  apply (simp only: word_unat_power Abs_fnat_homs shiftl_t2n)
+  apply (rule conjI)
+   apply (rule arg_cong[where f=of_nat])
+   apply (subst mult_div_rearrange)
+     apply simp
+   apply (subst minus_mod_eq_mult_div[symmetric])
+     apply (simp add:diff_mult_distrib2)
+  (* avoid revealing word_bits *)
+  apply (rule of_nat_mono_maybe[where 'a=machine_word_len, folded word_bits_def])
+   apply (rule power_strict_increasing)
+   apply (rule le_less_trans[OF diff_le_self])
+  apply (clarsimp simp: obj_bits_api_default_object obj_bits_dev_irr not_unt
+                        (* avoid revealing word_bits *)
+                        range_cover_def[where 'a=machine_word_len, folded word_bits_def])+
+  done
+
+lemma retype_pspace_relation:
+  assumes  sr: "pspace_relation (kheap s) (ksPSpace s')"
+      and  vs: "valid_pspace s" "valid_mdb s"
+      and vs': "pspace_aligned' s'" "pspace_distinct' s'"
+      and  pn: "pspace_no_overlap_range_cover ptr sz s"
+      and pn': "pspace_no_overlap' ptr sz s'"
+      and  ko: "makeObjectKO dev d ty = Some ko"
+      and cover: "range_cover ptr sz (obj_bits_api (APIType_map2 ty) us) n"
+      and orr: "obj_relation_retype (default_object (APIType_map2 ty) dev us d) ko"
+      and num_r: "m = 2 ^ (obj_bits_api (APIType_map2 ty) us - objBitsKO ko) * n"
+  shows
+  "pspace_relation (foldr (\<lambda>p ps. ps(p \<mapsto> default_object (APIType_map2 ty) dev us d))
+                              (retype_addrs ptr (APIType_map2 ty) n us) (kheap s))
+            (foldr (\<lambda>addr. data_map_insert addr ko) (new_cap_addrs m ptr ko) (ksPSpace s'))"
+  (is "pspace_relation ?ps ?ps'")
+  unfolding pspace_relation_def
+proof
+  have not_unt: "ty \<noteq> Inr (APIObjectType ArchTypes_H.Untyped)"
+     by (rule makeObjectKO_Untyped[OF ko])
+
+  have dom_not_ra:
+    "\<forall>x \<in> dom (kheap s). x \<notin> set (retype_addrs ptr (APIType_map2 ty) n us)"
+    apply clarsimp
+    apply (erule(1) pspace_no_overlapC[OF pn _ _ cover vs(1)])
+    done
+
+  hence dom_Int_ra:
+    "set (retype_addrs ptr (APIType_map2 ty) n us) \<inter> dom (kheap s) = {}"
+    by auto
+
+  note pdom = pspace_dom_upd [OF dom_Int_ra, where ko="default_object (APIType_map2 ty) dev us d"]
+
+  have pdom': "dom ?ps' = dom (ksPSpace s') \<union> set (new_cap_addrs m ptr ko)"
+    by (clarsimp simp add: foldr_upd_app_if[folded data_map_insert_def]
+                           dom_if_Some Un_commute
+                split del: if_split)
+
+  note not_unt = makeObjectKO_Untyped [OF ko]
+
+  have "pspace_dom (kheap s) = dom (ksPSpace s')"
+    using sr by (simp add: pspace_relation_def)
+
+  thus "pspace_dom ?ps = dom ?ps'"
+    apply (simp add: pdom pdom')
+    apply (rule arg_cong[where f="\<lambda>T. S \<union> T" for S])
+    apply (rule obj_relation_retype_addrs_eq[OF not_unt num_r orr cover])
+    done
+
+  have dom_same:
+    "\<And>x v. kheap s x = Some v \<Longrightarrow> ?ps x = Some v"
+    apply (frule bspec [OF dom_not_ra, OF domI])
+    apply (simp add: foldr_upd_app_if)
+    done
+  have cover':"range_cover ptr sz (objBitsKO ko) m"
+    by (rule range_cover_rel[OF cover objBits_le_obj_bits_api[OF ko] num_r])
+  have dom_same':
+    "\<And>x v. ksPSpace s' x = Some v \<Longrightarrow> ?ps' x = Some v"
+    apply (clarsimp simp:foldr_upd_app_if[folded data_map_insert_def])
+    apply (drule domI[where m = "ksPSpace s'"])
+    apply (drule(1) IntI)
+    apply (erule_tac A = "A \<inter> B" for A B in in_emptyE[rotated])
+    apply (rule disjoint_subset[OF new_cap_addrs_subset[OF cover']])
+    apply (clarsimp simp:ptr_add_def field_simps)
+    apply (rule pspace_no_overlap_disjoint'[OF vs'(1) pn'])
+  done
+
+  show "\<forall>x \<in> dom ?ps. \<forall>(y, P) \<in> obj_relation_cuts (the (?ps x)) x.
+                   P (the (?ps x)) (the (?ps' y))"
+    using sr
+    apply (clarsimp simp: pspace_relation_def)
+    apply (simp add: foldr_upd_app_if split: if_split_asm)
+     apply (clarsimp simp: foldr_upd_app_if[folded data_map_insert_def])
+     apply (rule conjI)
+      apply (drule obj_relation_retype_cutsD [OF _ orr], clarsimp)
+     apply (rule impI, erule notE)
+     apply (simp add: obj_relation_retype_addrs_eq[OF not_unt num_r orr cover,symmetric])
+     apply (erule rev_bexI)
+     apply (simp add: image_def)
+     apply (erule rev_bexI, simp)
+    apply (drule bspec, erule domI)
+    apply clarsimp
+    apply (drule(1) bspec, simp)
+    apply (subgoal_tac "a \<in> pspace_dom (kheap s)")
+     apply clarsimp
+     apply (frule dom_same', simp)
+    apply (simp(no_asm) add: pspace_dom_def)
+    apply (rule rev_bexI, erule domI)
+    apply (simp add: image_def)
+    apply (erule rev_bexI, simp)
+    done
+qed
+
+end (* Retype_R *)
+
+(*Clagged from Retype_AC*)
+lemma foldr_upd_app_if': "foldr (\<lambda>p ps. ps(p := f p)) as g = (\<lambda>x. if x \<in> set as then (f x) else g x)"
+  apply (induct as)
+   apply simp
+  apply simp
+  apply (rule ext)
+  apply simp
+  done
+
+lemma pspace_no_overlapD':
+  "\<lbrakk> ksPSpace s x = Some ko; pspace_no_overlap' p bits s \<rbrakk>
+       \<Longrightarrow> {x .. x + 2 ^ objBitsKO ko - 1} \<inter> {p .. (p && ~~ mask bits) + 2 ^ bits - 1} = {}"
+  by (simp add:pspace_no_overlap'_def mask_def add_diff_eq)
+
+lemma new_range_subset:
+  assumes
+        cover: "range_cover ptr sz (objBitsKO ko) n"
+    and addr: "x \<in> set (new_cap_addrs n ptr ko)"
+  shows       "mask_range x (objBitsKO ko) \<subseteq> {ptr .. (ptr && ~~ mask sz) + 2 ^ sz - 1}"
+  (is "?lhs \<subseteq> ?rhs")
+proof -
+  have base_in: "x \<in> {ptr..ptr_add (ptr && ~~ mask sz) (2 ^ sz - 1)}"
+    by (rule set_mp[OF new_cap_addrs_subset[OF cover] addr])
+  have aligned: "is_aligned x (objBitsKO ko)"
+    apply (insert cover)
+    apply (clarsimp simp:range_cover_def)
+    apply (drule new_cap_addrs_aligned)
+    apply (erule bspec[OF _ addr])
+  done
+  show ?thesis using base_in aligned addr
+    apply (intro range_subsetI)
+    apply (clarsimp simp:ptr_add_def field_simps)+
+    apply (simp add:x_power_minus_1)
+    apply (clarsimp simp:new_cap_addrs_def)
+   apply (subst word_plus_and_or_coroll2[symmetric,where w = "mask sz"])
+   apply (subst add.commute)
+  apply (subst add.assoc)
+  apply (subst add.assoc)
+  apply (rule word_plus_mono_right)
+  apply (simp add:mask_2pm1[symmetric])
+    apply (rule iffD2[OF shiftr_mask_cmp[where c = "objBitsKO ko"]])
+    apply (insert cover)
+      apply (simp add:range_cover_def)
+    apply (simp add:range_cover_def word_bits_def)
+       apply (subst aligned_shift')
+      apply (simp add:mask_lt_2pn range_cover_def word_bits_def )
+     apply (drule is_aligned_addD1)
+      apply (simp add:range_cover_def)
+     apply (rule aligned_add_aligned)
+       apply (rule aligned_already_mask)
+       apply (fastforce simp:range_cover_def)
+      apply (simp_all add: range_cover_def)[3]
+   apply (subst shiftr_mask2[symmetric])
+    apply (simp add:range_cover_def word_bits_def)
+   apply (rule le_shiftr)
+   apply (subst le_mask_iff_lt_2n[THEN iffD1])
+    apply (simp add:range_cover_def word_bits_def)
+   apply (clarsimp simp:word_less_nat_alt)
+   apply (rule le_less_trans[OF unat_plus_gt])
+   apply (frule(1) range_cover.range_cover_compare)
+   apply (clarsimp simp:shiftl_t2n mult.commute range_cover_def)
+  apply (rule is_aligned_no_wrap'[OF is_aligned_neg_mask])
+    apply (rule le_refl)
+   apply (simp add:range_cover_def)
+  done
+qed
+
+lemma retype_aligned_distinct':
+  assumes vs': "pspace_aligned' s'" "pspace_distinct' s'"
+      and pn': "pspace_no_overlap' ptr sz s'"
+      and cover: "range_cover ptr sz (objBitsKO ko) n "
+  shows
+  "pspace_distinct' (s' \<lparr>ksPSpace := foldr (\<lambda>addr. data_map_insert addr ko)
+                                             (new_cap_addrs n ptr ko) (ksPSpace s')\<rparr>)"
+  "pspace_aligned' (s' \<lparr>ksPSpace := foldr (\<lambda>addr. data_map_insert addr ko)
+                                             (new_cap_addrs n ptr ko) (ksPSpace s')\<rparr>)"
+  (is "pspace_aligned' (s'\<lparr>ksPSpace := ?ps\<rparr>)")
+proof -
+  have al: "is_aligned ptr (objBitsKO ko)"
+    using cover
+    by (simp add:cover range_cover_def)
+  let ?s' = "s'\<lparr>ksPSpace := ?ps\<rparr>"
+  note nc_al = bspec [OF new_cap_addrs_aligned [OF al]]
+  note nc_al' = nc_al[unfolded objBits_def]
+
+  show pa': "pspace_aligned' ?s'" using vs'(1)
+    apply (subst foldr_upd_app_if[folded data_map_insert_def])
+    apply (clarsimp simp add: pspace_aligned'_def nc_al'
+                       split: if_split_asm)
+    apply (drule bspec, erule domI, simp)
+    done
+
+  have okov: "objBitsKO ko < word_bits"
+    by (simp add: objBits_def)
+
+  have new_range_disjoint:
+    "\<And>x. x \<in> set (new_cap_addrs n ptr ko) \<Longrightarrow>
+         ({x .. x + 2 ^ (objBitsKO ko) - 1} - {x}) \<inter> set (new_cap_addrs n ptr ko) = {}"
+    apply safe
+    apply (rule ccontr)
+    apply (frule(2) aligned_neq_into_no_overlap [OF _ nc_al nc_al])
+    apply (drule_tac a=xa in equals0D)
+    apply (clarsimp simp: field_simps is_aligned_no_overflow [OF nc_al])
+    done
+  note new_range_sub = new_range_subset [OF cover]
+
+  show pd': "pspace_distinct' ?s'" using vs'(2)
+    apply (subst foldr_upd_app_if[folded data_map_insert_def])
+    apply (simp add: pspace_distinct'_def dom_if_Some ball_Un)
+    apply (intro conjI ballI impI)
+      apply (simp add: ps_clear_def dom_if_Some Int_Un_distrib mask_def add_diff_eq
+                       objBits_def[symmetric])
+      apply (rule conjI)
+       apply (erule new_range_disjoint)
+      apply (rule disjoint_subset[OF Diff_subset])
+      apply (simp only: add_mask_fold)
+      apply (erule disjoint_subset[OF new_range_sub])
+      apply (rule pspace_no_overlap_disjoint'[OF vs'(1) pn'])
+    apply (clarsimp simp add: ps_clear_def dom_if_Some Int_Un_distrib mask_def add_diff_eq)
+    apply (rule conjI)
+      apply (erule new_range_disjoint)
+     apply (rule disjoint_subset[OF Diff_subset])
+     apply (simp only: add_mask_fold)
+     apply (erule disjoint_subset[OF new_range_sub])
+     apply (rule pspace_no_overlap_disjoint'[OF vs'(1) pn'])
+    apply (clarsimp simp add: ps_clear_def dom_if_Some Int_Un_distrib)
+    apply (subst Int_commute)
+    apply (rule disjoint_subset[OF new_cap_addrs_subset,OF cover])
+    apply (subst Int_commute)
+    apply (simp add:ptr_add_def field_simps)
+    apply (rule disjoint_subset[OF Diff_subset])
+    apply (drule pspace_no_overlapD' [OF _ pn'])
+    apply (simp add: mask_def add_diff_eq)
+    done
+qed
+
+context Retype_R begin
+
+lemma retype_ksPSpace_dom_same:
+  fixes x v
+  assumes   vs': "pspace_aligned' s'" "pspace_distinct' s'"
+  assumes   pn': "pspace_no_overlap' ptr sz s'"
+  assumes    ko: "makeObjectKO dev d ty = Some ko"
+  assumes cover: "range_cover ptr sz (obj_bits_api (APIType_map2 ty) us) n"
+  assumes num_r: "m = 2 ^ (obj_bits_api (APIType_map2 ty) us - objBitsKO ko) * n"
+  shows
+    "ksPSpace s' x = Some v \<Longrightarrow>
+     foldr (\<lambda>addr. data_map_insert addr ko) (new_cap_addrs m ptr ko) (ksPSpace s') x
+      = Some v"
+proof -
+  have cover':"range_cover ptr sz (objBitsKO ko) m"
+    by (rule range_cover_rel[OF cover objBits_le_obj_bits_api[OF ko] num_r])
+  assume "ksPSpace s' x = Some v"
+  thus ?thesis
+    apply (clarsimp simp:foldr_upd_app_if[folded data_map_insert_def])
+    apply (drule domI[where m = "ksPSpace s'"])
+    apply (drule(1) IntI)
+    apply (erule_tac A = "A \<inter> B" for A B in in_emptyE[rotated])
+    apply (rule disjoint_subset[OF new_cap_addrs_subset[OF cover']])
+    apply (clarsimp simp:ptr_add_def field_simps)
+    apply (rule pspace_no_overlap_disjoint'[OF vs'(1) pn'])
+    done
+qed
+
+lemma retype_ksPSpace_None:
+  assumes ad: "pspace_aligned' s" "pspace_distinct' s"
+  assumes pn: "pspace_no_overlap' ptr sz s"
+  assumes cover: "range_cover ptr sz (objBitsKO val + gbits) n"
+  shows "\<And>x. x \<in> set (new_cap_addrs (2 ^ gbits * n) ptr val) \<Longrightarrow> ksPSpace s x = None"
+proof -
+  note cover' = range_cover_rel[where sbit' = "objBitsKO val",OF cover _ refl,simplified]
+  show "\<And>x. x \<in> set (new_cap_addrs (2 ^ gbits * n) ptr val) \<Longrightarrow> ksPSpace s x = None"
+    apply (drule subsetD[OF new_cap_addrs_subset [OF cover' ]])
+    apply (insert pspace_no_overlap_disjoint' [OF ad(1) pn])
+    apply (fastforce simp: ptr_add_def p_assoc_help)
+    done
+qed
+
+lemma retype_tcbSchedPrevs_of:
+  assumes   vs': "pspace_aligned' s'" "pspace_distinct' s'"
+  assumes   pn': "pspace_no_overlap' ptr sz s'"
+  assumes    ko: "makeObjectKO dev d ty = Some ko"
+  assumes cover: "range_cover ptr sz (obj_bits_api (APIType_map2 ty) us) n"
+  assumes num_r: "m = 2 ^ (obj_bits_api (APIType_map2 ty) us - objBitsKO ko) * n"
+  shows
+    "tcbSchedPrevs_of
+       (s'\<lparr>ksPSpace := foldr (\<lambda>addr. data_map_insert addr ko) (new_cap_addrs m ptr ko) (ksPSpace s')\<rparr>)
+     = tcbSchedPrevs_of s'"
+proof -
+  note dom_same' = retype_ksPSpace_dom_same[OF vs' pn' ko cover num_r]
+  show ?thesis
+    apply (rule ext)
+    apply (clarsimp simp: opt_map_def split: option.splits)
+    apply (intro impI conjI allI; (drule dom_same'; simp)?)
+     apply (clarsimp simp: foldr_upd_app_if[folded data_map_insert_def]
+                    split: if_split_asm kernel_object.split_asm)
+     using ko
+     apply (simp add: makeObjectKO_eq makeObjectKO_gen_def makeObject_tcb)
+    apply fastforce
+    done
+qed
+
+lemma retype_tcbSchedNexts_of:
+  assumes   vs': "pspace_aligned' s'" "pspace_distinct' s'"
+  assumes   pn': "pspace_no_overlap' ptr sz s'"
+  assumes    ko: "makeObjectKO dev d ty = Some ko"
+  assumes cover: "range_cover ptr sz (obj_bits_api (APIType_map2 ty) us) n"
+  assumes num_r: "m = 2 ^ (obj_bits_api (APIType_map2 ty) us - objBitsKO ko) * n"
+  shows
+    "tcbSchedNexts_of
+       (s'\<lparr>ksPSpace := foldr (\<lambda>addr. data_map_insert addr ko) (new_cap_addrs m ptr ko) (ksPSpace s')\<rparr>)
+     = tcbSchedNexts_of s'"
+proof -
+  note dom_same' = retype_ksPSpace_dom_same[OF vs' pn' ko cover num_r]
+  show ?thesis
+    apply (rule ext)
+    apply (clarsimp simp: opt_map_def split: option.splits)
+    apply (intro impI conjI allI; (drule dom_same'; simp)?)
+     apply (clarsimp simp: foldr_upd_app_if[folded data_map_insert_def]
+                    split: if_split_asm kernel_object.split_asm)
+     using ko
+     apply (simp add: makeObjectKO_eq makeObjectKO_gen_def makeObject_tcb)
+    apply fastforce
+    done
+qed
+
+lemma retype_inQ:
+  assumes   vs': "pspace_aligned' s'" "pspace_distinct' s'"
+  assumes   pn': "pspace_no_overlap' ptr sz s'"
+  assumes    ko: "makeObjectKO dev d ty = Some ko"
+  assumes cover: "range_cover ptr sz (obj_bits_api (APIType_map2 ty) us) n"
+  assumes num_r: "m = 2 ^ (obj_bits_api (APIType_map2 ty) us - objBitsKO ko) * n"
+  shows
+    "\<forall>d p.
+      inQ d p |< tcbs_of'
+       (s'\<lparr>ksPSpace := foldr (\<lambda>addr. data_map_insert addr ko) (new_cap_addrs m ptr ko) (ksPSpace s')\<rparr>)
+      = inQ d p |< tcbs_of' s'"
+proof -
+  note dom_same' = retype_ksPSpace_dom_same[OF vs' pn' ko cover num_r]
+  show ?thesis
+    apply (intro allI)
+    apply (rule ext)
+    apply (clarsimp simp: inQ_def opt_pred_def opt_map_def split: option.splits)
+    apply (intro impI conjI allI; (drule dom_same'; simp)?)
+     apply (clarsimp simp: foldr_upd_app_if[folded data_map_insert_def]
+                    split: if_split_asm kernel_object.split_asm)
+     using ko
+     apply (simp add: makeObjectKO_eq makeObjectKO_gen_def makeObject_tcb)
+    apply fastforce
+    done
+qed
+
+lemma retype_ready_queues_relation:
+  assumes  rlqr: "ready_queues_relation s s'"
+  assumes   vs': "pspace_aligned' s'" "pspace_distinct' s'"
+  assumes   pn': "pspace_no_overlap' ptr sz s'"
+  assumes    ko: "makeObjectKO dev d ty = Some ko"
+  assumes cover: "range_cover ptr sz (obj_bits_api (APIType_map2 ty) us) n"
+  assumes num_r: "m = 2 ^ (obj_bits_api (APIType_map2 ty) us - objBitsKO ko) * n"
+  shows
+    "ready_queues_relation
+       (s \<lparr>kheap := foldr (\<lambda>p. data_map_insert p (default_object (APIType_map2 ty) dev us d))
+                                             (retype_addrs ptr (APIType_map2 ty) n us) (kheap s)\<rparr>)
+       (s'\<lparr>ksPSpace := foldr (\<lambda>addr. data_map_insert addr ko) (new_cap_addrs m ptr ko) (ksPSpace s')\<rparr>)"
+  using rlqr
+  unfolding ready_queues_relation_def Let_def
+  by (clarsimp simp: retype_tcbSchedNexts_of[OF vs' pn' ko cover num_r, simplified]
+                     retype_tcbSchedPrevs_of[OF vs' pn' ko cover num_r, simplified]
+                     retype_inQ[OF vs' pn' ko cover num_r, simplified])
+
+end (* Retype_R *)
+
+lemma new_cap_addrs_fold':
+  "1 \<le> n \<Longrightarrow>
+   map (\<lambda>n. ptr + (n << objBitsKO ko)) [0.e.n - 1] =
+   new_cap_addrs (unat n) ptr ko"
+  by (clarsimp simp:new_cap_addrs_def ptr_add_def upto_enum_red'
+            shiftl_t2n power_add field_simps)
+
+lemma getObject_tcb_gets:
+  "getObject addr >>= (\<lambda>x::tcb. gets proj >>= (\<lambda>y. G x y))
+   = gets proj >>= (\<lambda>y. getObject addr >>= (\<lambda>x. G x y))"
+  by (auto simp: exec_gets fun_eq_iff intro: bind_apply_cong dest!: in_inv_by_hoareD[OF getObject_inv_tcb])
+
+lemma setObject_tcb_gets_ksCurDomain:
+  "setObject addr (tcb::tcb) >>= (\<lambda>_. gets ksCurDomain >>= G)
+   = gets ksCurDomain >>= (\<lambda>x. setObject addr tcb >>= (\<lambda>_. G x))"
+  apply (clarsimp simp: exec_gets fun_eq_iff)
+  apply (rule bind_apply_cong)
+   apply simp
+  apply (drule_tac P1="\<lambda>cdom. cdom = ksCurDomain x" in use_valid[OF _ setObject_cd_inv])
+  apply (simp_all add: exec_gets)
+  done
+
+lemma curDomain_mapM_x_futz:
+  "curDomain >>= (\<lambda>cdom. mapM_x (threadSet (F cdom)) addrs)
+   = mapM_x (\<lambda>addr. curDomain >>= (\<lambda>cdom. threadSet (F cdom) addr)) addrs"
+proof(induct addrs)
+  case Nil thus ?case
+    by (simp add: curDomain_def mapM_x_def sequence_x_def bind_def gets_def get_def return_def)
+next
+  case (Cons addr addrs)
+  have H: "\<And>G. do cdom \<leftarrow> curDomain;
+                   _ \<leftarrow> threadSet (F cdom) addr;
+                   G cdom
+                od
+              = do cdom \<leftarrow> curDomain;
+                   threadSet (F cdom) addr;
+                   cdom \<leftarrow> curDomain;
+                   G cdom
+                od"
+    by (simp add: bind_assoc curDomain_def threadSet_def setObject_tcb_gets_ksCurDomain
+                  getObject_tcb_gets double_gets_drop_regets)
+  from Cons.hyps show ?case
+    apply (simp add: mapM_x_def sequence_x_def)
+    apply (simp add: bind_assoc foldr_map o_def)
+    apply (subst H)
+    apply (simp add: mapM_x_def sequence_x_def)
+    done
+qed
+
+lemma default_object_ignore_domain:
+  "api \<noteq> Structures_A.TCBObject \<Longrightarrow> default_object api dev n d = default_object api dev n d'"
+  by (simp add: default_object_def split: Structures_A.apiobject_type.splits)
+
+definition caps_overlap_reserved' :: "machine_word set \<Rightarrow> kernel_state \<Rightarrow> bool" where
+ "caps_overlap_reserved' S s \<equiv>
+    \<forall>cte \<in> ran (ctes_of s). (isUntypedCap (cteCap cte) \<longrightarrow> usableUntypedRange (cteCap cte) \<inter> S = {})"
+
+definition caps_no_overlap'' :: "machine_word \<Rightarrow> nat \<Rightarrow> kernel_state \<Rightarrow> bool" where
+  "caps_no_overlap'' ptr sz s \<equiv>
+     \<forall>cte \<in> ran (ctes_of s).
+       untypedRange (cteCap cte) \<inter> {ptr .. (ptr && ~~ mask sz) + 2 ^ sz - 1} \<noteq> {}
+       \<longrightarrow> {ptr .. (ptr && ~~ mask sz) + 2 ^ sz - 1} \<subseteq> untypedRange (cteCap cte)"
+
+lemma nullPointer_0_simp[simp]:
+  "(nullPointer = 0) = True"
+  by (simp add: nullPointer_def)
+
+lemma descendants_of_retype':
+  assumes P: "\<And>p. P p \<Longrightarrow> m p = None"
+  shows "descendants_of' p (\<lambda>p. if P p then Some makeObject else m p) =
+         descendants_of' p m"
+  apply (rule set_eqI)
+  apply (simp add: descendants_of'_def)
+  apply (rule iffI)
+   apply (erule subtree.induct)
+    apply (rule direct_parent)
+      apply (clarsimp simp: mdb_next_unfold makeObject_cte split: if_split_asm)
+     apply assumption
+    apply (clarsimp simp: parentOf_def makeObject_cte split: if_split_asm)
+   apply (erule trans_parent)
+     apply (clarsimp simp: mdb_next_unfold makeObject_cte split: if_split_asm)
+    apply assumption
+   apply (clarsimp simp: parentOf_def makeObject_cte split: if_split_asm)
+  apply (erule subtree.induct)
+   apply (rule direct_parent)
+     apply (clarsimp simp: mdb_next_unfold dest!: P)
+    apply assumption
+   apply (fastforce simp: parentOf_def dest!: P)
+  apply (erule trans_parent)
+    apply (clarsimp simp: mdb_next_unfold dest!: P)
+   apply assumption
+  apply (fastforce simp: parentOf_def dest!: P)
+  done
+
+lemma capRange_Null [simp]: "capRange NullCap = {}"
+  by (simp add: capRange_def)
+
+locale retype_mdb = vmdb +
+  fixes P n
+  assumes P: "\<And>p. P p \<Longrightarrow> m p = None"
+  assumes 0: "\<not>P 0"
+  defines "n \<equiv> \<lambda>p. if P p then Some makeObject else m p"
+begin
+
+lemma no_0_n: "no_0 n"
+  using no_0 by (simp add: no_0_def n_def 0)
+
+lemma n_next:
+  "n \<turnstile> c \<leadsto> c' = (if P c then c' = 0 else m \<turnstile> c \<leadsto> c')"
+  by (simp add: mdb_next_unfold n_def makeObject_cte nullPointer_def)
+
+lemma n_prev:
+  "n \<turnstile> c \<leftarrow> c' = (if P c' then c = 0 else m \<turnstile> c \<leftarrow> c')"
+  by (simp add: mdb_prev_def n_def makeObject_cte nullPointer_def)
+
+lemma dlist_n: "valid_dlist n"
+  using dlist no_0 no_0_n
+  apply (simp add: valid_dlist_def2)
+  apply (clarsimp simp: n_prev n_next)
+  apply (rule conjI)
+   apply clarsimp
+   apply (erule allE, erule (1) impE)
+   apply (erule_tac x=c' in allE)
+   apply simp
+   apply (drule P)
+   apply (simp add: mdb_next_unfold)
+  apply clarsimp
+  apply (erule allE, erule (1) impE)
+  apply (erule_tac x=c' in allE)
+  apply simp
+  apply (drule P)
+  apply (simp add: mdb_prev_def)
+  done
+
+lemma n_next_trancl:
+  "n \<turnstile> c \<leadsto>\<^sup>+ c' \<Longrightarrow> (if P c then c' = 0 else m \<turnstile> c \<leadsto>\<^sup>+ c')"
+  apply (insert no_0_n chain)
+  apply (erule trancl_induct)
+   apply (fastforce simp: n_next)
+  apply (simp split: if_split_asm)
+   apply (clarsimp simp: mdb_next_unfold)
+  apply (simp add: n_next split: if_split_asm)
+  apply (simp add: mdb_chain_0_def)
+  apply (drule_tac x=c in bspec)
+   apply (drule tranclD)
+   apply (clarsimp simp: mdb_next_unfold)
+  apply assumption
+  done
+
+lemma next_not_P:
+  "m \<turnstile> c \<leadsto> c' \<Longrightarrow> \<not>P c"
+  by (clarsimp simp: mdb_next_unfold dest!: P)
+
+lemma m_next_trancl:
+  "m \<turnstile> c \<leadsto>\<^sup>+ c' \<Longrightarrow> n \<turnstile> c \<leadsto>\<^sup>+ c'"
+  apply (erule trancl_induct)
+   apply (rule r_into_trancl)
+   apply (clarsimp simp: n_next)
+   apply (drule next_not_P)
+   apply simp
+  apply (erule trancl_trans)
+  apply (rule r_into_trancl)
+  apply (clarsimp simp: n_next)
+  apply (drule next_not_P)
+  apply simp
+  done
+
+lemma P_to_0:
+  "P c \<Longrightarrow> n \<turnstile> c \<leadsto>\<^sup>+ 0"
+  by (rule r_into_trancl) (simp add: n_next)
+
+lemma n_trancl_eq:
+  "n \<turnstile> c \<leadsto>\<^sup>+ c' = (if P c then c' = 0 else m \<turnstile> c \<leadsto>\<^sup>+ c')"
+  by (auto dest: m_next_trancl n_next_trancl P_to_0)
+
+lemma n_rtrancl_eq:
+  "n \<turnstile> c \<leadsto>\<^sup>* c' = (if P c then c' = 0 \<or> c = c' else m \<turnstile> c \<leadsto>\<^sup>* c')"
+  by (auto simp: n_trancl_eq rtrancl_eq_or_trancl)
+
+lemma dom_n:
+  "dom n = dom m \<union> Collect P"
+  by (auto simp add: n_def)
+
+lemma mdb_chain_0_n: "mdb_chain_0 n"
+  using chain
+  by (auto simp: mdb_chain_0_def dom_n n_trancl_eq)
+
+lemma n_Some_eq:
+  "(n p = Some (CTE cap node)) =
+  (if P p then cap = NullCap \<and> node = nullMDBNode
+          else m p = Some (CTE cap node))"
+  by (auto simp: n_def makeObject_cte)
+
+lemma caps_contained_n: "caps_contained' n"
+proof -
+  from valid
+  have "caps_contained' m" ..
+  thus ?thesis
+    apply (clarsimp simp: caps_contained'_def)
+    apply (simp add: n_Some_eq split: if_split_asm)
+    apply fastforce
+    done
+qed
+
+lemma mdb_chunked_n: "mdb_chunked n"
+proof -
+  from valid
+  have "mdb_chunked m" ..
+  thus ?thesis
+    apply (clarsimp simp: mdb_chunked_def)
+    apply (simp add: n_Some_eq split: if_split_asm)
+    apply (simp add: n_Some_eq n_trancl_eq n_rtrancl_eq is_chunk_def)
+    apply fastforce
+    done
+qed
+
+lemma descendants [simp]:
+  "descendants_of' p n = descendants_of' p m"
+  apply (unfold n_def)
+  apply (subst descendants_of_retype')
+   apply (erule P)
+  apply (rule refl)
+  done
+
+lemma untyped_mdb_n: "untyped_mdb' n"
+proof -
+  from valid
+  have "untyped_mdb' m" ..
+  thus ?thesis
+    apply (clarsimp simp: untyped_mdb'_def)
+    apply (simp add: n_Some_eq split: if_split_asm)
+    done
+qed
+
+lemma untyped_inc_n: "untyped_inc' n"
+proof -
+  from valid
+  have "untyped_inc' m" ..
+  thus ?thesis
+    apply (clarsimp simp: untyped_inc'_def)
+    apply (simp add: n_Some_eq split: if_split_asm)
+    apply blast
+    done
+qed
+
+lemma valid_nullcaps_n: "valid_nullcaps n"
+proof -
+  from valid
+  have "valid_nullcaps m" ..
+  thus ?thesis
+    apply (clarsimp simp: valid_nullcaps_def)
+    apply (simp add: n_Some_eq split: if_split_asm)
+    done
+qed
+
+lemma ut_rev_n: "ut_revocable' n"
+proof -
+  from valid
+  have "ut_revocable' m" ..
+  thus ?thesis
+    apply (clarsimp simp: ut_revocable'_def)
+    apply (simp add: n_Some_eq split: if_split_asm)
+    done
+qed
+
+lemma next_not_P2:
+  "\<lbrakk> m \<turnstile> p \<leadsto> p'; p' \<noteq> nullPointer \<rbrakk> \<Longrightarrow> \<not> P p'"
+  using dlist
+  apply (clarsimp simp: mdb_next_unfold)
+  apply (erule(1) valid_dlistE)
+   apply clarsimp
+  apply (clarsimp dest!: P)
+  done
+
+lemma class_links_n:
+  "class_links n"
+  using class_links
+  apply (simp add: class_links_def)
+  apply (elim allEI)
+  apply clarsimp
+  apply (subgoal_tac "p' \<noteq> nullPointer")
+   apply (simp add: n_next split: if_split_asm)
+   apply (case_tac cte, case_tac cte')
+   apply (clarsimp simp add: n_Some_eq split: if_split_asm)
+   apply (drule(1) next_not_P2)
+   apply simp
+  apply (clarsimp simp: no_0_n nullPointer_def)
+  done
+
+lemma irq_control_n:
+  "irq_control n"
+  apply (clarsimp simp add: irq_control_def)
+  apply (simp add: n_Some_eq split: if_split_asm)
+  apply (frule irq_revocable, rule irq_control)
+  apply clarsimp
+  apply (erule (1) irq_controlD, rule irq_control)
+  done
+
+lemma dist_z_m: "distinct_zombies m"
+  using valid by auto
+
+lemma dist_z_n: "distinct_zombies n"
+  using dist_z_m
+  apply (simp add: n_def distinct_zombies_def
+                   distinct_zombie_caps_def
+               split del: if_split)
+  apply (erule allEI, erule allEI)
+  apply (clarsimp split del: if_split)
+  apply (clarsimp split: if_split_asm simp: makeObject_cte)
+  apply (clarsimp simp: gen_isCap_simps)
+  done
+
+lemma reply_masters_rvk_fb_m: "reply_masters_rvk_fb m"
+  using valid by auto
+
+lemma reply_masters_rvk_fb_n: "reply_masters_rvk_fb n"
+  using reply_masters_rvk_fb_m
+  by (simp add: n_def reply_masters_rvk_fb_def
+                ball_ran_eq makeObject_cte gen_isCap_simps)
+
+end (* retype_mdb *)
+
+locale Retype_R_2 = Retype_R +
+  assumes retype_state_relation:
+    "\<And>s s' ptr sz dev us d ko ty n m.
+     \<lbrakk>(s, s') \<in> state_relation; valid_pspace s; valid_mdb s; valid_list s; pspace_aligned' s';
+      pspace_distinct' s'; pspace_no_overlap (up_aligned_area ptr sz) s; pspace_no_overlap' ptr sz s';
+      range_cover ptr sz (obj_bits_api (APIType_map2 ty) us) n; makeObjectKO dev d ty = Some ko;
+      obj_bits_api (APIType_map2 ty) us \<le> sz;
+      obj_relation_retype (default_object (APIType_map2 ty) dev us d) ko;
+      m = 2 ^ (obj_bits_api (APIType_map2 ty) us - objBitsKO ko) * n\<rbrakk>
+     \<Longrightarrow> (s\<lparr>kheap :=
+            foldr (\<lambda>p. data_map_insert p (default_object (APIType_map2 ty) dev us d))
+             (retype_addrs ptr (APIType_map2 ty) n us) (kheap s)\<rparr>,
+        update_gs (APIType_map2 ty) us (set (retype_addrs ptr (APIType_map2 ty) n us))
+         (s'\<lparr>ksPSpace := foldr (\<lambda>addr. data_map_insert addr ko) (new_cap_addrs m ptr ko) (ksPSpace s')\<rparr>))
+       \<in> state_relation"
+  assumes createObjects_valid_objs':
+    "\<And>dev d ty val s ptr sz gbits n.
+     \<lbrakk>makeObjectKO dev d ty = Some val;
+      ty = Inr (APIObjectType ArchTypes_H.apiobject_type.TCBObject) \<longrightarrow> d \<le> maxDomain; valid_objs' s;
+      pspace_aligned' s; pspace_distinct' s; pspace_no_overlap' ptr sz s;
+      range_cover ptr sz (objBitsKO val + gbits) n; caps_no_overlap'' ptr sz s;
+      caps_overlap_reserved' {ptr..ptr + word_of_nat n * 2 ^ gbits * 2 ^ objBitsKO val - 1} s\<rbrakk>
+     \<Longrightarrow> valid_objs'
+          (s\<lparr>ksPSpace := foldr (\<lambda>addr. data_map_insert addr val)
+                               (new_cap_addrs (n * 2 ^ gbits) ptr val) (ksPSpace s)\<rparr>)"
+  assumes createNewCaps_null_filter':
+    "\<And>P ptr sz ty us n dev.
+     \<lbrace>(\<lambda>s. P (null_filter' (ctes_of s))) and pspace_aligned' and pspace_distinct' and
+      pspace_no_overlap' ptr sz and K (range_cover ptr sz (APIType_capBits ty us) n \<and> n \<noteq> 0)\<rbrace>
+     createNewCaps ty ptr n us dev
+     \<lbrace>\<lambda>_ s. P (null_filter' (ctes_of s))\<rbrace>"
+  assumes retype_mdb_valid_n: (* retype_mdb.valid_n, needs Arch *)
+    "\<And>m P. retype_mdb m P \<Longrightarrow> valid_mdb_ctes (\<lambda>p. if P p then Some makeObject else m p)"
+  assumes createNewCaps_idle'[wp]:
+    "\<And>ptr sz ty us n d.
+     \<lbrace>valid_idle' and valid_pspace' and pspace_no_overlap' ptr sz
+      and K (range_cover ptr sz (APIType_capBits ty us) n \<and> n \<noteq> 0)\<rbrace>
+     createNewCaps ty ptr n us d
+     \<lbrace>\<lambda>rv. valid_idle'\<rbrace>"
+  assumes createNewCaps_valid_arch_state:
+    "\<And>ty ptr n us d sz tp.
+     \<lbrace>(\<lambda>s. valid_arch_state' s \<and> valid_pspace' s \<and> pspace_no_overlap' ptr sz s \<and>
+          (tp = APIObjectType ArchTypes_H.apiobject_type.CapTableObject \<longrightarrow> 0 < us)) and
+      K (range_cover ptr sz (APIType_capBits ty us) n \<and> n \<noteq> 0)\<rbrace>
+     createNewCaps ty ptr n us d
+     \<lbrace>\<lambda>rv. valid_arch_state'\<rbrace>"
+  assumes createNewCaps_sched_queues:
+    "\<And>ty ptr n us dev sz P.
+     \<lbrakk>range_cover ptr sz (APIType_capBits ty us) n; n \<noteq> 0\<rbrakk> \<Longrightarrow>
+     \<lbrace>\<lambda>s. valid_pspace' s \<and> pspace_no_overlap' ptr sz s \<and> P (tcbSchedNexts_of s) (tcbSchedPrevs_of s)\<rbrace>
+     createNewCaps ty ptr n us dev
+     \<lbrace>\<lambda>_ s. P (tcbSchedNexts_of s) (tcbSchedPrevs_of s)\<rbrace>"
+  assumes createObjects_no_cte_valid_global:
+    "\<And>val ptr sz n gbits.
+     \<lbrakk>\<And>c::cte. projectKO_opt val \<noteq> Some c; \<And>t. tcb_of' val \<noteq> Some t\<rbrakk> \<Longrightarrow>
+     \<lbrace>\<lambda>s. pspace_aligned' s \<and> pspace_distinct' s \<and> pspace_no_overlap' ptr sz s \<and>
+          range_cover ptr sz (objBitsKO val + gbits) n \<and> n \<noteq> 0 \<and> valid_global_refs' s\<rbrace>
+     createObjects ptr n val gbits
+     \<lbrace>\<lambda>rv. valid_global_refs'\<rbrace>"
+  assumes createObjects_untyped_ranges_zero':
+    "\<And>val ptr sz n d ty gSize.
+     makeObjectKO dev d ty = Some val \<Longrightarrow>
+     \<lbrace>ct_active' and valid_pspace' and pspace_no_overlap' ptr sz and untyped_ranges_zero' and
+      K (range_cover ptr sz (objBitsKO val + gSize) n \<and> n \<noteq> 0)\<rbrace>
+     createObjects ptr n val gSize
+     \<lbrace>\<lambda>_. untyped_ranges_zero'\<rbrace>"
+begin
+
+lemma corres_retype':
+  assumes    not_zero: "n \<noteq> 0"
+  and         aligned: "is_aligned ptr (objBitsKO ko + gbits)"
+  and    obj_bits_api: "obj_bits_api (APIType_map2 ty) us = objBitsKO ko + gbits"
+  and           check: "(sz < obj_bits_api (APIType_map2 ty) us) = (sz < objBitsKO ko + gbits)"
+  and             usv: "APIType_map2 ty = Structures_A.CapTableObject \<Longrightarrow> 0 < us"
+  and              ko: "makeObjectKO dev d ty = Some ko"
+  and             orr: "obj_bits_api (APIType_map2 ty) us \<le> sz \<Longrightarrow>
+                        obj_relation_retype (default_object (APIType_map2 ty) dev us d) ko"
+  and           cover: "range_cover ptr sz (obj_bits_api (APIType_map2 ty) us) n"
+  shows "corres (\<lambda>rv rv'. rv' = g rv)
+                (\<lambda>s. valid_pspace s \<and> pspace_no_overlap_range_cover ptr sz s
+                     \<and> valid_mdb s \<and> valid_list s)
+                (\<lambda>s. pspace_aligned' s \<and> pspace_distinct' s \<and> pspace_no_overlap' ptr sz s
+                      \<and> (ty = Inr (APIObjectType TCBObject) \<longrightarrow> d = ksCurDomain s))
+                (retype_region ptr n us (APIType_map2 ty) dev)
+                (do addrs \<leftarrow> createObjects ptr n ko gbits;
+                    _ \<leftarrow> modify (update_gs (APIType_map2 ty) us (set addrs));
+                    return (g addrs)
+                 od)"
+  (is "corres ?r ?P ?P' ?C ?A")
+proof -
+  note data_map_insert_def[simp del]
+  have not_zero':"((of_nat n)::machine_word) \<noteq> 0"
+    by (rule range_cover_not_zero[OF not_zero cover])
+  have shiftr_not_zero:" ((of_nat n)::machine_word) << gbits \<noteq> 0"
+    apply (rule range_cover_not_zero_shift[OF not_zero cover])
+    apply (simp add:obj_bits_api)
+    done
+  have unat_of_nat_shift:"unat (((of_nat n)::machine_word) << gbits) =
+                          (n * 2^ gbits)"
+    apply (rule range_cover.unat_of_nat_n_shift[OF cover])
+    using obj_bits_api
+    apply simp
+    done
+  have unat_of_nat_shift':
+    "unat (((of_nat n)::machine_word) * 2^(gbits + objBitsKO ko)) =
+     n * 2^(gbits + objBitsKO ko)"
+    apply (subst mult.commute)
+    apply (simp add:shiftl_t2n[symmetric])
+    apply (rule range_cover.unat_of_nat_n_shift[OF cover])
+    using obj_bits_api
+    apply simp
+    done
+  have unat_of_nat_n':
+    "unat (((of_nat n)::machine_word) * 2 ^ (gbits + objBitsKO ko)) \<noteq> 0"
+    by (simp add:unat_of_nat_shift' not_zero)
+  have bound:"obj_bits_api (APIType_map2 ty) us \<le> sz"
+    using cover
+    by (simp add:range_cover_def)
+  have n_estimate: "n < 2 ^ (word_bits - (objBitsKO ko + gbits))"
+    apply (rule le_less_trans)
+    apply (rule range_cover.range_cover_n_le(2)[OF cover])
+    apply (rule power_strict_increasing)
+    apply (simp add:obj_bits_api ko)
+    apply (rule diff_less_mono)
+    using cover obj_bits_api
+    apply (simp_all add:range_cover_def ko word_bits_def)
+    done
+
+  have set_retype_addrs_fold:
+    "image (\<lambda>n. ptr + 2 ^ obj_bits_api (APIType_map2 ty) us * n)
+           {x. x \<le> of_nat n - 1} =
+     set (retype_addrs ptr (APIType_map2 ty) n us)"
+    apply (clarsimp simp: retype_addrs_def image_def Bex_def ptr_add_def
+                          Collect_eq)
+    apply (rule iffI)
+     apply (clarsimp simp: field_simps word_le_nat_alt)
+     apply (rule_tac x="unat x" in exI)
+     apply (simp add: unat_sub_if_size range_cover.unat_of_nat_n[OF cover]
+                      not_le not_zero
+               split: if_split_asm)
+    apply (clarsimp simp: field_simps word_le_nat_alt)
+    apply (rule_tac x="of_nat x" in exI)
+    apply (simp add: unat_sub_if_size range_cover.unat_of_nat_n[OF cover])
+    apply (rule nat_le_Suc_less_imp)
+    apply (metis le_unat_uoi nat_less_le not_le_imp_less)
+    done
+
+  have new_caps_adds_fold:
+    "map (\<lambda>n. ptr + 2 ^ objBitsKO ko * n) [0.e.2 ^ gbits * of_nat n - 1] =
+     new_cap_addrs (2 ^ gbits * n) ptr ko"
+    apply (simp add: new_cap_addrs_def shiftl_t2n)
+    apply (subgoal_tac "1 \<le> (2::machine_word) ^ gbits * of_nat n")
+     apply (simp add: upto_enum_red' o_def)
+     apply (rule arg_cong2[where f=map, OF refl])
+     apply (rule arg_cong2[where f=upt, OF refl])
+     apply (metis mult.commute shiftl_t2n unat_of_nat_shift)
+    using shiftr_not_zero
+    apply (simp add: shiftl_t2n)
+    apply (metis word_less_1 word_not_le)
+    done
+
+  from aligned
+  have al': "is_aligned ptr (obj_bits_api (APIType_map2 ty) us)"
+     by (simp add: obj_bits_api ko)
+  show ?thesis
+  apply (simp add: when_def retype_region_def createObjects'_def
+                   createObjects_def aligned obj_bits_api[symmetric]
+                   ko[symmetric] al' shiftl_t2n data_map_insert_def[symmetric]
+                   is_aligned_mask[symmetric] split_def unless_def
+                   lookupAround2_pspace_no check
+        split del: if_split)
+  apply (subst retype_addrs_fold)+
+  apply (subst if_P)
+    using ko
+    apply (clarsimp simp: makeObjectKO_gen_def)
+   apply (simp add: bind_assoc)
+   apply (rule corres_guard_imp)
+     apply (rule_tac r'=pspace_relation in corres_underlying_split)
+        apply (clarsimp dest!: state_relation_pspace_relation)
+       apply (simp add: gets_def)
+       apply (rule corres_symb_exec_l[rotated])
+          apply (rule exs_valid_get)
+         apply (rule get_sp)
+        apply (simp add: get_def no_fail_def)
+       apply (rule corres_symb_exec_r)
+          apply (simp add: not_less modify_modify bind_assoc[symmetric]
+                           obj_bits_api[symmetric] shiftl_t2n upto_enum_red'
+                           range_cover.unat_of_nat_n[OF cover])
+          apply (rule corres_guard_imp)
+            apply (rule corres_split_nor[OF _ corres_trivial])
+               apply (rename_tac ps ps' sa)
+               apply (rule_tac P="\<lambda>s. ps = kheap s \<and> sa = s \<and> ?P s" and
+                               P'="\<lambda>s. ps' = ksPSpace s \<and> ?P' s" in corres_modify)
+               apply(frule curdomain_relation[THEN sym])
+               apply (simp add: set_retype_addrs_fold new_caps_adds_fold)
+                apply (drule retype_state_relation[OF _ _ _ _ _ _ _ _ cover _ _ orr],
+                       simp_all add: ko not_zero obj_bits_api
+                                     bound[simplified obj_bits_api ko])[1]
+                apply (case_tac "ty = Inr (APIObjectType ArchTypes_H.apiobject_type.TCBObject)"; simp)
+                apply (subst default_object_ignore_domain)
+                 apply simp
+                apply assumption
+               apply (clarsimp simp: retype_addrs_fold[symmetric] ptr_add_def upto_enum_red' not_zero'
+                                     range_cover.unat_of_nat_n[OF cover] word_le_sub1)
+              apply (rule_tac f=g in arg_cong)
+              apply clarsimp
+             apply wpsimp+
+           apply simp+
+         apply (clarsimp split: option.splits)
+         apply (intro conjI impI)
+          apply (clarsimp|wp)+
+        apply (clarsimp split: option.splits)
+        apply wpsimp
+       apply (clarsimp split: option.splits)
+       apply (intro conjI impI)
+        apply wp
+       apply (clarsimp simp:lookupAround2_char1)
+       apply wp
+       apply (clarsimp simp: obj_bits_api ko)
+       apply (drule(1) pspace_no_overlap_disjoint')
+       apply (rule_tac x1 = a in ccontr[OF in_empty_interE])
+         apply simp
+        apply (clarsimp simp: not_less shiftL_nat)
+        apply (erule order_trans)
+        apply (subst p_assoc_help)
+        apply (subst word_plus_and_or_coroll2[symmetric,where w = "mask sz"])
+        apply (subst add.commute)
+        apply (subst add.assoc)
+        apply (rule word_plus_mono_right)
+         using cover
+         apply -
+         apply (rule iffD2[OF word_le_nat_alt])
+         apply (subst word_of_nat_minus)
+          using not_zero
+          apply simp
+         apply (rule le_trans[OF unat_plus_gt])
+         apply simp
+         apply (subst unat_minus_one)
+          apply (subst mult.commute)
+          (* avoid unfolding word_bits to keep proof generic *)
+          apply (rule word_power_nonzero[where 'a=machine_word_len, folded word_bits_def])
+            apply (rule of_nat_power[OF n_estimate, where 'a=machine_word_len, folded word_bits_def])
+            apply (simp add: objBitsKO_gt_0 ko)
+           apply (simp add: range_cover_def[where 'a=machine_word_len, folded word_bits_def]
+                            obj_bits_api ko)
+          apply (cut_tac not_zero', clarsimp simp: ko)
+         apply(clarsimp simp:field_simps ko)
+         apply (subst unat_sub[OF word_1_le_power])
+          apply (simp add:range_cover_def)
+         apply (subst diff_add_assoc[symmetric])
+          apply (cut_tac unat_of_nat_n',simp add:ko)
+         apply (clarsimp simp: obj_bits_api ko)
+         apply (rule diff_le_mono)
+         apply (frule range_cover.range_cover_compare_bound)
+         apply (cut_tac obj_bits_api unat_of_nat_shift')
+         apply (clarsimp simp:add.commute range_cover_def ko)
+        apply (rule is_aligned_no_wrap'[OF is_aligned_neg_mask,OF le_refl ])
+        apply (simp add:range_cover_def domI)+
+      apply wpsimp+
+   done
+qed
+
+end (* Retype_R_2 *)
+
+lemma createObjects_corres':
+  "\<lbrakk>corres r P P' f (createObjects a b ko d); ko = injectKO val\<rbrakk>
+   \<Longrightarrow> corres dc P P' f (createObjects' a b ko d)"
+  apply (clarsimp simp:corres_underlying_def createObjects_def return_def)
+  apply (rule conjI)
+  apply (clarsimp simp:bind_def split_def)
+    apply (drule(1) bspec)
+    apply (clarsimp simp:image_def)
+    apply (drule(1) bspec)
+    apply clarsimp
+    apply (erule bexI[rotated])
+    apply simp
+  apply (clarsimp simp:bind_def split_def image_def)
+  apply (drule(1) bspec|clarsimp)+
+  done
+
+lemmas retype_aligned_distinct'' = retype_aligned_distinct'
+       [unfolded foldr_upd_app_if[folded data_map_insert_def]]
+
+lemma retype_ko_wp_at':
+  assumes vs: "pspace_aligned' s" "pspace_distinct' s"
+     and  pn: "pspace_no_overlap' ptr sz s"
+   and cover: "range_cover ptr sz (objBitsKO obj) n"
+  shows
+  "ko_wp_at' P p (s \<lparr>ksPSpace := foldr (\<lambda>addr. data_map_insert addr obj)
+                      (new_cap_addrs n ptr obj) (ksPSpace s)\<rparr>)
+     = (if p \<in> set (new_cap_addrs n ptr obj) then P obj
+                         else ko_wp_at' P p s)"
+  apply (subst foldr_upd_app_if[folded data_map_insert_def])
+  apply (rule foldr_update_ko_wp_at' [OF vs])
+    apply (simp add: retype_aligned_distinct'' [OF vs pn cover])+
+  apply (rule new_cap_addrs_aligned)
+  using cover
+  apply (simp add:range_cover_def cover)
+  done
+
+lemma retype_obj_at':
+  assumes vs: "pspace_aligned' s" "pspace_distinct' s"
+     and  pn: "pspace_no_overlap' ptr sz s"
+     and cover: "range_cover ptr sz (objBitsKO obj) n"
+  shows
+  "obj_at' P p (s \<lparr>ksPSpace := foldr (\<lambda>addr. data_map_insert addr obj)
+                      (new_cap_addrs n ptr obj) (ksPSpace s)\<rparr>)
+     = (if p \<in> set (new_cap_addrs n ptr obj) then (\<exists>ko. projectKO_opt obj = Some ko \<and> P ko)
+                         else obj_at' P p s)"
+  unfolding obj_at'_real_def
+  apply (rule retype_ko_wp_at'[OF vs pn cover])
+done
+
+lemma retype_obj_at_disj':
+  assumes vs: "pspace_aligned' s" "pspace_distinct' s"
+     and  pn: "pspace_no_overlap' ptr sz s"
+     and cover: "range_cover ptr sz (objBitsKO obj) n"
+  shows
+  "obj_at' P p (s \<lparr>ksPSpace := foldr (\<lambda>addr. data_map_insert addr obj)
+                      (new_cap_addrs n ptr obj) (ksPSpace s)\<rparr>)
+     = (obj_at' P p s \<or> p \<in> set (new_cap_addrs n ptr obj)
+                         \<and> (\<exists>ko. projectKO_opt obj = Some ko \<and> P ko))"
+  apply (simp add: retype_obj_at' [OF vs pn cover])
+  apply (safe, simp_all)
+  apply (drule subsetD [OF new_cap_addrs_subset [OF cover]])
+  apply (insert pspace_no_overlap_disjoint' [OF vs(1) pn ])
+  apply (clarsimp simp: obj_at'_def)
+  apply (rule_tac x1 = p in ccontr[OF in_empty_interE])
+    apply (simp add:ptr_add_def p_assoc_help domI)+
+  done
+
+declare word_unat_power[symmetric,simp]
+
+lemma createObjects_ko_at_strg:
+  fixes ptr :: machine_word
+  assumes    cover: "range_cover ptr sz ((objBitsKO ko) + gbits) n"
+  assumes    not_0: "n\<noteq> 0"
+  assumes       pi: "projectKO_opt ko  = Some val"
+  shows "\<lbrace>\<lambda>s. pspace_no_overlap' ptr sz s \<and> pspace_aligned' s \<and> pspace_distinct' s\<rbrace>
+             createObjects ptr n ko gbits
+         \<lbrace>\<lambda>r s. \<forall>x \<in> set r. \<forall>offs < 2 ^ gbits. ko_at' val (x + (offs << objBitsKO ko)) s\<rbrace>"
+proof -
+  have shiftr_not_zero:" 1 \<le> ((of_nat n)::machine_word) << gbits"
+    using range_cover_not_zero_shift[OF not_0 cover,where gbits = gbits]
+    apply -
+    apply (simp add:word_le_sub1)
+    done
+  note unat_of_nat_shiftl = range_cover.unat_of_nat_n_shift[OF cover,where gbits = gbits,simplified]
+  have in_new:"\<And>idx offs. \<lbrakk>idx \<le> of_nat n - 1;offs<2 ^ gbits\<rbrakk>
+    \<Longrightarrow> ptr + (idx << objBitsKO ko + gbits) + (offs << objBitsKO ko)
+        \<in> set (new_cap_addrs (n * 2 ^ gbits) ptr ko)"
+      apply (insert range_cover_not_zero[OF not_0 cover] not_0)
+      apply (clarsimp simp:new_cap_addrs_def image_def)
+      apply (rule_tac x ="unat (2 ^ gbits * idx + offs)" in bexI)
+        apply (subst add.commute)
+        apply (simp add:shiftl_shiftl[symmetric])
+        apply (simp add:shiftl_t2n distrib_left[symmetric])
+      apply simp
+      apply (rule unat_less_helper)
+      apply (rule less_le_trans)
+       apply (erule word_plus_strict_mono_right)
+       apply (subst distrib_left[where c = "1 :: machine_word",symmetric,simplified])
+       apply (subst mult.commute[where a = "2^gbits"])+
+       apply (insert cover)
+       apply (rule word_mult_le_iff[THEN iffD2])
+         apply (simp add:p2_gt_0)
+         apply (clarsimp simp:range_cover_def word_bits_def)
+         apply (drule range_cover_rel[where sbit' = "objBitsKO ko "])
+           apply simp
+          apply simp
+         apply (rule less_le_trans)
+          apply (rule range_cover.range_cover_le_n_less)
+           apply simp
+          apply (subst unat_power_lower)
+           using cover
+           apply (clarsimp simp:range_cover_def)
+          apply (simp add:field_simps)
+          apply (rule unat_le_helper)
+          apply (erule order_trans[OF _ word_sub_1_le])
+          apply (simp add:range_cover_not_zero[OF not_0 cover])
+         apply (simp add:word_bits_def)
+        apply (drule range_cover_rel[where sbit' = "objBitsKO ko "])
+          apply simp
+         apply simp
+        apply (erule less_le_trans[OF range_cover.range_cover_le_n_less(1)])
+        apply (subst unat_power_lower)
+         using cover
+         apply (clarsimp simp:range_cover_def)
+        apply (simp add:field_simps)
+        apply (rule unat_le_helper[OF inc_le])
+        apply (simp add:word_leq_minus_one_le)
+       apply (simp add:word_bits_def)
+      apply (rule no_plus_overflow_neg)
+      apply (rule less_le_trans[where y = "of_nat n"])
+       apply unat_arith
+      using range_cover.range_cover_n_less[OF cover]
+     apply (simp add:word_bits_def)
+    apply (subst distrib_left[where c = "1 :: machine_word",symmetric,simplified])
+   apply (subst mult.commute)
+   apply simp
+   apply (rule word_mult_le_iff[THEN iffD2])
+       apply (simp add:p2_gt_0)
+      apply (simp add:range_cover_def word_bits_def)
+     apply (drule range_cover_rel[where sbit' = "objBitsKO ko "])
+       apply simp
+      apply simp
+     apply (rule less_le_trans)
+     apply (rule range_cover.range_cover_le_n_less)
+       apply simp
+     apply (subst unat_power_lower)
+       using cover
+       apply (clarsimp simp:range_cover_def)
+      apply (simp add:field_simps)
+     apply (rule unat_le_helper)
+    apply unat_arith
+   apply (simp add:word_bits_def)
+   apply (drule range_cover_rel[where sbit' = "objBitsKO ko "])
+       apply simp
+      apply simp
+     apply (rule less_le_trans)
+      apply (erule range_cover.range_cover_le_n_less)
+     apply (simp add:range_cover.unat_of_nat_n[OF cover])
+    apply (simp add: unat_le_helper)
+   apply (simp add:word_bits_def)
+  apply unat_arith
+  done
+  show ?thesis
+  apply (simp add: split_def createObjects_def lookupAround2_pspace_no
+                   alignError_def unless_def createObjects'_def)
+  apply (rule hoare_pre)
+   apply (wp|simp add:data_map_insert_def[symmetric]
+     cong: if_cong del: fun_upd_apply data_map_insert_def)+
+   apply (wpc|wp|clarsimp simp del:fun_upd_apply)+
+   apply (subst new_cap_addrs_fold'[OF shiftr_not_zero])+
+   apply (subst data_map_insert_def[symmetric])+
+   apply (subst retype_obj_at_disj')
+     apply (simp add:valid_pspace'_def unat_of_nat_shiftl)+
+     apply (rule range_cover_rel[OF cover])
+     apply simp+
+   apply (subst retype_obj_at_disj')
+     apply (simp add:valid_pspace'_def unat_of_nat_shiftl)+
+     apply (rule range_cover_rel[OF cover])
+     apply simp+
+  using range_cover.unat_of_nat_n_shift[OF cover,where gbits = gbits,simplified] pi
+  apply (simp add: in_new)
+  done
+qed
+
+lemma createObjects_ko_at:
+  fixes ptr :: machine_word
+  assumes    cover: "range_cover ptr sz ((objBitsKO ko) + gbits) n"
+  assumes    not_0: "n\<noteq> 0"
+  assumes       pi: "projectKO_opt ko = Some val"
+  shows "\<lbrace>\<lambda>s. pspace_no_overlap' ptr sz s \<and> valid_pspace' s\<rbrace>
+             createObjects ptr n ko gbits
+         \<lbrace>\<lambda>r s. \<forall>x \<in> set r. \<forall>offs < 2 ^ gbits. ko_at' val (x + (offs << objBitsKO ko)) s\<rbrace>"
+  by (wp createObjects_ko_at_strg[OF cover not_0 pi],fastforce)
+
+lemma createObjects_obj_at:
+  fixes ptr :: machine_word and val :: "'a :: pspace_storable"
+  assumes  cover:"range_cover ptr sz ((objBitsKO ko) + gbits) n"
+  and      not_0:"n \<noteq> 0"
+  and       pi: "\<exists>(val::'a). projectKO_opt ko = Some val"
+  shows "\<lbrace>\<lambda>s. pspace_no_overlap' ptr sz s \<and> valid_pspace' s\<rbrace>
+  createObjects ptr n ko gbits \<lbrace>\<lambda>r s. \<forall>x \<in> set r. \<forall>offs < 2 ^ gbits.
+                                     obj_at' (\<lambda>(x::'a). True) (x + (offs << objBitsKO ko)) s\<rbrace>"
+  apply (rule exE[OF pi])
+  apply (erule_tac val1 = x in
+    hoare_post_imp [OF _ createObjects_ko_at [OF cover not_0 ],rotated])
+  apply (intro allI ballI impI)
+  apply (drule(1) bspec)
+  apply (drule spec, drule(1) mp)
+  apply (clarsimp elim!: obj_at'_weakenE)
+  done
+
+(* until we figure out what we really need of page
+   mappings it's just alignment, which, fortunately,
+   is trivial *)
+lemma createObjects_aligned:
+  assumes al: "is_aligned ptr (objBitsKO ko + gbits)"
+  and bound :"n < 2 ^ word_bits" "n\<noteq>0"
+  and bound':"objBitsKO ko + gbits < word_bits"
+  shows "\<lbrace>\<top>\<rbrace> createObjects ptr n ko gbits
+         \<lbrace>\<lambda>rv s. \<forall>x \<in> set rv. is_aligned x (objBitsKO ko + gbits)\<rbrace>"
+  apply (rule hoare_strengthen_post)
+   apply (rule createObjects_ret[OF bound])
+  apply (clarsimp dest!: less_two_pow_divD)
+  apply (rule is_aligned_ptr_add_helper[OF al])
+  apply (simp_all add:bound')
+  done
+
+lemma createObjects_aligned2:
+  "\<lbrace>\<lambda>s. is_aligned ptr (objBitsKO ko + gbits) \<and> n < 2 ^ word_bits \<and> n \<noteq> 0
+      \<and> aln < word_bits
+      \<and> aln = objBitsKO ko + gbits\<rbrace>
+    createObjects ptr n ko gbits
+   \<lbrace>\<lambda>rv s. \<forall>x \<in> set rv. is_aligned x aln\<rbrace>"
+  apply (rule hoare_name_pre_state)
+  apply simp
+  apply (rule hoare_pre, wp createObjects_aligned, simp_all)
+  done
+
+lemma range_cover_n_wb:
+  "range_cover (ptr :: obj_ref) sz us n \<Longrightarrow> n < 2 ^ word_bits"
+  apply (rule order_le_less_trans, erule range_cover.range_cover_n_le(2))
+  apply (clarsimp simp: range_cover_def)
+  apply (simp add: word_bits_def)
+  done
+
+lemma createObjects_nonzero:
+  assumes not_0: "n \<noteq> 0"
+  assumes  cover:"range_cover ptr sz ((objBitsKO ko) + bits) n"
+  shows "\<lbrace>\<lambda>s. ptr \<noteq> 0\<rbrace>
+            createObjects ptr n ko bits
+         \<lbrace>\<lambda>rv s. \<forall>p \<in> set rv. p \<noteq> 0\<rbrace>"
+  apply (insert not_0)
+  apply (rule hoare_pre)
+   apply (rule hoare_gen_asm [where P = "ptr \<noteq> 0"])
+   using cover
+   apply (clarsimp simp:range_cover_def)
+   apply (erule is_aligned_get_word_bits,simp_all)
+  apply (rule hoare_post_imp [OF _ createObjects_ret])
+    apply (simp add: ptr_add_def)
+    apply (intro allI impI ballI)
+    apply (simp add:power_add[symmetric] mult.assoc)
+    apply (drule(1) range_cover_no_0[OF _ cover])
+    apply (simp add: objBits_def)
+   apply (simp add: range_cover_n_wb[OF cover])
+  apply simp
+  done
+
+lemmas objBits_if_dev = objBitsKO_Data
+
+lemmas capFreeIndex_update_valid_untyped' =
+  capFreeIndex_update_valid_cap'[unfolded valid_cap'_def,simplified,THEN conjunct2,THEN conjunct1]
+
+lemma word_to_tcb_flags_0[simp]:
+  "word_to_tcb_flags 0 = {}"
+  by (clarsimp simp: word_to_tcb_flags_def)
+
+context Retype_R begin
+
+lemma other_objs_default_relation:
+  "\<lbrakk> case ty of Structures_A.EndpointObject \<Rightarrow> ko = injectKO (makeObject :: endpoint)
+             | Structures_A.NotificationObject \<Rightarrow> ko = injectKO (makeObject :: Structures_H.notification)
+             | _ \<Rightarrow> False \<rbrakk> \<Longrightarrow>
+    obj_relation_retype (default_object ty dev n d) ko"
+  apply (rule obj_relation_retype_other_obj)
+   apply (clarsimp simp: default_object_def
+                  split: Structures_A.apiobject_type.split_asm)
+  apply (clarsimp simp: other_obj_relation_def default_object_def
+                        ep_relation_def ntfn_relation_def
+                        default_ep_def makeObject_endpoint default_notification_def
+                        makeObject_notification default_ntfn_def
+                 split: Structures_A.apiobject_type.split_asm)
+  done
+
+lemma tcb_relation_retype:
+  "obj_relation_retype (default_object Structures_A.TCBObject dev n d)
+                       (KOTCB (tcbDomain_update (\<lambda>_. d) makeObject))"
+  supply tcb_bits_def[simp del] (* FIXME arch-split: we might not want this in the simpset *)
+  by (clarsimp simp: tcb_relation_cut_def default_object_def obj_relation_retype_def
+                     tcb_relation_def default_tcb_def
+                     makeObject_tcb makeObject_cte
+                     fault_rel_optionation_def default_priority_def
+                     gen_objBits_simps VPtr_def tcbBlockSizeBits_tcb_bits
+                     arch_tcb_relation_default)
+
+end (* Retype_R *)
+
+lemma captable_relation_retype:
+  "n < word_bits \<Longrightarrow>
+   obj_relation_retype (default_object Structures_A.CapTableObject dev n d) (KOCTE makeObject)"
+  apply (clarsimp simp: obj_relation_retype_def default_object_def
+                        wf_empty_bits gen_objBits_simps
+                        dom_empty_cnode ex_with_length cteSizeBits_cte_level_bits)
+  apply (rule conjI)
+   defer
+   apply (clarsimp simp: cte_relation_def empty_cnode_def makeObject_cte)
+  apply (rule set_eqI, rule iffI)
+   apply (clarsimp simp: cte_map_def shiftl_t2n')
+   apply (rule_tac x="of_bl y" in exI)
+   (* avoid unfolding word_bits_def *)
+   apply (simp add: of_bl_length[where 'a=machine_word_len, folded word_bits_def])
+  apply (clarsimp simp: image_def cte_map_def shiftl_t2n')
+  apply (rule_tac x="drop (word_bits - n) (to_bl xa)" in exI)
+   (* avoid revealing word size via LENGTH *)
+  supply word_bl_Rep'[simp del]
+         word_bl_Rep'[where 'a=machine_word_len, folded word_bits_def, simp]
+  apply (simp add: of_drop_to_bl word_bits_size less_mask_eq)
+  done
+
+lemma (in Retype_R_2) corres_retype:
+  assumes    not_zero: "n \<noteq> 0"
+  and         aligned: "is_aligned ptr (objBitsKO ko + gbits)"
+  and    obj_bits_api: "obj_bits_api (APIType_map2 ty) us = objBitsKO ko + gbits"
+  and              tp: "APIType_map2 ty \<in> no_gs_types"
+  and              ko: "makeObjectKO dev d ty = Some ko"
+  and             orr: "obj_bits_api (APIType_map2 ty) us \<le> sz \<Longrightarrow>
+                        obj_relation_retype (default_object (APIType_map2 ty) dev us d) ko"
+  and           cover: "range_cover ptr sz (obj_bits_api (APIType_map2 ty) us) n"
+  shows
+    "corres (=)
+       (\<lambda>s. valid_pspace s \<and> pspace_no_overlap_range_cover ptr sz s \<and> valid_mdb s \<and> valid_list s)
+       (\<lambda>s. pspace_aligned' s \<and> pspace_distinct' s \<and> pspace_no_overlap' ptr sz s
+            \<and> (\<exists>val. ko = injectKO val)
+            \<and> (ty = Inr (APIObjectType TCBObject) \<longrightarrow> d = ksCurDomain s))
+       (retype_region ptr n us (APIType_map2 ty) dev) (createObjects ptr n ko gbits)"
+  apply (rule corres_guard_imp)
+    apply (rule_tac F = "(\<exists>val. ko = injectKO val)" in corres_gen_asm2)
+    apply (erule exE)
+    apply (rule corres_rel_imp)
+    apply (rule corres_retype'[where g=id and ty=ty and sz = sz,OF not_zero aligned _ _ _ ko,
+                                     simplified update_gs_id[OF tp] modify_id_return,simplified])
+        using assms
+        apply (simp_all add: objBits_def no_gs_types_CapTableObject)
+  apply auto
+  done
+
+lemmas gen_object_splits =
+  apiobject_type.split_asm
+  sum.split_asm kernel_object.split_asm
+
+(* FIXME: these were manually added to [wp] sometime after their definition; those declarations
+   should become localised rather than global *)
+declare hoare_in_monad_post[wp del]
+declare univ_get_wp[wp del]
+
+lemma obj_range'_subset:
+  "\<lbrakk>range_cover ptr sz (objBitsKO val) n; ptr' \<in> set (new_cap_addrs n ptr val)\<rbrakk>
+   \<Longrightarrow> obj_range' ptr' val \<subseteq> {ptr..(ptr && ~~ mask sz) + 2 ^ sz - 1}"
+  unfolding obj_range'_def
+  by (rule new_range_subset, auto)
+
+lemma obj_range'_subset_strong:
+  assumes "range_cover ptr sz (objBitsKO val) n"
+      and "ptr' \<in> set (new_cap_addrs n ptr val)"
+  shows "obj_range' ptr' val \<subseteq> {ptr..ptr + (of_nat n * 2 ^ objBitsKO val) - 1}"
+proof -
+  {
+    assume cover: "range_cover ptr sz (objBitsKO val) n"
+      and  mem_p: "ptr' \<in> set (new_cap_addrs n ptr val)"
+      and  not_0: "n\<noteq> 0"
+    note n_less = range_cover.range_cover_n_less[OF cover]
+    have unat_of_nat_m1: "unat (of_nat n - (1::machine_word)) < n"
+      using not_0 n_less by (simp add:unat_of_nat_minus_1)
+    have decomp:
+      "of_nat n * 2 ^ objBitsKO val =
+       of_nat (n - 1) * 2 ^ objBitsKO val + (2 :: machine_word) ^ objBitsKO val"
+      apply (simp add:distrib_right[where b = "1 :: machine_word",simplified,symmetric])
+      using not_0 n_less
+      apply simp
+      done
+    have "ptr' + 2 ^ objBitsKO val - 1 \<le> ptr + of_nat n * 2 ^ objBitsKO val - 1"
+      using cover
+      apply (subst decomp)
+      apply (simp add:add.assoc[symmetric])
+      apply (simp add:p_assoc_help)
+      apply (rule order_trans[OF word_plus_mono_left word_plus_mono_right])
+         using mem_p not_0
+         apply (clarsimp simp:new_cap_addrs_def shiftl_t2n)
+         apply (rule word_plus_mono_right)
+          apply (subst mult.commute)
+          apply (rule word_mult_le_mono1[OF word_of_nat_le])
+            using n_less not_0
+            apply (simp add:unat_of_nat_minus_1)
+           apply (rule p2_gt_0[THEN iffD2])
+           apply (simp add:word_bits_def range_cover_def)
+          apply (simp only: word_bits_def[symmetric])
+          apply (clarsimp simp: unat_of_nat_minus_1[OF n_less(1) not_0])
+          apply (rule nat_less_power_trans2
+            [OF range_cover.range_cover_le_n_less(2),OF cover, folded word_bits_def])
+           apply (simp add:unat_of_nat_m1 less_imp_le)
+          apply (simp add:range_cover_def word_bits_def)
+         apply (rule machine_word_plus_mono_right_split[where sz = sz])
+          using range_cover.range_cover_compare[OF cover,where p = "unat (of_nat n - (1::machine_word))"]
+          apply (clarsimp simp:unat_of_nat_m1)
+         apply (simp add:range_cover_def word_bits_def)
+        apply (rule olen_add_eqv[THEN iffD2])
+        apply (subst add.commute[where a = "2^objBitsKO val - 1"])
+        apply (subst p_assoc_help[symmetric])
+        apply (rule is_aligned_no_overflow)
+        apply (clarsimp simp:range_cover_def word_bits_def)
+        apply (erule aligned_add_aligned[OF _  is_aligned_mult_triv2]; simp)
+       apply simp
+      by (meson assms(1) is_aligned_add is_aligned_mult_triv2 is_aligned_no_overflow' range_cover_def)
+  }
+  with assms show ?thesis
+    unfolding obj_range'_def
+    apply -
+    apply (frule(1) obj_range'_subset)
+    apply (simp add: obj_range'_def)
+    apply (cases "n = 0"; clarsimp simp:new_cap_addrs_def mask_def field_simps)
+    done
+qed
+
+lemma caps_no_overlapD'':
+  "\<lbrakk>cte_wp_at' (\<lambda>cap. cteCap cap = c) q s;caps_no_overlap'' ptr sz s\<rbrakk>
+   \<Longrightarrow> untypedRange c \<inter> {ptr .. (ptr && ~~ mask sz) + 2 ^ sz - 1} \<noteq> {} \<longrightarrow>
+       {ptr .. (ptr && ~~ mask sz) + 2 ^ sz - 1} \<subseteq> untypedRange c"
+  apply (clarsimp simp: cte_wp_at_ctes_of gen_isCap_simps caps_no_overlap''_def
+                  simp del: atLeastAtMost_iff atLeastatMost_subset_iff atLeastLessThan_iff
+                            Int_atLeastAtMost atLeastatMost_empty_iff)
+  apply (drule_tac x = cte in bspec)
+    apply fastforce
+  apply (erule(1) impE)
+  apply blast
+  done
+
+lemma (in Retype_R) valid_untyped'_helper:
+  assumes valid : "valid_cap' c s"
+  and  cte_at : "cte_wp_at' (\<lambda>cap. cteCap cap = c) q s"
+  and  cover  : "range_cover ptr sz (objBitsKO val) n"
+  and  range  : "caps_no_overlap'' ptr sz s"
+  and  pres   : "isUntypedCap c \<longrightarrow> usableUntypedRange c \<inter>  {ptr..ptr + of_nat n * 2 ^ objBitsKO val - 1} = {}"
+  shows "\<lbrakk>pspace_aligned' s; pspace_distinct' s; pspace_no_overlap' ptr sz s\<rbrakk>
+ \<Longrightarrow> valid_cap' c (s\<lparr>ksPSpace := foldr (\<lambda>addr. data_map_insert addr val) (new_cap_addrs n ptr val) (ksPSpace s)\<rparr>)"
+  proof -
+  note blah[simp del] = atLeastAtMost_iff atLeastatMost_subset_iff atLeastLessThan_iff
+        Int_atLeastAtMost atLeastatMost_empty_iff
+  assume pn : "pspace_aligned' s" "pspace_distinct' s"
+  and   no_overlap: "pspace_no_overlap' ptr sz s"
+  show ?thesis
+  using pn pres no_overlap valid cover cte_wp_at_ctes_of[THEN iffD1,OF cte_at]
+        caps_no_overlapD''[OF cte_at range]
+  apply (clarsimp simp:valid_cap'_def retype_ko_wp_at')
+  apply (case_tac "cteCap cte";
+         simp add: valid_cap'_def cte_wp_at_obj_cases' valid_pspace'_def retype_obj_at_disj'
+            split: zombie_type.split_asm)
+   apply (simp add: valid_untyped'_helper_arch_cap)
+  unfolding valid_untyped'_def
+  apply (intro allI)
+  apply (rule ccontr)
+  apply clarify
+  using cover[unfolded range_cover_def]
+  apply (clarsimp simp: gen_isCap_simps retype_ko_wp_at' split:if_split_asm)
+   apply (thin_tac "\<forall>x. Q x" for Q)
+   apply (frule aligned_untypedRange_non_empty)
+    apply (simp add: gen_isCap_simps)
+   apply (elim disjE)
+    apply (frule(1) obj_range'_subset)
+    apply (erule impE)
+     apply (drule(1) psubset_subset_trans)
+     apply (drule Int_absorb1[OF psubset_imp_subset])
+     apply (drule aligned_untypedRange_non_empty)
+      apply (simp add: gen_isCap_simps)
+     apply (simp add:Int_ac add_mask_fold)
+    apply (drule(1) subset_trans)
+    apply (simp only: add_mask_fold)
+   apply (frule(1) obj_range'_subset_strong)
+   apply (drule(1) non_disjoing_subset)
+   apply blast
+  apply (thin_tac "\<forall>x. Q x" for Q)
+  apply (frule aligned_untypedRange_non_empty)
+   apply (simp add: gen_isCap_simps)
+  apply (frule(1) obj_range'_subset)
+  apply (drule(1) subset_trans)
+  apply (erule impE)
+   apply (clarsimp simp: add_mask_fold)
+   apply blast
+  apply (simp only: add_mask_fold)
+  apply blast
+  done
+qed
+
+lemma retype_canonical':
+  assumes pc': "pspace_canonical' s'"
+      and cover: "range_cover ptr sz (objBitsKO ko) n"
+      and sz_limit: "sz \<le> maxUntypedSizeBits"
+      and ptr_cn: "canonical_address (ptr && ~~ mask sz)"
+  shows
+  "pspace_canonical' (s' \<lparr>ksPSpace := foldr (\<lambda>addr. data_map_insert addr ko)
+                                             (new_cap_addrs n ptr ko) (ksPSpace s')\<rparr>)"
+  (is "pspace_canonical' (s'\<lparr>ksPSpace := ?ps\<rparr>)")
+proof -
+  show "pspace_canonical' (s'\<lparr>ksPSpace := ?ps\<rparr>)" using assms
+    apply (subst foldr_upd_app_if[folded data_map_insert_def])
+    apply (clarsimp simp: pspace_canonical'_def split: if_split_asm)
+     apply (clarsimp simp add: new_cap_addrs_def shiftl_t2n)
+     apply (fastforce intro: range_cover_canonical_address[OF cover] simp: mult.commute)+
+    done
+qed
+
+lemma (in Retype_R_2) createObjects_valid_pspace':
+  assumes  mko: "makeObjectKO dev d ty = Some val"
+  and    max_d: "ty = Inr (APIObjectType TCBObject) \<longrightarrow> d \<le> maxDomain"
+  and    not_0: "n \<noteq> 0"
+  and    cover: "range_cover ptr sz (objBitsKO val + gbits) n"
+  and    sz_limit: "sz \<le> maxUntypedSizeBits"
+  and    ptr_cn: "canonical_address (ptr && ~~ mask sz)"
+  and    ptr_km: "ptr && ~~ mask sz \<in> kernel_mappings"
+  shows "\<lbrace>\<lambda>s. pspace_no_overlap' ptr sz s \<and> valid_pspace' s \<and> caps_no_overlap'' ptr sz s
+            \<and> caps_overlap_reserved' {ptr .. ptr + of_nat (n * 2^gbits * 2 ^ objBitsKO val ) - 1} s
+            \<and> ptr \<noteq> 0\<rbrace>
+  createObjects' ptr n val gbits \<lbrace>\<lambda>r. valid_pspace'\<rbrace>"
+  apply (cut_tac not_0)
+  apply (simp add: split_def createObjects'_def
+                   lookupAround2_pspace_no
+                   alignError_def unless_def)
+  apply (rule hoare_pre)
+   apply (wp|simp cong: if_cong del: data_map_insert_def del:fun_upd_apply)+
+   apply (wpc|wp)+
+   apply (subst new_cap_addrs_fold')
+     apply (simp add:unat_1_0 unat_gt_0)
+     apply (rule range_cover_not_zero_shift[OF _  cover])
+     apply simp+
+   apply (subst new_cap_addrs_fold')
+     apply (simp add:unat_1_0 unat_gt_0)
+     apply (rule range_cover_not_zero_shift[OF _  cover])
+     apply simp+
+   apply (subst data_map_insert_def[symmetric])+
+  apply (rule impI)
+  apply (clarsimp simp: new_cap_addrs_fold'
+                        valid_pspace'_def linorder_not_less
+                        objBits_def[symmetric])
+  apply (simp only: imp_disjL[symmetric] imp_conjL[symmetric] imp_ex[symmetric]
+                    range_cover.unat_of_nat_n_shift[OF cover,where gbits=gbits,simplified])
+proof (intro conjI impI)
+
+  fix s
+
+  assume pn: "pspace_no_overlap' ptr sz s"
+     and vo: "valid_objs' s"
+     and ad: "pspace_aligned' s" "pspace_distinct' s"
+     and cn: "pspace_canonical' s"
+     and km: "pspace_in_kernel_mappings' s"
+     and pc: "caps_no_overlap'' ptr sz s"
+    and mdb: "valid_mdb' s"
+    and p_0: "ptr \<noteq> 0"
+    and reserved : "caps_overlap_reserved' {ptr..ptr + of_nat n *2 ^ gbits * 2 ^ objBitsKO val - 1} s"
+    and no_0_obj': "no_0_obj' s"
+  have obj': "objBitsKO val \<le> sz"
+    using cover
+    by (simp add:range_cover_def)
+
+  let ?s' = "s\<lparr>ksPSpace := foldr (\<lambda>addr. data_map_insert addr val) (new_cap_addrs (n * 2 ^ gbits) ptr val) (ksPSpace s)\<rparr>"
+
+  note cover' = range_cover_rel[where sbit' = "objBitsKO val",OF cover _ refl,simplified]
+
+  note ad' = retype_aligned_distinct'[OF ad pn cover']
+
+  note shift = range_cover.unat_of_nat_n_shift[OF cover,where gbits=gbits,simplified]
+
+  have al: "is_aligned ptr (objBitsKO val)"
+    using cover'
+    by (simp add:range_cover_def)
+
+  show pspace_aligned: "pspace_aligned' ?s'"
+    using ad' shift
+    by (simp add:field_simps)
+
+  show pspace_canonical: "pspace_canonical' ?s'"
+    using retype_canonical'[OF cn cover' sz_limit ptr_cn]
+    by (clarsimp simp: field_simps)
+
+  show pspace_in_kernel_mappings: "pspace_in_kernel_mappings' ?s'"
+    using retype_in_kernel_mappings'[OF km cover' sz_limit ptr_km]
+    by (simp add: mult.commute)
+
+  show "pspace_distinct' ?s'"
+    using ad' shift
+    by (simp add: shiftl_t2n' field_simps)
+
+  have obj_atC: "\<And>P x. x \<in> set (new_cap_addrs (2 ^ gbits * n) ptr val) \<Longrightarrow> \<not> obj_at' P x s"
+    apply (clarsimp simp: obj_at'_def)
+    apply (drule subsetD [OF new_cap_addrs_subset [OF cover' ]])
+    apply (insert pspace_no_overlap_disjoint' [OF ad(1) pn])
+    apply (drule domI[where m = "ksPSpace s"])
+    apply (drule(1) orthD2)
+    apply (clarsimp simp:ptr_add_def p_assoc_help)
+    done
+
+  have valid_cap: "\<And>cap q. \<lbrakk> s \<turnstile>' cap; cte_wp_at' (\<lambda>cte. cteCap cte = cap) q s \<rbrakk>
+                      \<Longrightarrow> ?s' \<turnstile>' cap"
+     apply (rule valid_untyped'_helper[OF _ _ _ pc _ ad pn ])
+          apply simp+
+        apply (subst mult.commute)
+        apply (rule cover')
+       using reserved
+     apply (clarsimp simp:caps_overlap_reserved'_def cte_wp_at_ctes_of)
+     apply (drule_tac x = cte in bspec)
+       apply fastforce
+     apply simp
+   done
+
+  show valid_objs: "valid_objs' ?s'" using vo mko max_d ad pn cover pc reserved
+   by (blast intro: createObjects_valid_objs')
+
+  have not_0: "0 \<notin> set (new_cap_addrs (2 ^ gbits * n) ptr val)"
+    using p_0
+    apply clarsimp
+    apply (drule subsetD [OF new_cap_addrs_subset [OF cover'],rotated])
+    apply (clarsimp simp:ptr_add_def)
+    done
+
+  show "valid_mdb' ?s'"
+    apply (simp add: valid_mdb'_def foldr_upd_app_if[folded data_map_insert_def])
+    apply (subst mult.commute)
+    apply (subst ctes_of_retype [OF mko ad])
+        apply (rule ad'[unfolded foldr_upd_app_if[folded data_map_insert_def]])+
+      apply (simp add: objBits_def[symmetric] new_cap_addrs_aligned [OF al])
+     apply (rule ballI, drule subsetD [OF new_cap_addrs_subset [OF cover']])
+     apply (insert pspace_no_overlap_disjoint' [OF ad(1) pn])
+     apply (drule_tac x = x in orthD1)
+       apply (simp add:ptr_add_def p_assoc_help)
+     apply fastforce
+    apply (fold makeObject_cte)
+    apply (rule retype_mdb_valid_n)
+    apply unfold_locales
+      apply (rule mdb[unfolded valid_mdb'_def])
+     apply (rule iffD2 [OF None_ctes_of_cte_at[unfolded cte_wp_at_obj_cases'], THEN sym])
+     apply (rule notI)
+     apply (elim disjE conjE, simp_all add: obj_atC)[1]
+       apply (thin_tac "S \<inter> T = {}" for S T)
+       apply (clarsimp simp: obj_at'_def gen_objBits_simps)
+       apply (drule pspace_no_overlapD' [OF _ pn])
+       apply (drule subsetD [OF new_cap_addrs_subset[OF cover']])
+       apply (frule_tac ptr'=p in mask_in_range)
+       apply (drule(1) tcb_cte_cases_aligned_helpers)
+       apply (drule_tac x = p in orthD1)
+        apply (clarsimp simp: gen_objBits_simps)
+       apply (clarsimp simp:ptr_add_def p_assoc_help)
+      apply (frule new_range_subset[OF cover'])
+      apply (drule bspec [OF new_cap_addrs_aligned[OF al]])
+      apply (drule(1) disjoint_subset[rotated])
+      apply (drule_tac a=p in equals0D)
+      apply (frule_tac ptr'=p in mask_in_range)
+      apply (simp only: add_mask_fold)
+      apply (insert sym [OF mko],
+             clarsimp simp: gen_objBits_simps makeObjectKO_gen_def obj_at'_def)[1]
+     apply (insert sym[OF mko] cover',
+            clarsimp simp: obj_at'_def gen_objBits_simps
+                           makeObjectKO_gen_def)[1]
+     apply (drule(1) tcb_cte_cases_aligned_helpers(2))
+     apply clarsimp
+     apply (drule subsetD [OF new_cap_addrs_subset,rotated])
+       apply (simp add: gen_objBits_simps)
+     apply (drule orthD1)
+       apply (fastforce simp:p_assoc_help ptr_add_def)
+     apply fastforce
+    apply (simp add: not_0)
+    done
+
+  have data_map_ext: "\<And>x y. data_map_insert x y = (\<lambda>m. m (x \<mapsto> y))"
+    by (rule ext) simp
+  show no_0_obj: "no_0_obj' ?s'"
+    using not_0 no_0_obj'
+    by (simp add: no_0_obj'_def data_map_ext field_simps foldr_upd_app_other)
+
+qed
+
+lemma (in Retype_R_2) createObjects_valid_pspace_untyped':
+  assumes  mko: "makeObjectKO dev d ty = Some val"
+  and    max_d: "ty = Inr (APIObjectType TCBObject) \<longrightarrow> d \<le> maxDomain"
+  and    not_0: "n \<noteq> 0"
+  and    cover: "range_cover ptr sz (objBitsKO val + gbits) n"
+  and    sz_limit: "sz \<le> maxUntypedSizeBits"
+  and    ptr_cn: "canonical_address (ptr && ~~ mask sz)"
+  and    ptr_km: "ptr && ~~ mask sz \<in> kernel_mappings"
+  shows "\<lbrace>\<lambda>s. pspace_no_overlap' ptr sz s \<and> valid_pspace' s \<and> caps_no_overlap'' ptr sz s \<and> ptr \<noteq> 0
+            \<and> caps_overlap_reserved' {ptr .. ptr + of_nat (n * 2^gbits * 2 ^ objBitsKO val ) - 1} s \<rbrace>
+  createObjects' ptr n val gbits \<lbrace>\<lambda>r. valid_pspace'\<rbrace>"
+  apply (wp createObjects_valid_pspace' [OF mko max_d not_0 cover sz_limit ptr_cn ptr_km])
+  apply simp
+  done
+
+declare bleeding_obvious [simp]
+
+lemma range_cover_new_cap_addrs_compare:
+  assumes not_0: "n \<noteq> 0"
+  and     cover: "range_cover ptr sz (objBitsKO val + gbits) n"
+  and    ptr_in: "p \<in> set (new_cap_addrs (unat (((of_nat n)::machine_word) << gbits)) ptr val)"
+  shows  "p \<le> ptr + of_nat (shiftL n (objBitsKO val + gbits) - Suc 0)"
+proof -
+  note unat_of_nat_shift = range_cover.unat_of_nat_n_shift[OF cover,where gbits=gbits,simplified]
+  have cover' :"range_cover ptr sz (objBitsKO val) (n*2^gbits)"
+    by (rule range_cover_rel[OF cover],simp+)
+  have upbound:" unat ((((of_nat n)::machine_word) * 2 ^ gbits)) * unat ((2::machine_word) ^ objBitsKO val) < 2 ^ word_bits"
+    using range_cover.range_cover_le_n_less[OF cover' le_refl] cover'
+    apply -
+      apply (drule nat_less_power_trans)
+       apply (simp add:range_cover_def)
+    apply (fold word_bits_def)
+    using unat_of_nat_shift not_0
+    apply (simp add:field_simps shiftl_t2n)
+    done
+  have not_0': "(2::machine_word) ^ (objBitsKO val + gbits) * of_nat n \<noteq> 0"
+    apply (rule range_cover_not_zero_shift[OF not_0,unfolded shiftl_t2n,OF _ le_refl])
+    apply (rule range_cover_rel[OF cover])
+      apply simp+
+    done
+  have "gbits < word_bits"
+    using cover
+    by (simp add:range_cover_def word_bits_def)
+  thus ?thesis
+  apply -
+  apply (insert not_0 cover ptr_in)
+  (* avoid revealing word_bits for the rest of this proof by folding it in every rule that would
+     expose it *)
+  apply (frule range_cover.range_cover_le_n_less[where 'a=machine_word_len, folded word_bits_def,
+                                                 OF _ le_refl])
+  apply (simp add:shiftL_nat )
+  apply (simp add:range_cover.unat_of_nat_n_shift)
+  apply (clarsimp simp:new_cap_addrs_def shiftl_t2n)
+  apply (rename_tac pa)
+  apply (rule word_plus_mono_right)
+    apply (rule order_trans)
+    apply (subst mult.commute)
+    apply (rule word_mult_le_iff[where 'a=machine_word_len, folded word_bits_def, THEN iffD2])
+       apply (clarsimp simp:p2_gt_0 range_cover_def)
+      apply (drule range_cover_rel[where sbit' = "0"])
+        apply (simp+)[2]
+      apply (erule less_le_trans[OF range_cover.range_cover_le_n_less(2)])
+       apply (clarsimp simp:field_simps power_add)
+       apply (rule unat_le_helper)
+       apply (rule of_nat_mono_maybe_le[THEN iffD1])
+         using range_cover.range_cover_le_n_less[OF cover' le_refl]
+       apply (simp_all only:word_bits_def[symmetric])
+      apply simp
+     apply (drule nat_less_power_trans)
+      apply (simp add: range_cover_def[where 'a=machine_word_len, folded word_bits_def])
+     apply (rule less_le_trans[OF mult_less_mono1])
+       apply (rule unat_mono)
+       apply (rule_tac y1= "pa" in of_nat_mono_maybe'[where 'a=machine_word_len, folded word_bits_def,
+                                                      THEN iffD1,rotated -1];
+              simp)
+       apply simp
+      apply simp
+        using unat_of_nat_shift
+      apply (simp add:field_simps shiftl_t2n)
+     apply simp
+    apply (rule word_less_sub_1)
+    apply (simp add:power_add field_simps)
+    apply (subst mult.assoc[symmetric])
+    apply (rule word_mult_less_mono1[where 'a=machine_word_len, folded word_bits_def])
+      apply (rule word_of_nat_less)
+      using unat_of_nat_shift
+      apply (simp add:shiftl_t2n field_simps)
+     apply (meson less_exp objBitsKO_less_word_bits word_gt_a_gt_0
+                   of_nat_power[where 'a=machine_word_len, folded word_bits_def])
+   using upbound
+   apply (simp add:word_bits_def)
+   apply (rule machine_word_plus_mono_right_split[where sz = sz])
+    apply (rule less_le_trans[rotated -1])
+     apply (rule range_cover.range_cover_compare_bound[OF cover'])
+    apply (simp add: unat_minus_one[OF not_0'])
+    using range_cover.unat_of_nat_n_shift[OF cover le_refl]
+    apply (simp add:shiftl_t2n power_add field_simps)
+  apply (simp add: range_cover_def[where 'a=machine_word_len, folded word_bits_def])
+  done
+qed
+
+lemma createObjects_orig_ko_wp_at2':
+  "\<lbrace>\<lambda>s. range_cover ptr sz (objBitsKO val + gbits) n \<and> n \<noteq> 0
+      \<and> pspace_aligned' s \<and> pspace_distinct' s
+      \<and> P (ko_wp_at' P' p s)
+      \<and> (P' val \<longrightarrow> P True)
+      \<and> pspace_no_overlap' ptr sz s\<rbrace>
+  createObjects' ptr n val gbits \<lbrace>\<lambda>r s. P (ko_wp_at' P' p s)\<rbrace>"
+   apply (simp add: createObjects'_def lookupAround2_pspace_no
+                    alignError_def unless_def split_def del:fun_upd_apply)
+   apply (rule hoare_grab_asm)+
+   apply (subst new_cap_addrs_fold')
+     apply (drule range_cover_not_zero_shift[rotated])
+     apply (rule le_add2)
+     apply (simp add:word_le_sub1 del:fun_upd_apply)+
+   apply (rule hoare_pre)
+    apply (wp|simp cong: if_cong del: data_map_insert_def fun_upd_apply)+
+   apply (wpc|wp)+
+   apply (clarsimp simp:valid_pspace'_def linorder_not_less simp del:fun_upd_apply)
+   apply (subgoal_tac " range_cover ptr sz (objBitsKO val) (unat (of_nat n << gbits))")
+    apply (subst data_map_insert_def[symmetric])+
+    apply (subst retype_ko_wp_at',simp+)+
+    apply clarsimp
+   apply (cases "P' val")
+    apply simp
+   apply clarsimp
+   apply (frule(1) subsetD [OF new_cap_addrs_subset])
+   apply (drule(1) pspace_no_overlap_disjoint')
+   apply (simp add:lookupAround2_None1)
+   apply (intro conjI impI allI)
+     apply (drule_tac x = p in spec)
+     apply (erule impE)
+      apply (erule(1) range_cover_new_cap_addrs_compare[rotated])
+      apply simp
+     apply (fastforce simp: ko_wp_at'_def)
+   apply (drule_tac x = p in orthD1)
+   apply (clarsimp simp:ptr_add_def p_assoc_help)
+   apply (simp add:dom_def)
+   apply (fastforce simp:ko_wp_at'_def)
+  apply (rule range_cover_rel)
+     apply (simp)+
+  apply (subst mult.commute)
+  apply (erule range_cover.unat_of_nat_n_shift)
+  apply simp
+  done
+
+lemma createObjects_orig_obj_at2':
+  "\<lbrace>\<lambda>s. n \<noteq> 0
+      \<and> range_cover ptr sz (objBitsKO val + gbits) n
+      \<and> pspace_aligned' s \<and> pspace_distinct' s
+      \<and> P (obj_at' P' p s)
+      \<and> \<not> (case_option False P' (projectKO_opt val))
+      \<and> pspace_no_overlap' ptr sz s\<rbrace>
+  createObjects' ptr n val gbits \<lbrace>\<lambda>r s. P (obj_at' P' p s)\<rbrace>"
+  unfolding obj_at'_real_def
+  by (wp createObjects_orig_ko_wp_at2') auto
+
+lemma createObjects_orig_cte_wp_at2':
+  "\<lbrace>\<lambda>s. P (cte_wp_at' P' p s)
+      \<and> n \<noteq> 0
+      \<and> range_cover ptr sz (objBitsKO val + gbits) n
+      \<and> pspace_aligned' s \<and> pspace_distinct' s
+      \<and> \<not> (case_option False P' (projectKO_opt val))
+      \<and> (\<forall>(getF, setF) \<in> ran tcb_cte_cases.
+              \<not> (case_option False (P' \<circ> getF) (projectKO_opt val)))
+      \<and> pspace_no_overlap' ptr sz s\<rbrace>
+  createObjects' ptr n val gbits \<lbrace>\<lambda>r s. P (cte_wp_at' P' p s)\<rbrace>"
+  including classic_wp_pre
+  apply (simp add: cte_wp_at'_obj_at')
+  apply (rule handy_prop_divs)
+   apply (wp createObjects_orig_obj_at2'[where sz = sz], simp)
+  apply (simp add: tcb_cte_cases_def tcb_cte_cases_neqs)
+  apply (wp handy_prop_divs createObjects_orig_obj_at2'[where sz = sz]
+             | simp add: o_def cong: option.case_cong)+
+  done
+
+lemmas threadSet_cte_wp_at2' =
+  threadSet_cte_wp_at'T[OF all_tcbI, OF ball_tcb_cte_casesI]
+
+crunch doMachineOp
+  for ko_wp_at'[wp]: "\<lambda>s. P (ko_wp_at' P' p s)"
+
+lemma createObjects_orig_obj_at':
+  "\<lbrace>\<lambda>s. n \<noteq> 0
+      \<and> range_cover ptr sz (objBitsKO val + gbits) n
+      \<and> pspace_aligned' s \<and> pspace_distinct' s
+      \<and> obj_at' P p s
+      \<and> pspace_no_overlap' ptr sz s\<rbrace>
+   createObjects' ptr n val gbits \<lbrace>\<lambda>r. obj_at' P p\<rbrace>"
+  apply (rule hoare_grab_asm)+
+  apply (clarsimp simp: createObjects'_def)
+  apply (subst new_cap_addrs_fold')
+   apply (simp add:unat_1_0 unat_gt_0)
+   apply (rule range_cover_not_zero_shift)
+     apply simp+
+  apply (wp|simp add:split_def cong: if_cong del: data_map_insert_def fun_upd_apply)+
+     apply (wpc|wp)+
+   apply (clarsimp simp del:fun_upd_apply)
+   apply (simp add:range_cover_def is_aligned_mask)
+  apply (subst data_map_insert_def[symmetric])+
+  apply clarsimp
+  apply (subgoal_tac "range_cover ptr sz (objBitsKO val) (unat (of_nat n << gbits))")
+   apply (subst retype_obj_at',simp+)+
+   apply (intro conjI impI allI)
+      apply (clarsimp simp:obj_at'_real_def ko_wp_at'_def)
+      apply (frule(1) subsetD [OF new_cap_addrs_subset])
+      apply (drule(1) pspace_no_overlap_disjoint')
+      apply (simp add:lookupAround2_None1)
+      apply (drule_tac x = p in spec)
+      apply (erule impE)
+       apply (erule(1) range_cover_new_cap_addrs_compare[rotated])
+       apply simp
+      apply simp
+     apply (frule(1) subsetD [OF new_cap_addrs_subset])
+     apply (drule(1) pspace_no_overlap_disjoint')
+     apply (drule_tac x = p in orthD1)
+      apply (clarsimp simp:ptr_add_def p_assoc_help)
+     apply (simp add:dom_def obj_at'_real_def ko_wp_at'_def)
+    apply simp+
+  apply (rule range_cover_rel)
+    apply (simp)+
+  apply (subst mult.commute)
+  apply (erule range_cover.unat_of_nat_n_shift)
+  apply simp
+  done
+
+lemma createObjects_orig_cte_wp_at':
+  "\<lbrace>\<lambda>s. range_cover ptr sz (objBitsKO val + gbits) n \<and> n \<noteq> 0
+      \<and> pspace_aligned' s \<and> pspace_distinct' s
+      \<and> cte_wp_at' P p s
+      \<and> pspace_no_overlap' ptr sz s\<rbrace>
+  createObjects' ptr n val gbits \<lbrace>\<lambda>r s. cte_wp_at' P p s\<rbrace>"
+  apply (simp add: cte_wp_at'_obj_at' tcb_cte_cases_def tcb_cte_cases_neqs)
+  apply (rule hoare_pre, wp hoare_vcg_disj_lift createObjects_orig_obj_at'[where sz = sz])
+  apply clarsimp
+  done
+
+lemma (in Retype_R_2) createNewCaps_cte_wp_at:
+  assumes cover: "range_cover ptr sz (APIType_capBits ty us) n"
+  and not_0 : "n \<noteq> 0"
+  shows "\<lbrace>\<lambda>s. cte_wp_at' P p s \<and> valid_pspace' s \<and> pspace_no_overlap' ptr sz s\<rbrace>
+  createNewCaps ty ptr n us dev
+  \<lbrace>\<lambda>_. cte_wp_at' P p\<rbrace>"
+  apply (wp createNewCaps_cte_wp_at')
+  apply (auto simp: cover not_0)
+  done
+
+lemma createObjects_obj_at_other:
+  assumes cover: "range_cover ptr sz (objBitsKO val + gbits) n"
+  and     not_0: "n\<noteq> 0"
+  shows  "\<lbrace>\<lambda>s. obj_at' P p s \<and> valid_pspace' s \<and> pspace_no_overlap' ptr sz s\<rbrace>
+  createObjects ptr n val gbits \<lbrace>\<lambda>_. obj_at' P p\<rbrace>"
+  apply (simp add: createObjects_def)
+  apply (wp createObjects_orig_obj_at'[where sz = sz])
+  using cover not_0
+  apply (clarsimp simp: cover not_0 valid_pspace'_def pspace_no_overlap'_def)
+  done
+
+lemma (in Retype_R) valid_cap'_range_no_overlap:
+  "\<lbrakk>untypedRange c \<inter> {ptr..(ptr && ~~ mask sz) + 2 ^ sz - 1} = {}; s \<turnstile>' c;
+    valid_pspace' s; pspace_no_overlap' ptr sz s;
+    range_cover ptr sz (objBitsKO val) n\<rbrakk>
+   \<Longrightarrow> s\<lparr>ksPSpace := foldr (\<lambda>addr. data_map_insert addr val)
+                           (new_cap_addrs n ptr val) (ksPSpace s)\<rparr> \<turnstile>' c"
+  apply (cases c; simp add: valid_cap'_def cte_wp_at_obj_cases' valid_pspace'_def
+                            retype_obj_at_disj'
+                       split: zombie_type.split_asm if_splits
+                       del: Int_atLeastAtMost)[1]
+  apply (clarsimp simp add: valid_untyped'_helper_arch_cap)
+  apply (rename_tac word nat1 nat2)
+  apply (clarsimp simp:valid_untyped'_def retype_ko_wp_at'
+        simp del: atLeastAtMost_iff atLeastatMost_subset_iff atLeastLessThan_iff
+        Int_atLeastAtMost atLeastatMost_empty_iff)
+  apply (frule aligned_untypedRange_non_empty)
+   apply (simp add: gen_isCap_simps)
+  apply (intro conjI impI)
+   apply (intro allI)
+   apply (drule_tac x = ptr' in spec)
+   apply (rule ccontr)
+   apply (clarsimp simp del: atLeastAtMost_iff atLeastatMost_subset_iff atLeastLessThan_iff
+                             Int_atLeastAtMost atLeastatMost_empty_iff)
+   apply (erule disjE)
+    apply (drule(2) disjoint_subset2 [OF obj_range'_subset])
+    apply (drule(1) disjoint_subset2[OF psubset_imp_subset])
+    apply (simp add: Int_absorb ptr_add_def p_assoc_help mask_def
+                del: atLeastAtMost_iff atLeastatMost_subset_iff atLeastLessThan_iff
+                     Int_atLeastAtMost atLeastatMost_empty_iff)
+   apply (drule(1) obj_range'_subset)
+   apply (drule_tac A'=" {word + of_nat nat2..word + 2 ^ nat1 - 1}" in disjoint_subset[rotated])
+    apply clarsimp
+    apply (rule is_aligned_no_wrap')
+     apply (fastforce simp: capAligned_def)
+    apply (erule of_nat_power[where 'a=machine_word_len, folded word_bits_def])
+    apply (simp add:capAligned_def)
+   apply (drule(1) disjoint_subset2)
+   apply (simp add: add_mask_fold)
+   apply blast
+  apply (intro allI)
+  apply (drule_tac x = ptr' in spec)
+  apply (rule ccontr)
+  apply (clarsimp simp del: atLeastAtMost_iff atLeastatMost_subset_iff atLeastLessThan_iff
+                            Int_atLeastAtMost atLeastatMost_empty_iff)
+  apply (drule(2) disjoint_subset2 [OF obj_range'_subset])
+  apply (drule(1) disjoint_subset2)
+  apply (simp add: Int_absorb ptr_add_def p_assoc_help mask_def
+              del: atLeastAtMost_iff atLeastatMost_subset_iff atLeastLessThan_iff
+                   Int_atLeastAtMost atLeastatMost_empty_iff)
+  done
+
+lemma (in Retype_R) createObjects_valid_cap':
+  "\<lbrace>valid_cap' c and valid_pspace' and pspace_no_overlap' ptr sz and
+    K (untypedRange c \<inter> {ptr .. (ptr && ~~ mask sz) + 2^sz - 1} = {} \<and>
+      range_cover ptr sz (objBitsKO val + gbits) n \<and> n \<noteq> 0)\<rbrace>
+  createObjects' ptr n val gbits
+  \<lbrace>\<lambda>_. valid_cap' c\<rbrace>"
+  apply (rule hoare_gen_asm)
+  apply (simp add: createObjects'_def lookupAround2_pspace_no
+                    alignError_def unless_def split_def)
+  apply (subst new_cap_addrs_fold')
+   apply (simp add:unat_1_0 unat_gt_0)
+   apply (rule range_cover_not_zero_shift)
+     apply fastforce+
+  apply (rule hoare_pre)
+   apply (wp|simp cong: if_cong del: data_map_insert_def fun_upd_apply)+
+     apply (clarsimp simp: linorder_not_less valid_pspace'_def)
+  apply (wpc|wp)+
+  apply (subst data_map_insert_def[symmetric])+
+  apply clarsimp
+  apply (subgoal_tac " range_cover ptr sz (objBitsKO val) (unat (of_nat n << gbits))")
+   apply (subst range_cover.unat_of_nat_n_shift,simp+)+
+   apply (subst (asm) range_cover.unat_of_nat_n_shift,simp+)+
+   apply (intro conjI impI allI)
+    apply (erule(4) valid_cap'_range_no_overlap)+
+  apply (rule range_cover_rel)
+    apply (simp)+
+  apply (subst mult.commute)
+  apply (erule range_cover.unat_of_nat_n_shift)
+  apply simp
+  done
+
+lemma createObjects_cte_wp_at':
+  "\<lbrakk>range_cover ptr sz (objBitsKO val + gbits) n; n \<noteq> 0\<rbrakk>
+  \<Longrightarrow>\<lbrace>\<lambda>s. cte_wp_at' P p s \<and> valid_pspace' s \<and> pspace_no_overlap' ptr sz s\<rbrace>
+  createObjects' ptr n val gbits
+  \<lbrace>\<lambda>_. cte_wp_at' P p\<rbrace>"
+  apply (clarsimp simp: valid_def cte_wp_at_obj_cases')
+  apply (erule disjE)
+   apply (erule use_valid[OF _ ])
+    apply (rule createObjects_orig_obj_at')
+   apply fastforce
+  apply clarsimp
+  apply (drule_tac x = na in bspec)
+   apply clarsimp
+  apply clarsimp
+  apply (drule use_valid[OF _ createObjects_orig_obj_at'])
+   apply fastforce
+  apply simp
+  done
+
+lemma createObjects_ret2:
+  "\<lbrace>(\<lambda>s. P (map (\<lambda>p. ptr_add y (p * 2 ^ (objBitsKO ko + gbits)))
+                    [0..<n]))
+        and K (n < 2 ^ word_bits \<and> n \<noteq> 0)\<rbrace>
+      createObjects y n ko gbits \<lbrace>\<lambda>rv s. P rv\<rbrace>"
+  apply (rule hoare_gen_asm)
+  apply (rule hoare_chain)
+    apply (rule hoare_vcg_conj_lift)
+     apply (rule createObjects_ret)
+      apply simp+
+    apply (rule hoare_vcg_prop)
+   defer
+   apply (clarsimp simp: power_add mult.commute mult.left_commute | assumption)+
+  done
+
+lemma state_refs_ko_wp_at_eq:
+  "state_refs_of' s = (\<lambda>x. {r. ko_wp_at' (\<lambda>ko. r \<in> refs_of' ko) x s})"
+  apply (rule ext)
+  apply (simp add: state_refs_of'_def ko_wp_at'_def
+            split: option.split)
+  done
+
+lemma state_hyp_refs_ko_wp_at_eq:
+  "state_hyp_refs_of' s = (\<lambda>x. {r. ko_wp_at' (\<lambda>ko. r \<in> hyp_refs_of' ko) x s})"
+  apply (rule ext)
+  apply (simp add: state_hyp_refs_of'_def ko_wp_at'_def
+            split: option.split)
+  done
+
+lemma createObjects_state_refs_of'':
+  "\<lbrace>\<lambda>s. n \<noteq> 0
+        \<and> range_cover ptr sz (objBitsKO val + gbits) n
+        \<and> P (state_refs_of' s) \<and> refs_of' val = {}
+        \<and> pspace_aligned' s \<and> pspace_distinct' s
+        \<and> pspace_no_overlap' ptr sz s\<rbrace>
+     createObjects' ptr n val gbits
+   \<lbrace>\<lambda>rv s. P (state_refs_of' s)\<rbrace>"
+   apply (clarsimp simp:valid_def lookupAround2_pspace_no state_refs_ko_wp_at_eq)
+   apply (erule ssubst[where P = P,rotated])
+   apply (rule ext)
+   apply (rule set_eqI)
+   apply clarsimp
+   apply (intro iffI,rule ccontr)
+     apply (drule_tac P1="\<lambda>x. \<not> x" in use_valid[OF _ createObjects_orig_ko_wp_at2'[where sz = sz]])
+     apply simp
+     apply (intro conjI)
+     apply simp+
+   apply (drule_tac P1="\<lambda>x. x" in use_valid[OF _ createObjects_orig_ko_wp_at2'[where sz = sz]])
+     apply simp+
+  done
+
+lemma createObjects_state_hyp_refs_of'':
+  "\<lbrace>\<lambda>s. n \<noteq> 0
+        \<and> range_cover ptr sz (objBitsKO val + gbits) n
+        \<and> P (state_hyp_refs_of' s) \<and> hyp_refs_of' val = {}
+        \<and> pspace_aligned' s \<and> pspace_distinct' s
+        \<and> pspace_no_overlap' ptr sz s\<rbrace>
+     createObjects' ptr n val gbits
+   \<lbrace>\<lambda>rv s. P (state_hyp_refs_of' s)\<rbrace>"
+   apply (clarsimp simp:valid_def lookupAround2_pspace_no state_hyp_refs_ko_wp_at_eq)
+   apply (erule ssubst[where P = P,rotated])
+   apply (rule ext)
+   apply (rule set_eqI)
+   apply clarsimp
+   apply (intro iffI,rule ccontr)
+     apply (drule_tac P1="\<lambda>x. \<not> x" in use_valid[OF _ createObjects_orig_ko_wp_at2'[where sz = sz]])
+     apply simp
+     apply (intro conjI)
+     apply simp+
+   apply (drule_tac P1="\<lambda>x. x" in use_valid[OF _ createObjects_orig_ko_wp_at2'[where sz = sz]])
+     apply simp+
+  done
+
+lemma createObjects_iflive':
+  "\<lbrace>\<lambda>s. if_live_then_nonz_cap' s \<and> \<not> live' val
+        \<and> n \<noteq> 0
+        \<and> range_cover ptr sz (objBitsKO val + gbits) n
+        \<and> pspace_aligned' s \<and> pspace_distinct' s
+        \<and> pspace_no_overlap' ptr sz s\<rbrace>
+     createObjects' ptr n val gbits
+   \<lbrace>\<lambda>rv s. if_live_then_nonz_cap' s\<rbrace>"
+  apply (rule hoare_pre)
+   apply (simp only: if_live_then_nonz_cap'_def
+                     ex_nonz_cap_to'_def imp_conv_disj)
+   apply (wp hoare_vcg_all_lift hoare_vcg_disj_lift
+             hoare_vcg_ex_lift createObjects_orig_ko_wp_at2'
+             createObjects_orig_cte_wp_at')
+  apply clarsimp
+  apply (intro conjI allI impI)
+  apply simp_all
+  apply (rule ccontr)
+  apply clarsimp
+  apply (drule(1) if_live_then_nonz_capE')
+  apply (fastforce simp: ex_nonz_cap_to'_def)
+  done
+
+lemma createObjects_pspace_only:
+  "\<lbrakk> \<And>f s. P (ksPSpace_update f s) = P s \<rbrakk>
+   \<Longrightarrow> \<lbrace>P\<rbrace> createObjects' ptr n val gbits \<lbrace>\<lambda>rv. P\<rbrace>"
+  apply (simp add: createObjects_def createObjects'_def unless_def alignError_def
+                   split_def lookupAround2_pspace_no)
+  apply wpsimp
+  done
+
+lemma sch_act_wf_lift_asm:
+  assumes tcb: "\<And>P t. \<lbrace>st_tcb_at' P t and Q \<rbrace> f \<lbrace>\<lambda>rv. st_tcb_at' P t\<rbrace>"
+  assumes tcbDomain: "\<And>P t. \<lbrace>obj_at' (\<lambda>tcb. P (tcbDomain tcb)) t and Q\<rbrace> f \<lbrace>\<lambda>rv. obj_at' (\<lambda>tcb. P (tcbDomain tcb)) t\<rbrace>"
+  assumes kCT: "\<And>P. \<lbrace>\<lambda>s. P (ksCurThread s)\<rbrace> f \<lbrace>\<lambda>_ s. P (ksCurThread s)\<rbrace>"
+  assumes kCD: "\<And>P. \<lbrace>\<lambda>s. P (ksCurDomain s)\<rbrace> f \<lbrace>\<lambda>_ s. P (ksCurDomain s)\<rbrace>"
+  assumes ksA: "\<And>P. \<lbrace>\<lambda>s. P (ksSchedulerAction s)\<rbrace> f \<lbrace>\<lambda>_ s. P (ksSchedulerAction s)\<rbrace>"
+  shows
+  "\<lbrace>\<lambda>s. sch_act_wf (ksSchedulerAction s) s \<and> Q s\<rbrace>
+  f
+  \<lbrace>\<lambda>rv s. sch_act_wf (ksSchedulerAction s) s\<rbrace>"
+  apply (clarsimp simp: valid_def)
+  apply (rule use_valid [OF _ ksA], assumption)
+  apply (frule use_valid[OF _ kCT[of "(=) (ksCurThread s)" for s] refl])
+  apply (frule use_valid[OF _ kCD[of "(=) (ksCurDomain s)" for s] refl])
+  apply (case_tac "ksSchedulerAction s")
+    apply (simp add: ct_in_state'_def)
+    apply (drule use_valid [OF _ tcb])
+     apply simp
+    apply simp
+   apply simp
+  apply (clarsimp simp: tcb_in_cur_domain'_def)
+  apply (frule use_valid [OF _ tcb], fastforce)
+  apply (frule use_valid [OF _ tcbDomain], fastforce)
+  apply auto
+  done
+
+lemma threadSet_ko_wp_at2':
+  "\<lbrace>\<lambda>s. P (ko_wp_at' P' p s) \<and> (\<forall>tcb_x :: tcb. P' (injectKO (F tcb_x)) = P' (injectKO tcb_x))\<rbrace>
+     threadSet F ptr
+   \<lbrace>\<lambda>_ s. P (ko_wp_at' P' p s)\<rbrace>"
+  apply (simp add: threadSet_def split del: if_split)
+  apply (wp setObject_ko_wp_at getObject_tcb_wp | simp add: gen_objBits_simps)+
+  apply (auto simp: ko_wp_at'_def obj_at'_def)
+  done
+
+lemma threadSet_ko_wp_at2'_futz:
+  "\<lbrace>\<lambda>s. P (ko_wp_at' P' p s) \<and> obj_at' Q ptr s
+         \<and> (\<forall>tcb_x :: tcb. Q tcb_x \<longrightarrow> P' (injectKO (F tcb_x)) = P' (injectKO tcb_x))\<rbrace>
+     threadSet F ptr
+   \<lbrace>\<lambda>_ s. P (ko_wp_at' P' p s)\<rbrace>"
+  apply (simp add: threadSet_def split del: if_split)
+  apply (wp setObject_ko_wp_at getObject_tcb_wp | simp add: gen_objBits_simps)+
+  apply (auto simp: ko_wp_at'_def obj_at'_def)
+  done
+
+lemma mapM_x_threadSet_createNewCaps_futz:
+  "\<lbrace>\<lambda>s. P (ko_wp_at' P' p s) \<and> (\<forall>addr\<in>set addrs. obj_at' (\<lambda>tcb. \<not>tcbQueued tcb \<and> tcbState tcb = Inactive) addr s)
+         \<and> (\<forall>tcb_x :: tcb. tcbQueued (F tcb_x) = tcbQueued tcb_x \<and> tcbState (F tcb_x) = tcbState tcb_x)
+         \<and> (\<forall>tcb_x :: tcb. \<not> tcbQueued tcb_x \<and> tcbState tcb_x = Inactive \<longrightarrow> P' (injectKO (F tcb_x)) = P' (injectKO tcb_x))\<rbrace>
+     mapM_x (threadSet F) addrs
+   \<lbrace>\<lambda>_ s. P (ko_wp_at' P' p s)\<rbrace>" (is "\<lbrace>?PRE\<rbrace> _ \<lbrace>\<lambda>_. ?POST\<rbrace>")
+  apply (rule mapM_x_inv_wp[where P="?PRE"])
+    apply simp
+   apply (rule hoare_pre)
+    apply (wp hoare_vcg_ball_lift threadSet_ko_wp_at2'[where P="id", simplified]
+        | wp (once) threadSet_ko_wp_at2'_futz[where Q="\<lambda>tcb. \<not>tcbQueued tcb \<and> tcbState tcb = Inactive"]
+        | simp)+
+  done
+
+lemma createObjects_makeObject_not_tcbQueued:
+  assumes "range_cover ptr sz (objBitsKO tcb) n"
+  assumes "n \<noteq> 0" "tcb = injectKO (makeObject::tcb)"
+  shows "\<lbrace>\<lambda>s. pspace_no_overlap' ptr sz s \<and> pspace_aligned' s \<and> pspace_distinct' s\<rbrace>
+           createObjects ptr n tcb 0
+         \<lbrace>\<lambda>rv s. \<forall>addr\<in>set rv. obj_at' (\<lambda>tcb. \<not> tcbQueued tcb \<and> tcbState tcb = Structures_H.thread_state.Inactive) addr s\<rbrace>"
+  apply (rule hoare_strengthen_post[OF createObjects_ko_at_strg[where 'a=tcb]])
+  using assms
+  apply (auto simp: obj_at'_def projectKO_opt_tcb objBitsKO_def objBits_def makeObject_tcb)
+  done
+
+lemma createObjects_ko_wp_at2:
+  "\<lbrace>\<lambda>s. range_cover ptr sz (objBitsKO ko + gbits) n \<and> n \<noteq> 0
+      \<and> pspace_aligned' s \<and> pspace_distinct' s
+      \<and> P (ko_wp_at' P' p s)
+      \<and> (P' ko \<longrightarrow> P True)
+      \<and> pspace_no_overlap' ptr sz s\<rbrace>
+    createObjects ptr n ko gbits
+   \<lbrace>\<lambda>_ s. P (ko_wp_at' P' p s)\<rbrace>"
+  apply (simp add: createObjects_def)
+  apply (wp createObjects_orig_ko_wp_at2')
+  apply auto
+  done
+
+context Retype_R begin
+
+lemmas createNewCaps_ko_wp_at'
+    = createNewCaps_ko_wp_atQ'[simplified, unfolded fold_K]
+
+lemmas createNewCaps_obj_at2 =
+   createNewCaps_ko_wp_at'
+      [where P'="\<lambda>ko. \<exists>obj :: ('b :: pspace_storable).
+                   projectKO_opt ko = Some obj \<and> P' obj" for P',
+       folded obj_at'_real_def,
+       unfolded pred_conj_def, simplified]
+
+lemma createNewCaps_obj_at':
+  "\<lbrace>\<lambda>s. obj_at' (P :: ('b :: pspace_storable) \<Rightarrow> bool) p s
+       \<and> range_cover ptr sz (APIType_capBits ty us) n \<and> n \<noteq> 0
+       \<and> pspace_aligned' s \<and> pspace_distinct' s
+       \<and> pspace_no_overlap' ptr sz s
+       \<and> createNewCaps_arch_ko_type_pre(koType(TYPE('b)))
+       \<and> (\<forall>tcb d. \<not>tcbQueued tcb \<and> tcbState tcb = Inactive \<longrightarrow>
+            ((\<exists>obj :: 'b. injectKOS obj = KOTCB (tcb\<lparr>tcbDomain := d\<rparr>) \<and> P obj) \<longleftrightarrow>
+             (\<exists>obj :: 'b. injectKOS obj = KOTCB tcb \<and> P obj)))\<rbrace>
+     createNewCaps ty ptr n us d
+   \<lbrace>\<lambda>rv s. obj_at' P p s\<rbrace>"
+  apply (simp add: obj_at'_real_def)
+  apply (wp createNewCaps_ko_wp_at')
+  apply clarsimp
+  apply (intro conjI impI)
+     apply simp+
+   apply (fastforce dest!: createNewCaps_arch_ko_type_preD)
+  apply (clarsimp simp: project_inject)+
+  done
+
+lemmas createNewCaps_pred_tcb_at'
+     = createNewCaps_obj_at'[
+         where P="\<lambda>ko. (Q :: 'a :: type \<Rightarrow> bool) (proj (tcb_to_itcb' ko))" for Q proj,
+         folded pred_tcb_at'_def, simplified]
+
+lemma createNewCaps_cur:
+  "\<lbrakk>range_cover ptr sz (APIType_capBits ty us) n ; n \<noteq> 0\<rbrakk> \<Longrightarrow>
+   \<lbrace>\<lambda>s. valid_pspace' s \<and>
+        pspace_no_overlap' ptr sz s \<and>
+        cur_tcb' s\<rbrace>
+      createNewCaps ty ptr n us d
+   \<lbrace>\<lambda>rv. cur_tcb'\<rbrace>"
+  apply (rule hoare_post_imp[where Q'="\<lambda>rv s. \<exists>t. ksCurThread s = t \<and> tcb_at' t s"])
+   apply (simp add: cur_tcb'_def)
+  apply (wp hoare_vcg_ex_lift createNewCaps_obj_at'[where 'b=tcb])
+  apply (auto simp: cur_tcb'_def createNewCaps_arch_ko_type_pre_non_arch)
+  done
+
+lemma createNewCaps_ifunsafe':
+  "\<lbrace>\<lambda>s. valid_pspace' s \<and>
+        pspace_no_overlap' ptr sz s \<and>
+        range_cover ptr sz (APIType_capBits ty us) n \<and> n \<noteq> 0 \<and>
+        if_unsafe_then_cap' s\<rbrace>
+      createNewCaps ty ptr n us d
+   \<lbrace>\<lambda>rv s. if_unsafe_then_cap' s\<rbrace>"
+  apply (simp only: if_unsafe_then_cap'_def ex_cte_cap_to'_def
+                    imp_conv_disj)
+  apply (rule hoare_pre)
+   apply (rule hoare_use_eq_irq_node'[OF createNewCaps_ksInterrupt])
+   apply (wp hoare_vcg_all_lift hoare_vcg_disj_lift createNewCaps_cte_wp_at2 hoare_vcg_ex_lift)
+  apply (simp add: makeObject_cte pspace_no_overlap'_def
+                   valid_pspace'_def)
+  apply auto
+  done
+
+lemma createObjects_idle':
+  "\<lbrace>valid_idle' and valid_pspace' and pspace_no_overlap' ptr sz
+        and (\<lambda>s. \<not> case_option False (\<lambda>cte. ksIdleThread s \<in> capRange (cteCap cte))
+                        (projectKO_opt val)
+               \<and> (\<forall>(getF, setF) \<in> ran tcb_cte_cases.
+                 \<not> case_option False (\<lambda>tcb. ksIdleThread s \<in> capRange (cteCap (getF tcb)))
+                        (projectKO_opt val)))
+        and K (range_cover ptr sz (objBitsKO val + gbits) n  \<and> n \<noteq> 0)\<rbrace>
+   createObjects' ptr n val gbits
+   \<lbrace>\<lambda>rv. valid_idle'\<rbrace>"
+  apply (rule hoare_gen_asm)
+  apply (rule hoare_pre)
+   apply (clarsimp simp add: valid_idle'_def pred_tcb_at'_def)
+   apply (rule hoare_vcg_conj_lift)
+   apply (rule hoare_as_subst[OF createObjects'_it])
+   apply (wp createObjects_orig_obj_at'
+             createObjects_orig_cte_wp_at2'
+             hoare_vcg_all_lift | simp)+
+  apply (clarsimp simp: valid_idle'_def o_def pred_tcb_at'_def valid_pspace'_def
+                  cong: option.case_cong)
+  apply auto
+  done
+
+end (* Retype_R *)
+
+
+lemma koTypeOf_eq_UserDataT:
+  "(koTypeOf ko = UserDataT) = (ko = KOUserData)"
+  by (cases ko, simp_all)
+
+lemma valid_irq_handlers_cte_wp_at_form':
+  "valid_irq_handlers' = (\<lambda>s. \<forall>irq. irq_issued' irq s \<or>
+                               (\<forall>p. \<not> cte_wp_at' (\<lambda>cte. cteCap cte = IRQHandlerCap irq) p s))"
+  by (auto simp: valid_irq_handlers'_def cteCaps_of_def cte_wp_at_ctes_of
+                 fun_eq_iff ran_def)
+
+lemma (in Retype_R) createNewCaps_irq_handlers':
+  "\<lbrace>valid_irq_handlers' and pspace_no_overlap' ptr sz
+       and pspace_aligned' and pspace_distinct'
+       and K (range_cover ptr sz (APIType_capBits ty us) n \<and> n \<noteq> 0)\<rbrace>
+     createNewCaps ty ptr n us d
+   \<lbrace>\<lambda>rv. valid_irq_handlers'\<rbrace>"
+  apply (simp add: valid_irq_handlers_cte_wp_at_form' irq_issued'_def)
+   apply (wp hoare_vcg_all_lift hoare_vcg_disj_lift
+             createNewCaps_cte_wp_at2)
+  apply (clarsimp simp: makeObject_cte)
+  apply auto
+  done
+
+lemma createObjects'_irq_states' [wp]:
+  "\<lbrace>valid_irq_states'\<rbrace> createObjects' a b c d \<lbrace>\<lambda>_. valid_irq_states'\<rbrace>"
+  apply (simp add: createObjects'_def split_def)
+  apply (wp unless_wp|wpc|simp add: alignError_def)+
+  apply fastforce
+  done
+
+lemma createObjects_irq_states'[wp]:
+  "createObjects a b c d \<lbrace>valid_irq_states'\<rbrace>"
+  unfolding createObjects_def
+  by wpsimp
+
+crunch createObjects
+  for ksMachine[wp]: "\<lambda>s. P (ksMachineState s)"
+  (simp: crunch_simps unless_def)
+
+lemma createObjects_valid_bitmaps:
+  "createObjects' ptr n val gbits \<lbrace>valid_bitmaps\<rbrace>"
+  apply (clarsimp simp: createObjects'_def alignError_def split_def)
+  apply (wp case_option_wp[where P="\<lambda>_. P" and P'=P for P, simplified] assert_inv
+         | clarsimp simp del: fun_upd_apply)+
+  apply (clarsimp simp: valid_bitmaps_def valid_bitmapQ_def bitmapQ_def bitmapQ_no_L2_orphans_def
+                        bitmapQ_no_L1_orphans_def)
+  done
+
+lemma valid_bitmaps_gsCNodes_update[simp]:
+  "valid_bitmaps (gsCNodes_update f s) = valid_bitmaps s"
+  by (simp add: valid_bitmaps_def bitmapQ_defs)
+
+lemma valid_bitmaps_gsUserPages_update[simp]:
+  "valid_bitmaps (gsUserPages_update f s) = valid_bitmaps s"
+  by (simp add: valid_bitmaps_def bitmapQ_defs)
+
+crunch curDomain
+  for valid_bitmaps[wp]: valid_bitmaps
+  and sched_pointers[wp]: "\<lambda>s. P (tcbSchedNexts_of s) (tcbSchedPrevs_of s)"
+  and valid_sched_pointers[wp]: valid_sched_pointers
+
+lemma (in Retype_R) createObjects_sched_queues:
+  "\<lbrace>\<lambda>s. n \<noteq> 0
+        \<and> range_cover ptr sz (objBitsKO val + gbits) n
+        \<and> P (tcbSchedNexts_of s) (tcbSchedPrevs_of s)
+        \<and> (case val of KOTCB tcb \<Rightarrow> tcbSchedNext tcb = None \<and> tcbSchedPrev tcb = None
+                     | _ \<Rightarrow> True)
+        \<and> pspace_aligned' s \<and> pspace_distinct' s
+        \<and> pspace_no_overlap' ptr sz s\<rbrace>
+   createObjects' ptr n val gbits
+   \<lbrace>\<lambda>_ s. P (tcbSchedNexts_of s) (tcbSchedPrevs_of s)\<rbrace>"
+  (is "\<lbrace> \<lambda>s. _ \<and> _ \<and> ?Pre s \<rbrace> _ \<lbrace>\<lambda>_. _\<rbrace>")
+proof (rule hoare_grab_asm)+
+  assume not_0: "\<not> n = 0"
+    and cover: "range_cover ptr sz ((objBitsKO val) + gbits) n"
+  then show
+    "\<lbrace>\<lambda>s. ?Pre s\<rbrace> createObjects' ptr n val gbits \<lbrace>\<lambda>_ s. P (tcbSchedNexts_of s) (tcbSchedPrevs_of s)\<rbrace>"
+  proof -
+    have shiftr_not_zero:" 1 \<le> ((of_nat n)::machine_word) << gbits"
+      using range_cover_not_zero_shift[OF not_0 cover,where gbits = gbits]
+      by (simp add:word_le_sub1)
+    show ?thesis
+      apply (clarsimp simp: createObjects'_def unless_def alignError_def split_def)
+      apply (wp | clarsimp simp del: fun_upd_apply)+
+      apply (clarsimp simp: shiftL_nat data_map_insert_def[symmetric]
+                            new_cap_addrs_fold'[OF shiftr_not_zero]
+                  simp del: data_map_insert_def)
+      using range_cover.unat_of_nat_n_shift[OF cover, where gbits=gbits, simplified]
+      apply (clarsimp simp: foldr_upd_app_if)
+      apply (rule_tac a="tcbSchedNexts_of s" and b="tcbSchedPrevs_of s"
+                   in rsubst2[rotated, OF sym sym, where P=P])
+        apply (rule ext)
+        apply (clarsimp simp: opt_map_def)
+        apply (frule (2) retype_ksPSpace_None[simplified mult.commute])
+          apply (fastforce intro: cover)
+         apply assumption
+        apply (clarsimp split: kernel_object.splits option.splits)
+       apply (rule ext)
+       apply (clarsimp simp: opt_map_def)
+       apply (frule (2) retype_ksPSpace_None[simplified mult.commute])
+         apply (fastforce intro: cover)
+        apply fastforce
+       apply (clarsimp split: kernel_object.splits option.splits)
+      apply simp
+      done
+  qed
+qed
+
+lemma createObjects_valid_sched_pointers:
+  "\<lbrace>\<lambda>s. valid_sched_pointers s
+        \<and> (case val of KOTCB tcb \<Rightarrow> tcbSchedNext tcb = None \<and> tcbSchedPrev tcb = None
+                     | _ \<Rightarrow> True)\<rbrace>
+   createObjects' ptr n val gbits
+   \<lbrace>\<lambda>_. valid_sched_pointers\<rbrace>"
+  apply (clarsimp simp: createObjects'_def unless_def alignError_def split_def)
+  apply (wp case_option_wp[where P="\<lambda>_. P" and P'=P for P, simplified] assert_inv
+         | clarsimp simp del: fun_upd_apply)+
+  apply (clarsimp simp: valid_sched_pointers_def foldr_upd_app_if opt_pred_def opt_map_def comp_def)
+  apply (cases "tcb_of' val"; clarsimp)
+  done
+
+lemma mapM_x_threadSet_valid_pspace:
+  "\<lbrace>valid_pspace' and K (curdom \<le> maxDomain)\<rbrace>
+      mapM_x (threadSet (tcbDomain_update (\<lambda>_. curdom))) addrs \<lbrace>\<lambda>y. valid_pspace'\<rbrace>"
+  apply (rule hoare_gen_asm)
+  apply (wp mapM_x_wp' threadSet_valid_pspace')
+             apply simp_all
+  done
+
+lemma doMachineOp_return_foo:
+  "doMachineOp (do x\<leftarrow>a;return () od) = (do (doMachineOp a); return () od)"
+  apply (clarsimp simp: doMachineOp_def bind_def gets_def
+                        get_def return_def select_f_def split_def simpler_modify_def)
+  apply (rule ext)+
+  apply simp
+  apply (rule set_eqI)
+  apply clarsimp
+  done
+
+lemma createObjects_pspace_domain_valid':
+  "\<lbrace>\<lambda>s. range_cover ptr sz (objBitsKO val + gbits) n \<and> n \<noteq> 0
+      \<and> {ptr .. (ptr && ~~ mask sz) + 2 ^ sz - 1} \<inter> kernel_data_refs = {}
+      \<and> pspace_domain_valid s\<rbrace>
+       createObjects' ptr n val gbits
+   \<lbrace>\<lambda>_. pspace_domain_valid\<rbrace>"
+  apply (simp add: createObjects'_def split_def unless_def)
+  apply (rule hoare_pre)
+   apply (wp | wpc | simp only: alignError_def haskell_assert_def)+
+  apply (clarsimp simp: new_cap_addrs_fold' unat_1_0 unat_gt_0
+                        range_cover_not_zero_shift
+                        caps_overlap_reserved'_def)
+  apply (simp add: pspace_domain_valid_def foldr_upd_app_if
+                   fun_upd_def[symmetric])
+  apply (subgoal_tac " \<forall>x \<in> set (new_cap_addrs (unat (of_nat n << gbits)) ptr val).
+                         mask_range x (objBitsKO val) \<subseteq> {ptr .. (ptr && ~~ mask sz) + 2 ^ sz - 1}")
+   apply blast
+
+  apply (rule ballI)
+  apply (rule new_range_subset)
+   apply (erule range_cover_rel, simp+)
+  apply (simp add: range_cover.unat_of_nat_n_shift field_simps)
+  done
+
+lemma createObjects_pspace_domain_valid:
+  "\<lbrace>\<lambda>s. range_cover ptr sz (objBitsKO val + gbits) n \<and> n \<noteq> 0
+      \<and> {ptr .. (ptr && ~~ mask sz) + 2 ^ sz - 1} \<inter> kernel_data_refs = {}
+      \<and> pspace_domain_valid s\<rbrace>
+       createObjects ptr n val gbits
+   \<lbrace>\<lambda>_. pspace_domain_valid\<rbrace>"
+  apply (simp add: createObjects_def)
+  apply (wp createObjects_pspace_domain_valid'[where sz=sz])
+  apply (simp add: objBits_def)
+  done
+
+crunch doMachineOp
+  for pspace_domain_valid[wp]: pspace_domain_valid
+
+(* FIXME: move *)
+lemma ct_idle_or_in_cur_domain'_lift_futz:
+  assumes a: "\<And>P. \<lbrace>\<lambda>s. P (ksCurDomain s)\<rbrace>       f \<lbrace>\<lambda>_ s. P (ksCurDomain s)\<rbrace>"
+  assumes b: "\<And>P. \<lbrace>\<lambda>s. P (ksSchedulerAction s)\<rbrace> f \<lbrace>\<lambda>_ s. P (ksSchedulerAction s)\<rbrace>"
+  assumes c: "\<And>P. \<lbrace>\<lambda>s. P (ksIdleThread s)\<rbrace>      f \<lbrace>\<lambda>_ s. P (ksIdleThread s)\<rbrace>"
+  assumes d: "\<And>P. \<lbrace>\<lambda>s. P (ksCurThread s)\<rbrace>       f \<lbrace>\<lambda>_ s. P (ksCurThread s)\<rbrace>"
+  assumes e: "\<And>d t. \<lbrace>\<lambda>s. obj_at' (\<lambda>tcb. tcbState tcb \<noteq> Inactive \<and> d = tcbDomain tcb) t s \<and> Q s\<rbrace>
+                            f
+                     \<lbrace>\<lambda>_. obj_at' (\<lambda>tcb. tcbState tcb \<noteq> Inactive \<and> d = tcbDomain tcb) t\<rbrace>"
+  shows "\<lbrace>ct_idle_or_in_cur_domain' and ct_active' and Q\<rbrace> f \<lbrace>\<lambda>_. ct_idle_or_in_cur_domain'\<rbrace>"
+proof -
+  from e have e':
+    "\<And>d t. \<lbrace>\<lambda>s. obj_at' (\<lambda>tcb. tcbState tcb \<noteq> Inactive \<and> d = tcbDomain tcb) t s \<and> Q s\<rbrace>
+              f
+            \<lbrace>\<lambda>_. obj_at' (\<lambda>tcb. d = tcbDomain tcb) t\<rbrace>"
+    apply (rule hoare_strengthen_post)
+    apply (auto simp: obj_at'_def)
+    done
+  show ?thesis
+    apply (simp add: ct_idle_or_in_cur_domain'_def tcb_in_cur_domain'_def)
+    apply (rule hoare_pre)
+    apply (wps a b c d)
+    apply (wp hoare_weak_lift_imp e' hoare_vcg_disj_lift)
+    apply (auto simp: obj_at'_def ct_in_state'_def st_tcb_at'_def)
+    done
+qed
+
+lemma (in Retype_R) createNewCaps_ct_idle_or_in_cur_domain':
+  "\<lbrace>ct_idle_or_in_cur_domain' and pspace_aligned' and pspace_distinct' and pspace_no_overlap' ptr sz and ct_active' and K (range_cover ptr sz (APIType_capBits ty us) n \<and> 0 < n) \<rbrace>
+    createNewCaps ty ptr n us dev
+   \<lbrace>\<lambda>rv. ct_idle_or_in_cur_domain'\<rbrace>"
+  apply (wp ct_idle_or_in_cur_domain'_lift_futz createNewCaps_obj_at'[where sz=sz]
+         | simp add: createNewCaps_arch_ko_type_pre_non_arch)+
+  done
+
+lemma sch_act_wf_lift_asm_futz:
+  assumes tcb: "\<And>P t. \<lbrace>st_tcb_at' P t and Q \<rbrace> f \<lbrace>\<lambda>rv. st_tcb_at' P t\<rbrace>"
+  assumes tcbDomain: "\<And>P t. \<lbrace>obj_at' (\<lambda>tcb. runnable' (tcbState tcb) \<longrightarrow> P (tcbDomain tcb)) t and Q\<rbrace> f \<lbrace>\<lambda>rv. obj_at' (\<lambda>tcb. runnable' (tcbState tcb) \<longrightarrow> P (tcbDomain tcb)) t\<rbrace>"
+  assumes kCT: "\<And>P. \<lbrace>\<lambda>s. P (ksCurThread s)\<rbrace> f \<lbrace>\<lambda>_ s. P (ksCurThread s)\<rbrace>"
+  assumes kCD: "\<And>P. \<lbrace>\<lambda>s. P (ksCurDomain s)\<rbrace> f \<lbrace>\<lambda>_ s. P (ksCurDomain s)\<rbrace>"
+  assumes ksA: "\<And>P. \<lbrace>\<lambda>s. P (ksSchedulerAction s)\<rbrace> f \<lbrace>\<lambda>_ s. P (ksSchedulerAction s)\<rbrace>"
+  shows
+  "\<lbrace>\<lambda>s. sch_act_wf (ksSchedulerAction s) s \<and> Q s\<rbrace>
+  f
+  \<lbrace>\<lambda>rv s. sch_act_wf (ksSchedulerAction s) s\<rbrace>"
+  apply (clarsimp simp: valid_def)
+  apply (rule use_valid [OF _ ksA], assumption)
+  apply (frule use_valid [OF _ kCT[of "(=) (ksCurThread s)" for s] refl])
+  apply (frule use_valid [OF _ kCD[of "(=) (ksCurDomain s)" for s] refl])
+  apply (case_tac "ksSchedulerAction s")
+    apply (simp add: ct_in_state'_def)
+    apply (drule use_valid [OF _ tcb])
+     apply simp
+    apply simp
+   apply simp
+  apply (clarsimp simp: tcb_in_cur_domain'_def)
+  apply (frule use_valid [OF _ tcb], fastforce)
+  apply simp
+  apply (rename_tac word)
+  apply (subgoal_tac "(obj_at' (\<lambda>tcb. runnable' (tcbState tcb) \<longrightarrow> ksCurDomain b = tcbDomain tcb) word and Q) s")
+   apply (drule use_valid [OF _ tcbDomain], fastforce)
+    apply (auto simp: st_tcb_at'_def o_def obj_at'_def ko_wp_at'_def)
+  done
+
+lemma (in Retype_R) createNewCaps_sch_act_wf:
+  "\<lbrace>(\<lambda>s. sch_act_wf (ksSchedulerAction s) s) and pspace_aligned' and pspace_distinct' and pspace_no_overlap' ptr sz and K (range_cover ptr sz (APIType_capBits ty us) n \<and> 0 < n)\<rbrace>
+     createNewCaps ty ptr n us dev
+   \<lbrace>\<lambda>_ s. sch_act_wf (ksSchedulerAction s) s\<rbrace>"
+  apply (wp sch_act_wf_lift_asm_futz
+            createNewCaps_pred_tcb_at'[where sz=sz]
+            createNewCaps_obj_at'[where sz=sz]
+       | simp add: createNewCaps_arch_ko_type_pre_non_arch)+
+  done
+
+lemma (in Retype_R) createObjects_null_filter':
+  "\<lbrace>\<lambda>s. P (null_filter' (ctes_of s)) \<and> makeObjectKO dev d ty = Some val \<and>
+        range_cover ptr sz (objBitsKO val + gbits) n \<and> n \<noteq> 0 \<and>
+        pspace_aligned' s \<and> pspace_distinct' s \<and> pspace_no_overlap' ptr sz s\<rbrace>
+   createObjects' ptr n val gbits
+   \<lbrace>\<lambda>addrs a. P (null_filter' (ctes_of a))\<rbrace>"
+   apply (clarsimp simp: createObjects'_def split_def)
+   apply (wp unless_wp|wpc
+          | clarsimp simp: alignError_def split del: if_split simp del:fun_upd_apply)+
+   apply (subst new_cap_addrs_fold')
+     apply (simp add:unat_1_0 unat_gt_0)
+     apply (rule range_cover_not_zero_shift)
+     apply fastforce+
+   apply (subst new_cap_addrs_fold')
+    apply (simp add:unat_1_0 unat_gt_0)
+    apply (rule range_cover_not_zero_shift)
+      apply simp
+     apply assumption
+    apply simp
+   apply (subst data_map_insert_def[symmetric])+
+   apply (frule(2) retype_aligned_distinct'[where ko = val])
+    apply (erule range_cover_rel)
+     apply simp+
+   apply (frule(2) retype_aligned_distinct'(2)[where ko = val])
+    apply (erule range_cover_rel)
+     apply simp+
+   apply (frule null_filter_ctes_retype
+     [where addrs = "(new_cap_addrs (unat (((of_nat n)::machine_word) << gbits)) ptr val)"])
+          apply assumption+
+     apply (clarsimp simp:field_simps foldr_upd_app_if[folded data_map_insert_def] shiftl_t2n range_cover.unat_of_nat_shift)+
+    apply (rule new_cap_addrs_aligned[THEN bspec])
+    apply (erule range_cover.aligned[OF range_cover_rel])
+     apply simp+
+   apply (clarsimp simp:shiftl_t2n field_simps range_cover.unat_of_nat_shift)
+   apply (drule subsetD[OF new_cap_addrs_subset,rotated])
+    apply (erule range_cover_rel)
+     apply simp
+    apply simp
+   apply (rule ccontr)
+   apply clarify
+   apply (frule(1) pspace_no_overlapD')
+   apply (erule_tac B = "{x..x+2^objBitsKO y - 1}" in in_empty_interE[rotated])
+    apply (drule(1) pspace_alignedD')
+    apply (clarsimp)
+    apply (erule is_aligned_no_overflow)
+    apply (simp del:atLeastAtMost_iff atLeastatMost_subset_iff atLeastLessThan_iff
+        Int_atLeastAtMost atLeastatMost_empty_iff add:Int_ac ptr_add_def p_assoc_help)
+  apply (simp add:field_simps foldr_upd_app_if[folded data_map_insert_def] shiftl_t2n)
+  apply auto
+  done
+
+lemma untyped_ranges_zero_inv_null_filter:
+  "untyped_ranges_zero_inv (option_map cteCap o null_filter' ctes)
+    = untyped_ranges_zero_inv (option_map cteCap o ctes)"
+  apply (simp add: untyped_ranges_zero_inv_def fun_eq_iff null_filter'_def)
+  apply clarsimp
+  apply (rule_tac f="\<lambda>caps. x = ran caps" for caps in arg_cong)
+  apply (clarsimp simp: fun_eq_iff map_comp_def untypedZeroRange_def)
+  done
+
+lemma untyped_ranges_zero_inv_null_filter_cteCaps_of:
+  "untyped_ranges_zero_inv (cteCaps_of s)
+    = untyped_ranges_zero_inv (option_map cteCap o null_filter' (ctes_of s))"
+  by (simp add: untyped_ranges_zero_inv_null_filter cteCaps_of_def)
+
+lemma (in Retype_R_2) createNewCaps_urz:
+  "\<lbrace>untyped_ranges_zero'
+      and pspace_aligned' and pspace_distinct' and pspace_no_overlap' ptr sz
+      and K (range_cover ptr sz (APIType_capBits ty us) n \<and> n \<noteq> 0) \<rbrace>
+   createNewCaps ty ptr n us dev
+   \<lbrace>\<lambda>archCaps. untyped_ranges_zero'\<rbrace>"
+  apply (simp add: untyped_ranges_zero_inv_null_filter_cteCaps_of)
+  apply (rule hoare_pre)
+   apply (rule untyped_ranges_zero_lift)
+    apply (wp createNewCaps_null_filter')+
+  apply (auto simp: o_def)
+  done
+
+locale Retype_R_3 = Retype_R_2 +
+  assumes createNewCaps_valid_pspace[wp]:
+    "\<And>n ptr sz ty us dev.
+     \<lbrakk>n \<noteq> 0; range_cover ptr sz (APIType_capBits ty us) n; sz \<le> maxUntypedSizeBits;
+      canonical_address (ptr && ~~ mask sz); ptr && ~~ mask sz \<in> kernel_mappings\<rbrakk> \<Longrightarrow>
+     \<lbrace>\<lambda>s. pspace_no_overlap' ptr sz s \<and> valid_pspace' s \<and> caps_no_overlap'' ptr sz s \<and> ptr \<noteq> 0 \<and>
+          caps_overlap_reserved' {ptr..ptr + word_of_nat n * 2 ^ APIType_capBits ty us - 1} s \<and>
+          ksCurDomain s \<le> maxDomain\<rbrace>
+     createNewCaps ty ptr n us dev
+     \<lbrace>\<lambda>r. valid_pspace'\<rbrace>"
+begin
+
+lemma createNewCaps_invs':
+  "\<lbrace>(\<lambda>s. invs' s \<and> ct_active' s \<and> pspace_no_overlap' ptr sz s
+        \<and> caps_no_overlap'' ptr sz s \<and> ptr \<noteq> 0
+        \<and> {ptr .. (ptr && ~~ mask sz) + 2 ^ sz - 1} \<inter> kernel_data_refs = {}
+        \<and> caps_overlap_reserved' {ptr..ptr + of_nat n * 2^(APIType_capBits ty us) - 1} s
+        \<and> (ty = APIObjectType ArchTypes_H.CapTableObject \<longrightarrow> us > 0)
+        \<and> gsMaxObjectSize s > 0)
+       and K (range_cover ptr sz (APIType_capBits ty us) n \<and> n \<noteq> 0
+              \<and> sz \<le> maxUntypedSizeBits \<and> canonical_address (ptr && ~~ mask sz)
+              \<and> ptr && ~~ mask sz \<in> kernel_mappings)\<rbrace>
+     createNewCaps ty ptr n us dev
+   \<lbrace>\<lambda>rv. invs'\<rbrace>"
+  (is "\<lbrace>?P and K ?Q\<rbrace> ?f \<lbrace>\<lambda>rv. invs'\<rbrace>")
+proof (rule hoare_gen_asm, elim conjE)
+  assume cover: "range_cover ptr sz (APIType_capBits ty us) n"
+     and not_0: "n \<noteq> 0"
+     and sz_limit: "sz \<le> maxUntypedSizeBits"
+     and ptr_cn: "canonical_address (ptr && ~~ mask sz)"
+     and  ptr_km: "ptr && ~~ mask sz \<in> kernel_mappings"
+  have cnc_ct_not_inQ:
+    "\<lbrace>ct_not_inQ and valid_pspace' and pspace_no_overlap' ptr sz\<rbrace>
+     createNewCaps ty ptr n us dev \<lbrace>\<lambda>_. ct_not_inQ\<rbrace>"
+    unfolding ct_not_inQ_def
+    apply (rule_tac P'="\<lambda>s. ksSchedulerAction s = ResumeCurrentThread
+                             \<longrightarrow> (obj_at' (Not \<circ> tcbQueued) (ksCurThread s) s
+                                  \<and> valid_pspace' s \<and> pspace_no_overlap' ptr sz s)"
+                    in hoare_pre_imp, clarsimp)
+    apply (rule hoare_convert_imp[OF createNewCaps_nosch])
+    apply (rule hoare_weaken_pre)
+     apply (wps createNewCaps_ct)
+     apply (wp createNewCaps_obj_at')
+    using cover not_0
+    apply (fastforce simp: valid_pspace'_def createNewCaps_arch_ko_type_pre_non_arch)
+    done
+  show "\<lbrace>?P\<rbrace>
+     createNewCaps ty ptr n us dev
+   \<lbrace>\<lambda>rv. invs'\<rbrace>"
+  apply (simp add: invs'_def valid_state'_def
+                   pointerInUserData_def typ_at'_def)
+    apply (rule hoare_pre)
+   supply createNewCaps_valid_pspace[wp]
+   apply (wp createNewCaps_valid_pspace[OF not_0 cover sz_limit ptr_cn ptr_km]
+               createNewCaps_state_refs_of'[OF cover not_0]
+               createNewCaps_state_hyp_refs_of'[OF cover not_0]
+               createNewCaps_iflive'[OF cover not_0]
+               irqs_masked_lift
+               createNewCaps_ifunsafe'
+               createNewCaps_cur[OF cover not_0]
+               createNewCaps_global_refs'
+               createNewCaps_valid_arch_state
+               valid_irq_node_lift_asm[unfolded pred_conj_def, OF _ createNewCaps_obj_at']
+               createNewCaps_irq_handlers' createNewCaps_vms
+               createNewCaps_pred_tcb_at' cnc_ct_not_inQ
+               createNewCaps_ct_idle_or_in_cur_domain'
+               createNewCaps_sch_act_wf
+               createNewCaps_urz[where sz=sz]
+               createNewCaps_sched_queues[OF cover not_0]
+               createNewCaps_valid_sched_pointers
+               createNewCaps_valid_bitmaps
+           | simp)+
+  using not_0
+  apply (clarsimp simp: valid_pspace'_def createNewCaps_arch_ko_type_pre_non_arch)
+  using cover
+  apply (intro conjI)
+   apply simp_all
+  done
+qed
+
+end (* Retype_R_3 *)
+
+lemma createObjects_obj_ranges':
+  "\<lbrace>\<lambda>s. (\<forall>x ko. ksPSpace s x = Some ko \<longrightarrow> (obj_range' x ko) \<inter> S = {}) \<and>
+        pspace_no_overlap' ptr sz s \<and>
+        pspace_aligned' s \<and> pspace_distinct' s \<and>
+        S \<inter> {ptr..(ptr &&~~ mask sz) + 2^sz - 1} = {} \<and>
+        range_cover ptr sz (objBitsKO val + gbits) n \<and> n \<noteq> 0\<rbrace>
+  createObjects' ptr n val gbits
+  \<lbrace>\<lambda>r s. (\<forall>x ko. ksPSpace s x = Some ko \<longrightarrow> (obj_range' x ko) \<inter> S = {})\<rbrace>"
+  apply (simp add: createObjects'_def lookupAround2_pspace_no
+                   alignError_def unless_def split_def del: fun_upd_apply)
+  apply (rule hoare_pre)
+   apply (wp|simp cong: if_cong del: data_map_insert_def fun_upd_apply)+
+  apply (subst new_cap_addrs_fold')
+   apply (simp add: unat_1_0 unat_gt_0)
+   apply (rule range_cover_not_zero_shift)
+     apply fastforce+
+  apply (clarsimp simp: foldr_fun_upd_value)
+  apply (subgoal_tac "range_cover ptr sz (objBitsKO val) (unat (of_nat n << gbits))")
+   apply (erule(1) disjoint_subset[OF obj_range'_subset])
+   apply (simp add: Int_commute)
+  apply (rule range_cover_rel)
+    apply (simp)+
+  apply (subst mult.commute)
+  apply (erule range_cover.unat_of_nat_n_shift)
+  apply simp
+  done
+
+lemma createObjects_pred_tcb_at':
+  "\<lbrace>pred_tcb_at' proj P t and K (range_cover ptr sz (objBitsKO val + gbits) n \<and> n \<noteq> 0)
+     and pspace_aligned' and pspace_distinct' and pspace_no_overlap' ptr sz\<rbrace>
+  createObjects ptr n val gbits \<lbrace>\<lambda>rv. pred_tcb_at' proj P t\<rbrace>"
+  apply (simp add: pred_tcb_at'_def createObjects_def)
+  apply (wp createObjects_orig_obj_at')
+  apply auto
+  done
+
+lemma (in Retype_R) createObjects_ex_cte_cap_to [wp]:
+  "\<lbrace>\<lambda>s. range_cover ptr sz (objBitsKO val + gbits) n \<and> n \<noteq> 0 \<and> pspace_aligned' s \<and>
+        pspace_distinct' s \<and> ex_cte_cap_to' p s \<and> pspace_no_overlap' ptr sz s\<rbrace>
+  createObjects ptr n val gbits \<lbrace>\<lambda>r. ex_cte_cap_to' p\<rbrace>"
+  apply (simp add: ex_cte_cap_to'_def createObjects_def)
+  apply (rule hoare_lift_Pf2 [where f="irq_node'"])
+   apply (wp hoare_vcg_ex_lift createObjects_orig_cte_wp_at'[where sz = sz])
+   apply simp
+  apply wp
+  done
+
+lemma createObjects_orig_obj_at3:
+  "\<lbrace>\<lambda>s. obj_at' P p s \<and> range_cover ptr sz (objBitsKO val + gbits) n \<and> n \<noteq> 0 \<and>
+        pspace_aligned' s \<and>
+        pspace_distinct' s \<and> pspace_no_overlap' ptr sz s\<rbrace>
+  createObjects ptr n val gbits \<lbrace>\<lambda>r. obj_at' P p\<rbrace>"
+  by (wp createObjects_orig_obj_at'[where sz = sz] | simp add: createObjects_def)+
+
+context Retype_R begin
+
+lemma createObjects_sch:
+  "\<lbrace>(\<lambda>s. sch_act_wf (ksSchedulerAction s) s) and pspace_aligned' and pspace_distinct' and pspace_no_overlap' ptr sz
+      and K (range_cover ptr sz (objBitsKO val + gbits) n \<and> n \<noteq> 0)\<rbrace>
+  createObjects ptr n val gbits
+  \<lbrace>\<lambda>rv s. sch_act_wf (ksSchedulerAction s) s\<rbrace>"
+  by (rule hoare_gen_asm)
+     (wp sch_act_wf_lift_asm createObjects_pred_tcb_at' createObjects_orig_obj_at3 | force)+
+
+lemma createObjects_no_cte_ifunsafe':
+  assumes no_cte: "\<And>c. projectKO_opt val \<noteq> Some (c::cte)"
+  assumes no_tcb: "\<And>t. projectKO_opt val \<noteq> Some (t::tcb)"
+  shows
+  "\<lbrace>\<lambda>s. valid_pspace' s \<and>
+       pspace_no_overlap' ptr sz s \<and>
+       range_cover ptr sz (objBitsKO val + gbits) n \<and> n \<noteq> 0 \<and>
+       if_unsafe_then_cap' s\<rbrace>
+      createObjects ptr n val gbits
+   \<lbrace>\<lambda>rv s. if_unsafe_then_cap' s\<rbrace>"
+  apply (simp only: if_unsafe_then_cap'_def ex_cte_cap_to'_def
+                    imp_conv_disj)
+  apply (rule hoare_pre)
+   apply (rule hoare_use_eq_irq_node'[OF createObjects_ksInterrupt])
+   apply (simp add: createObjects_def)
+   apply (wp hoare_vcg_all_lift hoare_vcg_disj_lift hoare_vcg_imp_lift
+             createObjects_orig_cte_wp_at2' hoare_vcg_ex_lift)
+  apply (simp add: valid_pspace'_def disj_imp)
+  using no_cte no_tcb
+  apply fastforce
+  done
+
+end (* Retype_R *)
+
+lemma createObjects'_typ_at:
+  "\<lbrace>\<lambda>s. n \<noteq> 0 \<and>
+        range_cover ptr sz (objBitsKO val + gbits) n \<and>
+        typ_at' T p s \<and>
+        pspace_aligned' s \<and> pspace_distinct' s \<and>
+        pspace_no_overlap' ptr sz s\<rbrace>
+  createObjects' ptr n val gbits \<lbrace>\<lambda>r s. typ_at' T p s\<rbrace>"
+  apply (rule hoare_grab_asm)+
+  apply (simp add: createObjects'_def lookupAround2_pspace_no
+                    alignError_def unless_def split_def typ_at'_def)
+  apply (subst new_cap_addrs_fold')
+   apply (simp add: unat_1_0 unat_gt_0)
+   apply (rule range_cover_not_zero_shift)
+     apply simp+
+  apply (wp|wpc|simp cong: if_cong del: data_map_insert_def fun_upd_apply)+
+  apply (subst data_map_insert_def[symmetric])
+  apply clarsimp
+  apply (subgoal_tac "range_cover ptr sz (objBitsKO val) (unat (of_nat n << gbits))")
+   apply (subst data_map_insert_def[symmetric])+
+   apply (subst retype_ko_wp_at',simp+)+
+   apply clarsimp
+   apply (frule(1) subsetD [OF new_cap_addrs_subset])
+   apply (drule(1) pspace_no_overlap_disjoint')
+   apply (simp add: lookupAround2_None1)
+   apply (intro conjI impI allI)
+    apply (drule_tac x = p in spec)
+    apply (erule impE)
+     apply (erule(1) range_cover_new_cap_addrs_compare[rotated])
+     apply simp
+    apply (fastforce simp: ko_wp_at'_def)
+   apply (drule_tac x = p in orthD1)
+    apply (clarsimp simp: ptr_add_def p_assoc_help)
+   apply (simp add: dom_def)
+   apply (fastforce simp: ko_wp_at'_def)
+  apply (rule range_cover_rel)
+    apply (simp)+
+  apply (subst mult.commute)
+  apply (erule range_cover.unat_of_nat_n_shift)
+  apply simp
+  done
+
+context Retype_R begin
+
+lemma createObjects_irq_state:
+  "\<lbrace>\<lambda>s. pspace_aligned' s \<and> pspace_distinct' s \<and>
+        pspace_no_overlap' ptr sz s \<and>
+        range_cover ptr sz (objBitsKO val + gbits) n \<and> n \<noteq> 0 \<and>
+        valid_irq_node' (irq_node' s) s\<rbrace>
+      createObjects ptr n val gbits
+   \<lbrace>\<lambda>rv s. valid_irq_node' (irq_node' s) s\<rbrace>"
+  apply (wp valid_irq_node_lift_asm [unfolded pred_conj_def, OF _ createObjects_orig_obj_at3])
+  apply auto
+  done
+
+lemma createObjects_no_cte_irq_handlers:
+  assumes no_cte: "\<And>c. projectKO_opt val \<noteq> Some (c::cte)"
+  assumes no_tcb: "\<And>t. projectKO_opt val \<noteq> Some (t::tcb)"
+  shows
+  "\<lbrace>\<lambda>s. pspace_aligned' s \<and> pspace_distinct' s \<and>
+        pspace_no_overlap' ptr sz s \<and>
+        range_cover ptr sz (objBitsKO val + gbits) n \<and> n \<noteq> 0 \<and>
+        valid_irq_handlers' s\<rbrace>
+      createObjects ptr n val gbits
+   \<lbrace>\<lambda>rv s.  valid_irq_handlers' s\<rbrace>"
+  apply (simp add: valid_irq_handlers_cte_wp_at_form' createObjects_def irq_issued'_def)
+   apply (wp hoare_vcg_all_lift hoare_vcg_disj_lift
+             createObjects_orig_cte_wp_at2')
+  using no_cte no_tcb by (auto simp: split_def split: option.splits)
+
+lemma createObjects_cur':
+  "\<lbrace>\<lambda>s. pspace_aligned' s \<and> pspace_distinct' s \<and>
+        pspace_no_overlap' ptr sz s \<and> range_cover ptr sz (objBitsKO val + gbits) n \<and> n \<noteq> 0 \<and>
+        cur_tcb' s\<rbrace>
+      createObjects ptr n val gbits
+   \<lbrace>\<lambda>rv s. cur_tcb' s\<rbrace>"
+  apply (rule hoare_post_imp[where Q'="\<lambda>rv s. \<exists>t. ksCurThread s = t \<and> tcb_at' t s"])
+   apply (simp add: cur_tcb'_def)
+  apply (wp hoare_vcg_ex_lift createObjects_orig_obj_at3)
+  apply (clarsimp simp: cur_tcb'_def)
+  apply auto
+  done
+
+end (* Retype_R *)
+
+lemma createObjects_vms'[wp]:
+  "\<lbrace>(\<lambda>_.  (range_cover ptr sz  (objBitsKO val + gbits) n \<and> 0 < n)) and pspace_aligned' and
+     pspace_distinct' and pspace_no_overlap' ptr sz and valid_machine_state'\<rbrace>
+      createObjects ptr n val gbits
+   \<lbrace>\<lambda>rv. valid_machine_state'\<rbrace>"
+  apply (simp add: valid_machine_state'_def pointerInUserData_def pointerInDeviceData_def
+                   typ_at'_def)
+  apply (wp hoare_vcg_all_lift hoare_vcg_disj_lift createObjects_orig_ko_wp_at2'
+         | simp add: createObjects_def)+
+  apply auto
+  done
+
+lemma (in Retype_R) createObjects_ct_idle_or_in_cur_domain':
+  "\<lbrace>ct_active' and valid_pspace' and pspace_no_overlap' ptr sz
+       and ct_idle_or_in_cur_domain'
+       and K (range_cover ptr sz (objBitsKO val + gSize) n \<and> n \<noteq> 0)\<rbrace>
+     createObjects ptr n val gSize
+   \<lbrace>\<lambda>_. ct_idle_or_in_cur_domain'\<rbrace>"
+  apply (rule hoare_gen_asm)
+  apply (wp ct_idle_or_in_cur_domain'_lift_futz createObjects_obj_at_other[where sz=sz])
+    apply simp_all
+  done
+
+lemma untyped_zero_ranges_cte_def:
+  "untyped_ranges_zero_inv (cteCaps_of s) rs
+    = (\<forall>r. (\<exists>p. cte_wp_at' (\<lambda>cte. untypedZeroRange (cteCap cte) = Some r) p s)
+        = (r \<in> rs))"
+  apply (clarsimp simp: untyped_ranges_zero_inv_def cte_wp_at_ctes_of
+                        cteCaps_of_def set_eq_iff ran_def map_comp_Some_iff)
+  apply (safe, metis+)
+  done
+
+lemma (in Retype_R_2) corres_retype_update_gsI:
+  assumes not_zero: "n \<noteq> 0"
+  and      aligned: "is_aligned ptr (objBitsKO ko + gbits)"
+  and obj_bits_api: "obj_bits_api (APIType_map2 ty) us = objBitsKO ko + gbits"
+  and        check: "sz < obj_bits_api (APIType_map2 ty) us \<longleftrightarrow> sz < objBitsKO ko + gbits"
+  and          usv: "APIType_map2 ty = Structures_A.CapTableObject \<Longrightarrow> 0 < us"
+  and           ko: "makeObjectKO dev d ty = Some ko"
+  and          orr: "obj_bits_api (APIType_map2 ty) us \<le> sz \<Longrightarrow>
+                     obj_relation_retype (default_object (APIType_map2 ty) dev us d) ko"
+  and        cover: "range_cover ptr sz (obj_bits_api (APIType_map2 ty) us) n"
+  and            f: "f = update_gs (APIType_map2 ty) us"
+  shows "corres (\<lambda>rv rv'. rv' = g rv)
+         (\<lambda>s. valid_pspace s \<and> pspace_no_overlap_range_cover ptr sz s
+            \<and> valid_mdb s \<and> valid_list s)
+         (\<lambda>s. pspace_aligned' s \<and> pspace_distinct' s \<and>
+              pspace_no_overlap' ptr sz s \<and>
+              (ty = Inr (APIObjectType TCBObject) \<longrightarrow> d = ksCurDomain s))
+         (retype_region ptr n us (APIType_map2 ty) dev)
+         (do addrs \<leftarrow> createObjects ptr n ko gbits;
+             _ \<leftarrow> modify (f (set addrs));
+             return (g addrs)
+          od)"
+  using corres_retype' [OF not_zero aligned obj_bits_api check usv ko orr cover]
+  by (simp add: f)
+
+lemma gcd_corres: "corres (=) \<top> \<top> (gets cur_domain) curDomain"
+  by (simp add: curDomain_def state_relation_def)
+
+lemma createObjects_tcb_at':
+  "\<lbrakk>range_cover ptr sz (objBitsKO (injectKOS (makeObject::tcb))) n; n \<noteq> 0\<rbrakk> \<Longrightarrow>
+   \<lbrace>\<lambda>s. pspace_no_overlap' ptr sz s \<and> pspace_aligned' s \<and> pspace_distinct' s\<rbrace>
+   createObjects ptr n (KOTCB makeObject) 0
+   \<lbrace>\<lambda>ptrs s. \<forall>addr\<in>set ptrs. tcb_at' addr s\<rbrace>"
+  apply (rule hoare_strengthen_post[OF createObjects_ko_at_strg[where val = "(makeObject :: tcb)"]])
+  apply (auto simp: obj_at'_def project_inject objBitsKO_def objBits_def makeObject_tcb)
+  done
+
+lemma regroup_createObjects_dmo_userPages:
+  "(do
+      addrs <- createObjects y n ko sz;
+      _ <- modify (\<lambda>ks. ks\<lparr>gsUserPages := g ks addrs\<rparr>);
+      _ <- when P (mapM_x (\<lambda>addr. doMachineOp (m addr)) addrs);
+      return (f addrs)
+    od) = (do
+      (addrs, faddrs) <- (do
+        addrs <- createObjects y n ko sz;
+        _ <- modify (\<lambda>ks. ks\<lparr>gsUserPages := g ks addrs\<rparr>);
+        return (addrs, f addrs)
+       od);
+      _ <- when P (mapM_x (\<lambda>addr. doMachineOp (m addr)) addrs);
+      return faddrs
+    od)"
+  by (simp add: bind_assoc)
+
+lemma regroup_createObjects_dmo_gsPTTypes:
+  "(do
+      addrs <- createObjects y n ko sz;
+      _ <- modify (\<lambda>ks. ks\<lparr>ksArchState := gsPTTypes_update (g ks addrs) (ksArchState ks)\<rparr>);
+      _ <- mapM_x (\<lambda>addr. doMachineOp (m addr)) addrs;
+      return (f addrs)
+    od) = (do
+      (addrs, faddrs) <- (do
+        addrs <- createObjects y n ko sz;
+        _ <- modify (\<lambda>ks. ks\<lparr>ksArchState := gsPTTypes_update (g ks addrs) (ksArchState ks)\<rparr>);
+        return (addrs, f addrs)
+       od);
+      _ <- mapM_x (\<lambda>addr. doMachineOp (m addr)) addrs;
+      return faddrs
+    od)"
+  by (simp add: bind_assoc)
+
 end
